<?xml version="1.0"?>
<rdf:RDF xmlns="http://www.semanticweb.org/k_mil/ontologies/2021/8/EvalLOD#"
     xml:base="http://www.semanticweb.org/k_mil/ontologies/2021/8/EvalLOD"
     xmlns:dc="http://purl.org/dc/elements/1.1/"
     xmlns:ns="http://www.w3.org/2003/06/sw-vocab-status/ns#"
     xmlns:oa="http://www.w3.org/ns/oa#"
     xmlns:owl="http://www.w3.org/2002/07/owl#"
     xmlns:rdf="http://www.w3.org/1999/02/22-rdf-syntax-ns#"
     xmlns:wot="http://xmlns.com/wot/0.1/"
     xmlns:xml="http://www.w3.org/XML/1998/namespace"
     xmlns:xsd="http://www.w3.org/2001/XMLSchema#"
     xmlns:adms="http://www.w3.org/ns/adms#"
     xmlns:foaf="http://xmlns.com/foaf/0.1/"
     xmlns:prov="http://www.w3.org/ns/prov#"
     xmlns:rdfs="http://www.w3.org/2000/01/rdf-schema#"
     xmlns:swrl="http://www.w3.org/2003/11/swrl#"
     xmlns:vann="http://purl.org/vocab/vann/"
     xmlns:void="http://rdfs.org/ns/void#"
     xmlns:swrla="http://swrl.stanford.edu/ontologies/3.3/swrla.owl#"
     xmlns:swrlb="http://www.w3.org/2003/11/swrlb#"
     xmlns:terms="http://purl.org/dc/terms/"
     xmlns:schema="https://schema.org/">
    <owl:Ontology rdf:about="http://www.semanticweb.org/k_mil/ontologies/2021/8/EvalLOD">
        <owl:imports rdf:resource="http://protege.stanford.edu/plugins/owl/dc/dublincore.owl"/>
        <owl:imports rdf:resource="http://purl.org/dc/elements/1.1/"/>
        <owl:imports rdf:resource="http://vocab.deri.ie/void"/>
        <owl:imports rdf:resource="http://www.w3.org/ns/prov-o-20130430"/>
        <owl:imports rdf:resource="http://www.w3.org/ns/oa#"/>
        <dc:description xml:lang="en-us"> 
     The Dublin Core Element Set v1.1 namespace  
     provides URIs for the Dublin Core Elements v1.1.  
     Entries are declared using OWL language to  
     support OWL applications. 
  </dc:description>
        <dc:description xml:lang="en-us">The Dublin Core Terms namespace provides URIs for the Dublin Core Element Set Qualifier Vocabulary. Vocabulary terms are declared using RDF Schema language to support RDF applications. The Dublin Core qualifiers form a richer vocabulary, which is intended to facilitate discovery of resources. It will be updated according to dc-usage decisions.</dc:description>
        <dc:description xml:lang="en-us">The Dublin Core Types namespace provides URIs for the entries of the DCMI Type Vocabulary. Entries are declared using RDF Schema language to support RDF applications. The Schema will be updated according to dc-usage decisions.</dc:description>
        <dc:description>The Friend of a Friend (FOAF) RDF vocabulary, described using W3C RDF Schema and the Web Ontology Language.</dc:description>
        <dc:language xml:lang="en-us"> 
     English 
  </dc:language>
        <dc:language xml:lang="en-us">English</dc:language>
        <dc:publisher xml:lang="en-us"> 
     The Dublin Core Metadata Initiative 
  </dc:publisher>
        <dc:publisher xml:lang="en-us">The Dublin Core Metadata Initiative</dc:publisher>
        <dc:source rdf:resource="http://dublincore.org/documents/dces/"/>
        <dc:source rdf:resource="http://dublincore.org/documents/dcmi-type-vocabulary/"/>
        <dc:source rdf:resource="http://dublincore.org/usage/decisions/"/>
        <dc:source rdf:resource="http://dublincore.org/usage/terms/"/>
        <dc:source rdf:resource="http://www.dublincore.org/documents/2000/07/11/dcmes-qualifiers/"/>
        <dc:source rdf:resource="http://www.dublincore.org/usage/decisions/"/>
        <dc:title xml:lang="en-us"> 
     The Dublin Core Element Set v1.1 namespace  
     providing access to its content by means of an  
     OWL DL Ontology 
  </dc:title>
        <dc:title>Friend of a Friend (FOAF) vocabulary</dc:title>
        <dc:title xml:lang="en-us">The DCMI Types namespace providing access to its content by means of an RDF Schema</dc:title>
        <dc:title xml:lang="en-us">The Dublin Core Terms Namespace providing access to its content by means of an RDF Schema.</dc:title>
        <dc:title>Web Annotation Ontology</dc:title>
        <terms:created rdf:datatype="http://www.w3.org/2001/XMLSchema#date">2010-01-26</terms:created>
        <terms:creator>
            <rdf:Description>
                <rdf:type rdf:resource="https://schema.org/Person"/>
                <schema:affiliation>
                    <rdf:Description>
                        <rdf:type rdf:resource="https://schema.org/Organization"/>
                    </rdf:Description>
                </schema:affiliation>
                <schema:email rdf:resource="mailto:richard.cyganiak@deri.org"/>
                <schema:name>Richard Cyganiak</schema:name>
                <schema:url rdf:resource="http://richard.cyganiak.de/"/>
            </rdf:Description>
        </terms:creator>
        <terms:creator>
            <rdf:Description>
                <rdf:type rdf:resource="https://schema.org/Person"/>
                <schema:affiliation>
                    <rdf:Description>
                        <rdf:type rdf:resource="https://schema.org/Organization"/>
                        <schema:name>Department of Zoology, University of Oxford</schema:name>
                        <schema:url rdf:resource="http://www.zoo.ox.ac.uk/"/>
                    </rdf:Description>
                </schema:affiliation>
                <schema:email rdf:resource="mailto:jun.zhao@zoo.ox.ac.uk"/>
                <schema:name>Jun Zhao</schema:name>
                <schema:url rdf:resource="http://users.ox.ac.uk/~zool0770/"/>
            </rdf:Description>
        </terms:creator>
        <terms:creator>
            <rdf:Description>
                <rdf:type rdf:resource="https://schema.org/Person"/>
                <schema:affiliation>
                    <rdf:Description>
                        <rdf:type rdf:resource="https://schema.org/Organization"/>
                        <schema:name>Talis</schema:name>
                        <schema:url rdf:resource="http://www.talis.com/"/>
                    </rdf:Description>
                </schema:affiliation>
                <schema:email rdf:resource="mailto:Keith.Alexander@talis.com"/>
                <schema:name>Keith Alexander</schema:name>
                <schema:url rdf:resource="http://kwijibo.talis.com/"/>
            </rdf:Description>
        </terms:creator>
        <terms:creator>
            <rdf:Description>
                <rdf:type rdf:resource="https://schema.org/Person"/>
                <schema:affiliation>
                    <rdf:Description>
                        <rdf:type rdf:resource="https://schema.org/Organization"/>
                        <schema:name>LiDRC</schema:name>
                        <schema:url rdf:resource="http://linkeddata.deri.ie/"/>
                    </rdf:Description>
                </schema:affiliation>
                <schema:email rdf:resource="mailto:michael.hausenblas@deri.org"/>
                <schema:name>Michael Hausenblas</schema:name>
                <schema:url rdf:resource="http://sw-app.org/about.html"/>
            </rdf:Description>
        </terms:creator>
        <terms:creator>
            <rdf:Description>
                <rdf:type rdf:resource="http://xmlns.com/foaf/0.1/Person"/>
            </rdf:Description>
        </terms:creator>
        <terms:creator>
            <rdf:Description>
                <rdf:type rdf:resource="http://xmlns.com/foaf/0.1/Person"/>
            </rdf:Description>
        </terms:creator>
        <terms:creator>
            <rdf:Description>
                <rdf:type rdf:resource="http://xmlns.com/foaf/0.1/Person"/>
            </rdf:Description>
        </terms:creator>
        <terms:description>The Vocabulary of Interlinked Datasets (VoID) is an RDF Schema vocabulary for expressing metadata about RDF datasets. It is intended as a bridge between the publishers and users of RDF data, with applications ranging from data discovery to cataloging and archiving of datasets. This document provides a formal definition of the new RDF classes and properties introduced for VoID. It is a companion to the main specification document for VoID, &lt;em&gt;&lt;a href=&quot;http://www.w3.org/TR/void/&quot;&gt;Describing Linked Datasets with the VoID Vocabulary&lt;/a&gt;&lt;/em&gt;.</terms:description>
        <terms:isReferencedBy rdf:resource="http://purl.org/dc/dcmitype/"/>
        <terms:isReferencedBy rdf:resource="http://purl.org/dc/terms/"/>
        <terms:isReferencedBy rdf:resource="http://www.dublincore.org/documents/2001/10/26/dcmi-namespace/"/>
        <terms:isRequiredBy rdf:resource="http://purl.org/dc/terms/"/>
        <terms:issued> 
     1999-07-02 
  </terms:issued>
        <terms:issued>2000-07-11</terms:issued>
        <terms:modified> 
     2003-09-2 
  </terms:modified>
        <terms:modified>2003-03-24</terms:modified>
        <terms:modified>2016-11-12T21:28:11Z</terms:modified>
        <terms:modified rdf:datatype="http://www.w3.org/2001/XMLSchema#date">2011-03-06</terms:modified>
        <terms:partOf rdf:resource="http://vocab.deri.ie"/>
        <terms:publisher>
            <rdf:Description>
                <rdfs:seeAlso rdf:resource="http://www.insight-centre.org"/>
                <rdfs:seeAlso rdf:resource="http://www.deri.ie/"/>
                <schema:identifier rdf:resource="http://vocab.deri.ie/void#Digital%20Enterprise%20Research%20Institute%2C%20NUI%20Galway"/>
                <schema:name>Digital Enterprise Research Institute, NUI Galway</schema:name>
            </rdf:Description>
        </terms:publisher>
        <terms:references rdf:resource="http://purl.org/dc/dcmitype/"/>
        <terms:requires rdf:resource="http://dublincore.org/documents/dcmi-type-vocabulary/"/>
        <terms:requires rdf:resource="http://purl.org/dc/elements/1.1/"/>
        <terms:status rdf:resource="http://purl.org/adms/status/UnderDevelopment"/>
        <terms:type rdf:resource="http://purl.org/adms/assettype/Ontology"/>
        <vann:preferredNamespacePrefix>void</vann:preferredNamespacePrefix>
        <vann:preferredNamespaceUri>http://rdfs.org/ns/void#</vann:preferredNamespaceUri>
        <rdfs:comment>The Web Annotation ontology defines the terms of the Web Annotation vocabulary. Any changes to this document MUST be from a Working Group in the W3C that has established expertise in the area.</rdfs:comment>
        <rdfs:comment xml:lang="en">This document defines a vocabulary to describe the trustworthiness of RDF data according to our trust model for RDF. Our trust model associates every RDF statement with a trust value which is either unknown or a number in the interval [-1,1]. The trust model is local, i.e., the trust values are specific to an information consumer.
We designed this vocabulary to permit its application in other use cases; i.e., the vocabulary can be used to assign trust values to anything, not just RDF statements.</rdfs:comment>
        <rdfs:comment xml:lang="en">This document is published by the Provenance Working Group (http://www.w3.org/2011/prov/wiki/Main_Page). 

If you wish to make comments regarding this document, please send them to public-prov-comments@w3.org (subscribe public-prov-comments-request@w3.org, archives http://lists.w3.org/Archives/Public/public-prov-comments/). All feedback is welcome.</rdfs:comment>
        <rdfs:label xml:lang="en">W3C PROVenance Interchange Ontology (PROV-O)</rdfs:label>
        <rdfs:seeAlso rdf:resource="http://www.w3.org/TR/annotation-vocab/"/>
        <rdfs:seeAlso rdf:resource="http://www.w3.org/TR/prov-o/"/>
        <rdfs:seeAlso rdf:resource="http://www.w3.org/ns/prov"/>
        <owl:versionInfo>2016-11-12T21:28:11Z</owl:versionInfo>
        <owl:versionInfo xml:lang="en">Recommendation version 2013-04-30</owl:versionInfo>
    </owl:Ontology>
    


    <!-- 
    ///////////////////////////////////////////////////////////////////////////////////////
    //
    // Annotation properties
    //
    ///////////////////////////////////////////////////////////////////////////////////////
     -->

    


    <!-- http://purl.org/dc/elements/1.1/contributor -->

    <owl:AnnotationProperty rdf:about="http://purl.org/dc/elements/1.1/contributor">
        <dc:description xml:lang="en-us">Examples of a Contributor include a person, an 
         organisation, or a service.  Typically, the name of a 
         Contributor should be used to indicate the entity.</dc:description>
        <dc:type rdf:resource="http://dublincore.org/usage/documents/principles/#element"/>
        <terms:hasVersion rdf:resource="http://dublincore.org/usage/terms/history/#contributor-004"/>
        <terms:issued>1999-07-02</terms:issued>
        <terms:modified>2002-10-04</terms:modified>
        <rdfs:comment xml:lang="en-us">An entity responsible for making contributions to the
         content of the resource.</rdfs:comment>
        <rdfs:isDefinedBy rdf:resource="http://purl.org/dc/elements/1.1/"/>
        <rdfs:label xml:lang="en-us">Contributor</rdfs:label>
    </owl:AnnotationProperty>
    


    <!-- http://purl.org/dc/elements/1.1/coverage -->

    <owl:AnnotationProperty rdf:about="http://purl.org/dc/elements/1.1/coverage">
        <dc:description xml:lang="en-us">Coverage will typically include spatial location (a place name
         or geographic coordinates), temporal period (a period label,
         date, or date range) or jurisdiction (such as a named
         administrative entity).
         Recommended best practice is to select a value from a
         controlled vocabulary (for example, the Thesaurus of Geographic
         Names [TGN]) and that, where appropriate, named places or time
         periods be used in preference to numeric identifiers such as
         sets of coordinates or date ranges.</dc:description>
        <dc:type rdf:resource="http://dublincore.org/usage/documents/principles/#element"/>
        <terms:hasVersion rdf:resource="http://dublincore.org/usage/terms/history/#coverage-004"/>
        <terms:issued>1999-07-02</terms:issued>
        <terms:modified>2002-10-04</terms:modified>
        <rdfs:comment xml:lang="en-us">The extent or scope of the content of the resource.</rdfs:comment>
        <rdfs:isDefinedBy rdf:resource="http://purl.org/dc/elements/1.1/"/>
        <rdfs:label xml:lang="en-us">Coverage</rdfs:label>
    </owl:AnnotationProperty>
    


    <!-- http://purl.org/dc/elements/1.1/creator -->

    <owl:AnnotationProperty rdf:about="http://purl.org/dc/elements/1.1/creator">
        <dc:description xml:lang="en-us">Examples of a Creator include a person, an organisation,
         or a service.  Typically, the name of a Creator should 
         be used to indicate the entity.</dc:description>
        <dc:type rdf:resource="http://dublincore.org/usage/documents/principles/#element"/>
        <terms:hasVersion rdf:resource="http://dublincore.org/usage/terms/history/#creator-004"/>
        <terms:issued>1999-07-02</terms:issued>
        <terms:modified>2002-10-04</terms:modified>
        <rdfs:comment xml:lang="en-us">An entity primarily responsible for making the content 
         of the resource.</rdfs:comment>
        <rdfs:isDefinedBy rdf:resource="http://purl.org/dc/elements/1.1/"/>
        <rdfs:label xml:lang="en-us">Creator</rdfs:label>
    </owl:AnnotationProperty>
    


    <!-- http://purl.org/dc/elements/1.1/date -->

    <owl:AnnotationProperty rdf:about="http://purl.org/dc/elements/1.1/date">
        <dc:description xml:lang="en-us">Typically, Date will be associated with the creation or
         availability of the resource.  Recommended best practice
         for encoding the date value is defined in a profile of
         ISO 8601 [W3CDTF] and follows the YYYY-MM-DD format.</dc:description>
        <dc:type rdf:resource="http://dublincore.org/usage/documents/principles/#element"/>
        <terms:hasVersion rdf:resource="http://dublincore.org/usage/terms/history/#date-004"/>
        <terms:issued>1999-07-02</terms:issued>
        <terms:modified>2002-10-04</terms:modified>
        <rdfs:comment xml:lang="en-us">A date associated with an event in the life cycle of the
         resource.</rdfs:comment>
        <rdfs:isDefinedBy rdf:resource="http://purl.org/dc/elements/1.1/"/>
        <rdfs:label xml:lang="en-us">Date</rdfs:label>
    </owl:AnnotationProperty>
    


    <!-- http://purl.org/dc/elements/1.1/description -->

    <owl:AnnotationProperty rdf:about="http://purl.org/dc/elements/1.1/description">
        <dc:description xml:lang="en-us">Description may include but is not limited to: an abstract,
         table of contents, reference to a graphical representation
         of content or a free-text account of the content.</dc:description>
        <dc:type rdf:resource="http://dublincore.org/usage/documents/principles/#element"/>
        <terms:hasVersion rdf:resource="http://dublincore.org/usage/terms/history/#description-004"/>
        <terms:issued>1999-07-02</terms:issued>
        <terms:modified>2002-10-04</terms:modified>
        <rdfs:comment xml:lang="en-us">An account of the content of the resource.</rdfs:comment>
        <rdfs:isDefinedBy rdf:resource="http://purl.org/dc/elements/1.1/"/>
        <rdfs:label xml:lang="en-us">Description</rdfs:label>
    </owl:AnnotationProperty>
    


    <!-- http://purl.org/dc/elements/1.1/format -->

    <owl:AnnotationProperty rdf:about="http://purl.org/dc/elements/1.1/format">
        <dc:description xml:lang="en-us">Typically, Format may include the media-type or dimensions of
         the resource. Format may be used to determine the software,
         hardware or other equipment needed to display or operate the
         resource. Examples of dimensions include size and duration.
         Recommended best practice is to select a value from a
         controlled vocabulary (for example, the list of Internet Media
         Types [MIME] defining computer media formats).</dc:description>
        <dc:type rdf:resource="http://dublincore.org/usage/documents/principles/#element"/>
        <terms:hasVersion rdf:resource="http://dublincore.org/usage/terms/history/#format-004"/>
        <terms:issued>1999-07-02</terms:issued>
        <terms:modified>2002-10-04</terms:modified>
        <rdfs:comment xml:lang="en-us">The physical or digital manifestation of the resource.</rdfs:comment>
        <rdfs:isDefinedBy rdf:resource="http://purl.org/dc/elements/1.1/"/>
        <rdfs:label xml:lang="en-us">Format</rdfs:label>
    </owl:AnnotationProperty>
    


    <!-- http://purl.org/dc/elements/1.1/identifier -->

    <owl:AnnotationProperty rdf:about="http://purl.org/dc/elements/1.1/identifier">
        <dc:description xml:lang="en-us">Recommended best practice is to identify the resource by means
         of a string or number conforming to a formal identification
         system.
         Example formal identification systems include the Uniform
         Resource Identifier (URI) (including the Uniform Resource
         Locator (URL)), the Digital Object Identifier (DOI) and the
         International Standard Book Number (ISBN).</dc:description>
        <dc:type rdf:resource="http://dublincore.org/usage/documents/principles/#element"/>
        <terms:hasVersion rdf:resource="http://dublincore.org/usage/terms/history/#identifier-004"/>
        <terms:issued>1999-07-02</terms:issued>
        <terms:modified>2002-10-04</terms:modified>
        <rdfs:comment xml:lang="en-us">An unambiguous reference to the resource within a given context.</rdfs:comment>
        <rdfs:isDefinedBy rdf:resource="http://purl.org/dc/elements/1.1/"/>
        <rdfs:label xml:lang="en-us">Resource Identifier</rdfs:label>
    </owl:AnnotationProperty>
    


    <!-- http://purl.org/dc/elements/1.1/language -->

    <owl:AnnotationProperty rdf:about="http://purl.org/dc/elements/1.1/language">
        <dc:description xml:lang="en-us">Recommended best practice is to use RFC 3066 [RFC3066],
         which, in conjunction with ISO 639 [ISO639], defines two-
         and three-letter primary language tags with optional
         subtags.  Examples include &quot;en&quot; or &quot;eng&quot; for English,
         &quot;akk&quot; for Akkadian, and &quot;en-GB&quot; for English used in the
         United Kingdom.</dc:description>
        <dc:type rdf:resource="http://dublincore.org/usage/documents/principles/#element"/>
        <terms:hasVersion rdf:resource="http://dublincore.org/usage/terms/history/#language-005"/>
        <terms:issued>1999-07-02</terms:issued>
        <terms:modified>2002-10-04</terms:modified>
        <rdfs:comment xml:lang="en-us">A language of the intellectual content of the resource.</rdfs:comment>
        <rdfs:isDefinedBy rdf:resource="http://purl.org/dc/elements/1.1/"/>
        <rdfs:label xml:lang="en-us">Language</rdfs:label>
    </owl:AnnotationProperty>
    


    <!-- http://purl.org/dc/elements/1.1/publisher -->

    <owl:AnnotationProperty rdf:about="http://purl.org/dc/elements/1.1/publisher">
        <dc:description xml:lang="en-us">Examples of a Publisher include a person, an organisation,
         or a service.
         Typically, the name of a Publisher should be used to
         indicate the entity.</dc:description>
        <dc:type rdf:resource="http://dublincore.org/usage/documents/principles/#element"/>
        <terms:hasVersion rdf:resource="http://dublincore.org/usage/terms/history/#publisher-004"/>
        <terms:issued>1999-07-02</terms:issued>
        <terms:modified>2002-10-04</terms:modified>
        <rdfs:comment xml:lang="en-us">An entity responsible for making the resource available</rdfs:comment>
        <rdfs:isDefinedBy rdf:resource="http://purl.org/dc/elements/1.1/"/>
        <rdfs:label xml:lang="en-us">Publisher</rdfs:label>
    </owl:AnnotationProperty>
    


    <!-- http://purl.org/dc/elements/1.1/relation -->

    <owl:AnnotationProperty rdf:about="http://purl.org/dc/elements/1.1/relation">
        <dc:description xml:lang="en-us">
         Recommended best practice is to reference the resource by means
         of a string or number conforming to a formal identification
         system.
    </dc:description>
        <dc:type rdf:resource="http://dublincore.org/usage/documents/principles/#element"/>
        <terms:hasVersion rdf:resource="http://dublincore.org/usage/terms/history/#relation-004"/>
        <terms:issued>1999-07-02</terms:issued>
        <terms:modified>2002-10-04</terms:modified>
        <rdfs:comment xml:lang="en-us">A reference to a related resource.</rdfs:comment>
        <rdfs:isDefinedBy rdf:resource="http://purl.org/dc/elements/1.1/"/>
        <rdfs:label xml:lang="en-us">Relation</rdfs:label>
    </owl:AnnotationProperty>
    


    <!-- http://purl.org/dc/elements/1.1/rights -->

    <owl:AnnotationProperty rdf:about="http://purl.org/dc/elements/1.1/rights">
        <dc:description xml:lang="en-us">
          Typically, a Rights element will contain a rights 
          management statement for the resource, or reference 
          a service providing such information. Rights information 
          often encompasses Intellectual Property Rights (IPR), 
          Copyright, and various Property Rights. 
          If the Rights element is absent, no assumptions can be made 
          about the status of these and other rights with respect to 
          the resource.
    </dc:description>
        <dc:type rdf:resource="http://dublincore.org/usage/documents/principles/#element"/>
        <terms:hasVersion rdf:resource="http://dublincore.org/usage/terms/history/#rights-004"/>
        <terms:issued>1999-07-02</terms:issued>
        <terms:modified>2002-10-04</terms:modified>
        <rdfs:comment xml:lang="en-us">Information about rights held in and over the resource.</rdfs:comment>
        <rdfs:isDefinedBy rdf:resource="http://purl.org/dc/elements/1.1/"/>
        <rdfs:label xml:lang="en-us">Rights Management</rdfs:label>
    </owl:AnnotationProperty>
    


    <!-- http://purl.org/dc/elements/1.1/source -->

    <owl:AnnotationProperty rdf:about="http://purl.org/dc/elements/1.1/source">
        <dc:description xml:lang="en-us">The present resource may be derived from the Source resource
         in whole or in part.  Recommended best practice is to reference
         the resource by means of a string or number conforming to a
         formal identification system.</dc:description>
        <dc:type rdf:resource="http://dublincore.org/usage/documents/principles/#element"/>
        <terms:hasVersion rdf:resource="http://dublincore.org/usage/terms/history/#source-004"/>
        <terms:issued>1999-07-02</terms:issued>
        <terms:modified>2002-10-04</terms:modified>
        <rdfs:comment xml:lang="en-us">A reference to a resource from which the present resource
         is derived.</rdfs:comment>
        <rdfs:isDefinedBy rdf:resource="http://purl.org/dc/elements/1.1/"/>
        <rdfs:label xml:lang="en-us">Source</rdfs:label>
    </owl:AnnotationProperty>
    


    <!-- http://purl.org/dc/elements/1.1/subject -->

    <owl:AnnotationProperty rdf:about="http://purl.org/dc/elements/1.1/subject">
        <dc:description xml:lang="en-us">Typically, a Subject will be expressed as keywords,
         key phrases or classification codes that describe a topic
         of the resource.  Recommended best practice is to select 
         a value from a controlled vocabulary or formal 
         classification scheme.</dc:description>
        <dc:type rdf:resource="http://dublincore.org/usage/documents/principles/#element"/>
        <terms:hasVersion rdf:resource="http://dublincore.org/usage/terms/history/#subject-004"/>
        <terms:issued>1999-07-02</terms:issued>
        <terms:modified>2002-10-04</terms:modified>
        <rdfs:comment xml:lang="en-us">The topic of the content of the resource.</rdfs:comment>
        <rdfs:isDefinedBy rdf:resource="http://purl.org/dc/elements/1.1/"/>
        <rdfs:label xml:lang="en-us">Subject and Keywords</rdfs:label>
    </owl:AnnotationProperty>
    


    <!-- http://purl.org/dc/elements/1.1/title -->

    <owl:AnnotationProperty rdf:about="http://purl.org/dc/elements/1.1/title">
        <dc:description xml:lang="en-us">
        Typically, a Title will be a name by which the resource is
         formally known.
    </dc:description>
        <dc:type rdf:resource="http://dublincore.org/usage/documents/principles/#element"/>
        <terms:hasVersion rdf:resource="http://dublincore.org/usage/terms/history/#title-004"/>
        <terms:issued>1999-07-02</terms:issued>
        <terms:modified>2002-10-04</terms:modified>
        <rdfs:comment xml:lang="en-us">A name given to the resource.</rdfs:comment>
        <rdfs:isDefinedBy rdf:resource="http://purl.org/dc/elements/1.1/"/>
        <rdfs:label xml:lang="en-us">Title</rdfs:label>
    </owl:AnnotationProperty>
    


    <!-- http://purl.org/dc/elements/1.1/type -->

    <owl:AnnotationProperty rdf:about="http://purl.org/dc/elements/1.1/type">
        <dc:description xml:lang="en-us">Type includes terms describing general categories, functions,
         genres, or aggregation levels for content. Recommended best
         practice is to select a value from a controlled vocabulary
         (for example, the DCMI Type Vocabulary [DCMITYPE]). To 
         describe the physical or digital manifestation of the 
         resource, use the Format element.</dc:description>
        <dc:type rdf:resource="http://dublincore.org/usage/documents/principles/#element"/>
        <terms:hasVersion rdf:resource="http://dublincore.org/usage/terms/history/#type-004"/>
        <terms:issued>1999-07-02</terms:issued>
        <terms:modified>2002-10-04</terms:modified>
        <rdfs:comment xml:lang="en-us">The nature or genre of the content of the resource.</rdfs:comment>
        <rdfs:isDefinedBy rdf:resource="http://purl.org/dc/elements/1.1/"/>
        <rdfs:label xml:lang="en-us">Resource Type</rdfs:label>
    </owl:AnnotationProperty>
    


    <!-- http://purl.org/dc/terms/abstract -->

    <owl:AnnotationProperty rdf:about="http://purl.org/dc/terms/abstract">
        <dc:type rdf:resource="http://dublincore.org/usage/documents/principles/#element-refinement"/>
        <terms:hasVersion rdf:resource="http://dublincore.org/usage/terms/history/#abstract-002"/>
        <terms:issued>2000-07-11</terms:issued>
        <terms:modified>2002-06-15</terms:modified>
        <rdfs:comment xml:lang="en-us">A summary of the content of the resource.</rdfs:comment>
        <rdfs:isDefinedBy rdf:resource="http://purl.org/dc/terms/"/>
        <rdfs:label xml:lang="en-us">Abstract</rdfs:label>
    </owl:AnnotationProperty>
    


    <!-- http://purl.org/dc/terms/accessRights -->

    <owl:AnnotationProperty rdf:about="http://purl.org/dc/terms/accessRights">
        <dc:description xml:lang="en-us">Access Rights may include information
            regarding access or restrictions based on privacy, 
            security or other regulations.
            </dc:description>
        <dc:type rdf:resource="http://dublincore.org/usage/documents/principles/#element-refinement"/>
        <terms:hasVersion rdf:resource="http://dublincore.org/usage/terms/history/#accessRights-001"/>
        <terms:issued>2003-02-15</terms:issued>
        <rdfs:comment xml:lang="en-us">Information about who can access the
            resource or an indication of its security status.
            </rdfs:comment>
        <rdfs:isDefinedBy rdf:resource="http://purl.org/dc/terms/"/>
        <rdfs:label xml:lang="en-us">Access Rights</rdfs:label>
    </owl:AnnotationProperty>
    


    <!-- http://purl.org/dc/terms/alternative -->

    <owl:AnnotationProperty rdf:about="http://purl.org/dc/terms/alternative">
        <dc:description xml:lang="en-us">This qualifier can include Title abbreviations as well 
            as translations.</dc:description>
        <dc:type rdf:resource="http://dublincore.org/usage/documents/principles/#element-refinement"/>
        <terms:hasVersion rdf:resource="http://dublincore.org/usage/terms/history/#alternative-002"/>
        <terms:issued>2000-07-11</terms:issued>
        <terms:modified>2002-06-15</terms:modified>
        <rdfs:comment xml:lang="en-us">Any form of the title used as a substitute or alternative 
            to the formal title of the resource.</rdfs:comment>
        <rdfs:isDefinedBy rdf:resource="http://purl.org/dc/terms/"/>
        <rdfs:label xml:lang="en-us">Alternative</rdfs:label>
    </owl:AnnotationProperty>
    


    <!-- http://purl.org/dc/terms/audience -->

    <owl:AnnotationProperty rdf:about="http://purl.org/dc/terms/audience">
        <dc:description xml:lang="en-us">A class of entity may be determined by the creator or the 
            publisher or by a third party.</dc:description>
        <dc:type rdf:resource="http://dublincore.org/usage/documents/principles/#element"/>
        <terms:hasVersion rdf:resource="http://dublincore.org/usage/terms/history/#audience-002"/>
        <terms:issued>2001-05-21</terms:issued>
        <terms:modified>2002-06-15</terms:modified>
        <rdfs:comment xml:lang="en-us">A class of entity for whom the resource is intended or useful.</rdfs:comment>
        <rdfs:isDefinedBy rdf:resource="http://purl.org/dc/terms/"/>
        <rdfs:label xml:lang="en-us">Audience</rdfs:label>
    </owl:AnnotationProperty>
    


    <!-- http://purl.org/dc/terms/available -->

    <owl:AnnotationProperty rdf:about="http://purl.org/dc/terms/available">
        <dc:type rdf:resource="http://dublincore.org/usage/documents/principles/#element-refinement"/>
        <terms:hasVersion rdf:resource="http://dublincore.org/usage/terms/history/#available-002"/>
        <terms:issued>2000-07-11</terms:issued>
        <terms:modified>2002-06-15</terms:modified>
        <rdfs:comment xml:lang="en-us">Date (often a range) that the resource will become or did 
            become available.</rdfs:comment>
        <rdfs:isDefinedBy rdf:resource="http://purl.org/dc/terms/"/>
        <rdfs:label xml:lang="en-us">Available</rdfs:label>
    </owl:AnnotationProperty>
    


    <!-- http://purl.org/dc/terms/bibliographicCitation -->

    <owl:AnnotationProperty rdf:about="http://purl.org/dc/terms/bibliographicCitation">
        <dc:description xml:lang="en-us">Recommended practice is to include sufficient 
            bibliographic detail to identify the resource as 
            unambiguously as possible, whether or not the
            citation is in a standard form.
            </dc:description>
        <dc:type rdf:resource="http://dublincore.org/usage/documents/principles/#element-refinement"/>
        <terms:hasVersion rdf:resource="http://dublincore.org/usage/terms/history/#bibliographicCitation-001"/>
        <terms:issued>2003-02-15</terms:issued>
        <rdfs:comment xml:lang="en-us">A bibliographic reference for the resource.
            </rdfs:comment>
        <rdfs:isDefinedBy rdf:resource="http://purl.org/dc/terms/"/>
        <rdfs:label xml:lang="en-us">Bibliographic Citation</rdfs:label>
    </owl:AnnotationProperty>
    


    <!-- http://purl.org/dc/terms/conformsTo -->

    <owl:AnnotationProperty rdf:about="http://purl.org/dc/terms/conformsTo">
        <dc:type rdf:resource="http://dublincore.org/usage/documents/principles/#element-refinement"/>
        <terms:hasVersion rdf:resource="http://dublincore.org/usage/terms/history/#conformsTo-002"/>
        <terms:issued>2001-05-21</terms:issued>
        <terms:modified>2002-06-15</terms:modified>
        <rdfs:comment xml:lang="en-us">A reference to an established standard to which the resource conforms.</rdfs:comment>
        <rdfs:isDefinedBy rdf:resource="http://purl.org/dc/terms/"/>
        <rdfs:label xml:lang="en-us">Conforms To</rdfs:label>
    </owl:AnnotationProperty>
    


    <!-- http://purl.org/dc/terms/created -->

    <owl:AnnotationProperty rdf:about="http://purl.org/dc/terms/created">
        <dc:type rdf:resource="http://dublincore.org/usage/documents/principles/#element-refinement"/>
        <terms:hasVersion rdf:resource="http://dublincore.org/usage/terms/history/#created-002"/>
        <terms:issued>2000-07-11</terms:issued>
        <terms:modified>2002-06-15</terms:modified>
        <rdfs:comment xml:lang="en-us">Date of creation of the resource.</rdfs:comment>
        <rdfs:isDefinedBy rdf:resource="http://purl.org/dc/terms/"/>
        <rdfs:label xml:lang="en-us">Created</rdfs:label>
    </owl:AnnotationProperty>
    


    <!-- http://purl.org/dc/terms/dateAccepted -->

    <owl:AnnotationProperty rdf:about="http://purl.org/dc/terms/dateAccepted">
        <dc:type rdf:resource="http://dublincore.org/usage/documents/principles/#element-refinement"/>
        <terms:hasVersion rdf:resource="http://dublincore.org/usage/terms/history/#dateAccepted-001"/>
        <terms:issued>2002-07-13</terms:issued>
        <rdfs:comment xml:lang="en-us">Date of acceptance of the resource (e.g. of thesis
            by university department, of article by journal, etc.).</rdfs:comment>
        <rdfs:isDefinedBy rdf:resource="http://purl.org/dc/terms/"/>
        <rdfs:label xml:lang="en-us">Date Accepted</rdfs:label>
    </owl:AnnotationProperty>
    


    <!-- http://purl.org/dc/terms/dateCopyrighted -->

    <owl:AnnotationProperty rdf:about="http://purl.org/dc/terms/dateCopyrighted">
        <dc:type rdf:resource="http://dublincore.org/usage/documents/principles/#element-refinement"/>
        <terms:hasVersion rdf:resource="http://dublincore.org/usage/terms/history/#dateCopyrighted-001"/>
        <terms:issued>2002-07-13</terms:issued>
        <rdfs:comment xml:lang="en-us">Date of a statement of copyright.</rdfs:comment>
        <rdfs:isDefinedBy rdf:resource="http://purl.org/dc/terms/"/>
        <rdfs:label xml:lang="en-us">Date Copyrighted</rdfs:label>
    </owl:AnnotationProperty>
    


    <!-- http://purl.org/dc/terms/dateSubmitted -->

    <owl:AnnotationProperty rdf:about="http://purl.org/dc/terms/dateSubmitted">
        <dc:type rdf:resource="http://dublincore.org/usage/documents/principles/#element-refinement"/>
        <terms:hasVersion rdf:resource="http://dublincore.org/usage/terms/history/#dateSubmitted-001"/>
        <terms:issued>2002-07-13</terms:issued>
        <rdfs:comment xml:lang="en-us">Date of submission of the resource (e.g. thesis, 
            articles, etc.).</rdfs:comment>
        <rdfs:isDefinedBy rdf:resource="http://purl.org/dc/terms/"/>
        <rdfs:label xml:lang="en-us">Date Submitted</rdfs:label>
    </owl:AnnotationProperty>
    


    <!-- http://purl.org/dc/terms/educationLevel -->

    <owl:AnnotationProperty rdf:about="http://purl.org/dc/terms/educationLevel">
        <dc:type rdf:resource="http://dublincore.org/usage/documents/principles/#element-refinement"/>
        <terms:hasVersion rdf:resource="http://dublincore.org/usage/terms/history/#educationLevel-001"/>
        <terms:issued>2002-07-13</terms:issued>
        <rdfs:comment xml:lang="en-us">A general statement describing the education or 
            training context.  Alternatively, a more specific 
            statement of the location of the audience in terms of 
            its progression through an education or training context.</rdfs:comment>
        <rdfs:isDefinedBy rdf:resource="http://purl.org/dc/terms/"/>
        <rdfs:label xml:lang="en-us">Audience Education Level</rdfs:label>
    </owl:AnnotationProperty>
    


    <!-- http://purl.org/dc/terms/extent -->

    <owl:AnnotationProperty rdf:about="http://purl.org/dc/terms/extent">
        <dc:type rdf:resource="http://dublincore.org/usage/documents/principles/#element-refinement"/>
        <terms:hasVersion rdf:resource="http://dublincore.org/usage/terms/history/#extent-002"/>
        <terms:issued>2000-07-11</terms:issued>
        <terms:modified>2002-06-15</terms:modified>
        <rdfs:comment xml:lang="en-us">The size or duration of the resource.</rdfs:comment>
        <rdfs:isDefinedBy rdf:resource="http://purl.org/dc/terms/"/>
        <rdfs:label xml:lang="en-us">Extent</rdfs:label>
    </owl:AnnotationProperty>
    


    <!-- http://purl.org/dc/terms/hasFormat -->

    <owl:AnnotationProperty rdf:about="http://purl.org/dc/terms/hasFormat">
        <dc:type rdf:resource="http://dublincore.org/usage/documents/principles/#element-refinement"/>
        <terms:hasVersion rdf:resource="http://dublincore.org/usage/terms/history/#hasFormat-002"/>
        <terms:issued>2000-07-11</terms:issued>
        <terms:modified>2002-06-15</terms:modified>
        <rdfs:comment xml:lang="en-us">The described resource pre-existed the referenced resource, 
            which is essentially the same intellectual content presented 
            in another format.</rdfs:comment>
        <rdfs:isDefinedBy rdf:resource="http://purl.org/dc/terms/"/>
        <rdfs:label xml:lang="en-us">Has Format</rdfs:label>
    </owl:AnnotationProperty>
    


    <!-- http://purl.org/dc/terms/hasPart -->

    <owl:AnnotationProperty rdf:about="http://purl.org/dc/terms/hasPart">
        <dc:type rdf:resource="http://dublincore.org/usage/documents/principles/#element-refinement"/>
        <terms:hasVersion rdf:resource="http://dublincore.org/usage/terms/history/#hasPart-002"/>
        <terms:issued>2000-07-11</terms:issued>
        <terms:modified>2002-06-15</terms:modified>
        <rdfs:comment xml:lang="en-us">The described resource includes the referenced resource either 
            physically or logically.</rdfs:comment>
        <rdfs:isDefinedBy rdf:resource="http://purl.org/dc/terms/"/>
        <rdfs:label xml:lang="en-us">Has Part</rdfs:label>
    </owl:AnnotationProperty>
    


    <!-- http://purl.org/dc/terms/hasVersion -->

    <owl:AnnotationProperty rdf:about="http://purl.org/dc/terms/hasVersion">
        <dc:type rdf:resource="http://dublincore.org/usage/documents/principles/#element-refinement"/>
        <terms:hasVersion rdf:resource="http://dublincore.org/usage/terms/history/#hasVersion-002"/>
        <terms:issued>2000-07-11</terms:issued>
        <terms:modified>2002-06-15</terms:modified>
        <rdfs:comment xml:lang="en-us">The described resource has a version, edition, or adaptation, 
            namely, the referenced resource.</rdfs:comment>
        <rdfs:isDefinedBy rdf:resource="http://purl.org/dc/terms/"/>
        <rdfs:label xml:lang="en-us">Has Version</rdfs:label>
    </owl:AnnotationProperty>
    


    <!-- http://purl.org/dc/terms/isFormatOf -->

    <owl:AnnotationProperty rdf:about="http://purl.org/dc/terms/isFormatOf">
        <dc:type rdf:resource="http://dublincore.org/usage/documents/principles/#element-refinement"/>
        <terms:hasVersion rdf:resource="http://dublincore.org/usage/terms/history/#isFormatOf-002"/>
        <terms:issued>2000-07-11</terms:issued>
        <terms:modified>2002-06-15</terms:modified>
        <rdfs:comment xml:lang="en-us">The described resource is the same intellectual content of 
            the referenced resource, but presented in another format.</rdfs:comment>
        <rdfs:isDefinedBy rdf:resource="http://purl.org/dc/terms/"/>
        <rdfs:label xml:lang="en-us">Is Format Of</rdfs:label>
    </owl:AnnotationProperty>
    


    <!-- http://purl.org/dc/terms/isPartOf -->

    <owl:AnnotationProperty rdf:about="http://purl.org/dc/terms/isPartOf">
        <dc:type rdf:resource="http://dublincore.org/usage/documents/principles/#element-refinement"/>
        <terms:hasVersion rdf:resource="http://dublincore.org/usage/terms/history/#isPartOf-002"/>
        <terms:issued>2000-07-11</terms:issued>
        <terms:modified>2002-06-15</terms:modified>
        <rdfs:comment xml:lang="en-us">The described resource is a physical or logical part of the 
            referenced resource.</rdfs:comment>
        <rdfs:isDefinedBy rdf:resource="http://purl.org/dc/terms/"/>
        <rdfs:label xml:lang="en-us">Is Part Of</rdfs:label>
    </owl:AnnotationProperty>
    


    <!-- http://purl.org/dc/terms/isReferencedBy -->

    <owl:AnnotationProperty rdf:about="http://purl.org/dc/terms/isReferencedBy">
        <dc:type rdf:resource="http://dublincore.org/usage/documents/principles/#element-refinement"/>
        <terms:hasVersion rdf:resource="http://dublincore.org/usage/terms/history/#isReferencedBy-002"/>
        <terms:issued>2000-07-11</terms:issued>
        <terms:modified>2002-06-15</terms:modified>
        <rdfs:comment xml:lang="en-us">The described resource is referenced, cited, or otherwise 
            pointed to by the referenced resource.</rdfs:comment>
        <rdfs:isDefinedBy rdf:resource="http://purl.org/dc/terms/"/>
        <rdfs:label xml:lang="en-us">Is Referenced By</rdfs:label>
    </owl:AnnotationProperty>
    


    <!-- http://purl.org/dc/terms/isReplacedBy -->

    <owl:AnnotationProperty rdf:about="http://purl.org/dc/terms/isReplacedBy">
        <dc:type rdf:resource="http://dublincore.org/usage/documents/principles/#element-refinement"/>
        <terms:hasVersion rdf:resource="http://dublincore.org/usage/terms/history/#isReplacedBy-002"/>
        <terms:issued>2000-07-11</terms:issued>
        <terms:modified>2002-06-15</terms:modified>
        <rdfs:comment xml:lang="en-us">The described resource is supplanted, displaced, or 
            superseded by the referenced resource.</rdfs:comment>
        <rdfs:isDefinedBy rdf:resource="http://purl.org/dc/terms/"/>
        <rdfs:label xml:lang="en-us">Is Replaced By</rdfs:label>
    </owl:AnnotationProperty>
    


    <!-- http://purl.org/dc/terms/isRequiredBy -->

    <owl:AnnotationProperty rdf:about="http://purl.org/dc/terms/isRequiredBy">
        <dc:type rdf:resource="http://dublincore.org/usage/documents/principles/#element-refinement"/>
        <terms:hasVersion rdf:resource="http://dublincore.org/usage/terms/history/#isRequiredBy-002"/>
        <terms:issued>2000-07-11</terms:issued>
        <terms:modified>2002-06-15</terms:modified>
        <rdfs:comment xml:lang="en-us">The described resource is required by the referenced resource, 
            either physically or logically.</rdfs:comment>
        <rdfs:isDefinedBy rdf:resource="http://purl.org/dc/terms/"/>
        <rdfs:label xml:lang="en-us">Is Required By</rdfs:label>
    </owl:AnnotationProperty>
    


    <!-- http://purl.org/dc/terms/isVersionOf -->

    <owl:AnnotationProperty rdf:about="http://purl.org/dc/terms/isVersionOf">
        <dc:type rdf:resource="http://dublincore.org/usage/documents/principles/#element-refinement"/>
        <terms:hasVersion rdf:resource="http://dublincore.org/usage/terms/history/#isVersionOf-002"/>
        <terms:issued>2000-07-11</terms:issued>
        <terms:modified>2002-06-15</terms:modified>
        <rdfs:comment xml:lang="en-us">The described resource is a version, edition, or adaptation 
            of the referenced resource. Changes in version imply substantive 
            changes in content rather than differences in format.</rdfs:comment>
        <rdfs:isDefinedBy rdf:resource="http://purl.org/dc/terms/"/>
        <rdfs:label xml:lang="en-us">Is Version Of</rdfs:label>
    </owl:AnnotationProperty>
    


    <!-- http://purl.org/dc/terms/issued -->

    <owl:AnnotationProperty rdf:about="http://purl.org/dc/terms/issued">
        <dc:type rdf:resource="http://dublincore.org/usage/documents/principles/#element-refinement"/>
        <terms:hasVersion rdf:resource="http://dublincore.org/usage/terms/history/#issued-002"/>
        <terms:issued>2000-07-11</terms:issued>
        <terms:modified>2002-06-15</terms:modified>
        <rdfs:comment xml:lang="en-us">Date of formal issuance (e.g., publication) of the resource.</rdfs:comment>
        <rdfs:isDefinedBy rdf:resource="http://purl.org/dc/terms/"/>
        <rdfs:label xml:lang="en-us">Issued</rdfs:label>
    </owl:AnnotationProperty>
    


    <!-- http://purl.org/dc/terms/mediator -->

    <owl:AnnotationProperty rdf:about="http://purl.org/dc/terms/mediator">
        <dc:description xml:lang="en-us">The audiences for a resource are of two basic classes: (1) an 
            ultimate beneficiary of the resource, and (2) frequently, an 
            entity that mediates access to the resource.  The mediator 
            element refinement represents the second of these two classes.</dc:description>
        <dc:type rdf:resource="http://dublincore.org/usage/documents/principles/#element-refinement"/>
        <terms:hasVersion rdf:resource="http://dublincore.org/usage/terms/history/#mediator-002"/>
        <terms:issued>2001-05-21</terms:issued>
        <terms:modified>2002-07-13</terms:modified>
        <rdfs:comment xml:lang="en-us">A class of entity that mediates access to the
            resource and for whom the resource is intended or useful.</rdfs:comment>
        <rdfs:isDefinedBy rdf:resource="http://purl.org/dc/terms/"/>
        <rdfs:label xml:lang="en-us">Mediator</rdfs:label>
    </owl:AnnotationProperty>
    


    <!-- http://purl.org/dc/terms/medium -->

    <owl:AnnotationProperty rdf:about="http://purl.org/dc/terms/medium">
        <dc:type rdf:resource="http://dublincore.org/usage/documents/principles/#element-refinement"/>
        <terms:hasVersion rdf:resource="http://dublincore.org/usage/terms/history/#medium-002"/>
        <terms:issued>2000-07-11</terms:issued>
        <terms:modified>2002-06-15</terms:modified>
        <rdfs:comment xml:lang="en-us">The material or physical carrier of the resource.</rdfs:comment>
        <rdfs:isDefinedBy rdf:resource="http://purl.org/dc/terms/"/>
        <rdfs:label xml:lang="en-us">Medium</rdfs:label>
    </owl:AnnotationProperty>
    


    <!-- http://purl.org/dc/terms/modified -->

    <owl:AnnotationProperty rdf:about="http://purl.org/dc/terms/modified">
        <dc:type rdf:resource="http://dublincore.org/usage/documents/principles/#element-refinement"/>
        <terms:hasVersion rdf:resource="http://dublincore.org/usage/terms/history/#modified-002"/>
        <terms:issued>2000-07-11</terms:issued>
        <terms:modified>2002-06-15</terms:modified>
        <rdfs:comment xml:lang="en-us">Date on which the resource was changed.</rdfs:comment>
        <rdfs:isDefinedBy rdf:resource="http://purl.org/dc/terms/"/>
        <rdfs:label xml:lang="en-us">Modified</rdfs:label>
    </owl:AnnotationProperty>
    


    <!-- http://purl.org/dc/terms/publisher -->

    <rdf:Description rdf:about="http://purl.org/dc/terms/publisher">
        <rdfs:range rdf:resource="http://www.w3.org/2000/10/swap/pim/contact#Person"/>
        <rdfs:range rdf:resource="https://schema.org/Organization"/>
        <rdfs:domain rdf:resource="http://rdfs.org/ns/void#Dataset"/>
    </rdf:Description>
    


    <!-- http://purl.org/dc/terms/references -->

    <owl:AnnotationProperty rdf:about="http://purl.org/dc/terms/references">
        <dc:type rdf:resource="http://dublincore.org/usage/documents/principles/#element-refinement"/>
        <terms:hasVersion rdf:resource="http://dublincore.org/usage/terms/history/#references-002"/>
        <terms:issued>2000-07-11</terms:issued>
        <terms:modified>2002-06-15</terms:modified>
        <rdfs:comment xml:lang="en-us">The described resource references, cites, or otherwise points 
            to the referenced resource.</rdfs:comment>
        <rdfs:isDefinedBy rdf:resource="http://purl.org/dc/terms/"/>
        <rdfs:label xml:lang="en-us">References</rdfs:label>
    </owl:AnnotationProperty>
    


    <!-- http://purl.org/dc/terms/replaces -->

    <owl:AnnotationProperty rdf:about="http://purl.org/dc/terms/replaces">
        <dc:type rdf:resource="http://dublincore.org/usage/documents/principles/#element-refinement"/>
        <terms:hasVersion rdf:resource="http://dublincore.org/usage/terms/history/#replaces-002"/>
        <terms:issued>2000-07-11</terms:issued>
        <terms:modified>2002-06-15</terms:modified>
        <rdfs:comment xml:lang="en-us">The described resource supplants, displaces, or supersedes 
            the referenced resource.</rdfs:comment>
        <rdfs:isDefinedBy rdf:resource="http://purl.org/dc/terms/"/>
        <rdfs:label xml:lang="en-us">Replaces</rdfs:label>
    </owl:AnnotationProperty>
    


    <!-- http://purl.org/dc/terms/requires -->

    <owl:AnnotationProperty rdf:about="http://purl.org/dc/terms/requires">
        <dc:type rdf:resource="http://dublincore.org/usage/documents/principles/#element-refinement"/>
        <terms:hasVersion rdf:resource="http://dublincore.org/usage/terms/history/#requires-002"/>
        <terms:issued>2000-07-11</terms:issued>
        <terms:modified>2002-06-15</terms:modified>
        <rdfs:comment xml:lang="en-us">The described resource requires the referenced resource to 
            support its function, delivery, or coherence of content.</rdfs:comment>
        <rdfs:isDefinedBy rdf:resource="http://purl.org/dc/terms/"/>
        <rdfs:label xml:lang="en-us">Requires</rdfs:label>
    </owl:AnnotationProperty>
    


    <!-- http://purl.org/dc/terms/spatial -->

    <owl:AnnotationProperty rdf:about="http://purl.org/dc/terms/spatial">
        <dc:type rdf:resource="http://dublincore.org/usage/documents/principles/#element-refinement"/>
        <terms:hasVersion rdf:resource="http://dublincore.org/usage/terms/history/#spatial-002"/>
        <terms:issued>2000-07-11</terms:issued>
        <terms:modified>2002-06-15</terms:modified>
        <rdfs:comment xml:lang="en-us">Spatial characteristics of the intellectual content of the resoure.</rdfs:comment>
        <rdfs:isDefinedBy rdf:resource="http://purl.org/dc/terms/"/>
        <rdfs:label xml:lang="en-us">Spatial</rdfs:label>
    </owl:AnnotationProperty>
    


    <!-- http://purl.org/dc/terms/tableOfContents -->

    <owl:AnnotationProperty rdf:about="http://purl.org/dc/terms/tableOfContents">
        <dc:type rdf:resource="http://dublincore.org/usage/documents/principles/#element-refinement"/>
        <terms:hasVersion rdf:resource="http://dublincore.org/usage/terms/history/#tableOfContents-002"/>
        <terms:issued>2000-07-11</terms:issued>
        <terms:modified>2002-06-15</terms:modified>
        <rdfs:comment xml:lang="en-us">A list of subunits of the content of the resource.</rdfs:comment>
        <rdfs:isDefinedBy rdf:resource="http://purl.org/dc/terms/"/>
        <rdfs:label xml:lang="en-us">Table Of Contents</rdfs:label>
    </owl:AnnotationProperty>
    


    <!-- http://purl.org/dc/terms/temporal -->

    <owl:AnnotationProperty rdf:about="http://purl.org/dc/terms/temporal">
        <dc:type rdf:resource="http://dublincore.org/usage/documents/principles/#element-refinement"/>
        <terms:hasVersion rdf:resource="http://dublincore.org/usage/terms/history/#temporal-002"/>
        <terms:issued>2000-07-11</terms:issued>
        <terms:modified>2002-06-15</terms:modified>
        <rdfs:comment xml:lang="en-us">Temporal characteristics of the intellectual content of the resource.</rdfs:comment>
        <rdfs:isDefinedBy rdf:resource="http://purl.org/dc/terms/"/>
        <rdfs:label xml:lang="en-us">Temporal</rdfs:label>
    </owl:AnnotationProperty>
    


    <!-- http://purl.org/dc/terms/valid -->

    <owl:AnnotationProperty rdf:about="http://purl.org/dc/terms/valid">
        <dc:type rdf:resource="http://dublincore.org/usage/documents/principles/#element-refinement"/>
        <terms:hasVersion rdf:resource="http://dublincore.org/usage/terms/history/#valid-002"/>
        <terms:issued>2000-07-11</terms:issued>
        <terms:modified>2002-06-15</terms:modified>
        <rdfs:comment xml:lang="en-us">Date (often a range) of validity of a resource.</rdfs:comment>
        <rdfs:isDefinedBy rdf:resource="http://purl.org/dc/terms/"/>
        <rdfs:label xml:lang="en-us">Valid</rdfs:label>
    </owl:AnnotationProperty>
    


    <!-- http://rdfs.org/ns/void#uriRegexPattern -->

    <rdf:Description rdf:about="http://rdfs.org/ns/void#uriRegexPattern">
        <rdfs:domain rdf:resource="http://rdfs.org/ns/void#Dataset"/>
    </rdf:Description>
    


    <!-- http://swrl.stanford.edu/ontologies/3.3/swrla.owl#isRuleEnabled -->

    <owl:AnnotationProperty rdf:about="http://swrl.stanford.edu/ontologies/3.3/swrla.owl#isRuleEnabled"/>
    


    <!-- http://www.w3.org/2000/01/rdf-schema#comment -->

    <owl:AnnotationProperty rdf:about="http://www.w3.org/2000/01/rdf-schema#comment">
        <rdfs:comment xml:lang="en"></rdfs:comment>
        <rdfs:isDefinedBy rdf:resource="http://www.w3.org/ns/prov-o#"/>
    </owl:AnnotationProperty>
    


    <!-- http://www.w3.org/2000/01/rdf-schema#isDefinedBy -->

    <owl:AnnotationProperty rdf:about="http://www.w3.org/2000/01/rdf-schema#isDefinedBy"/>
    


    <!-- http://www.w3.org/2000/01/rdf-schema#label -->

    <owl:AnnotationProperty rdf:about="http://www.w3.org/2000/01/rdf-schema#label">
        <rdfs:comment xml:lang="en"></rdfs:comment>
        <rdfs:isDefinedBy rdf:resource="http://www.w3.org/ns/prov-o#"/>
    </owl:AnnotationProperty>
    


    <!-- http://www.w3.org/2000/01/rdf-schema#seeAlso -->

    <owl:AnnotationProperty rdf:about="http://www.w3.org/2000/01/rdf-schema#seeAlso">
        <rdfs:comment xml:lang="en"></rdfs:comment>
    </owl:AnnotationProperty>
    


    <!-- http://www.w3.org/2002/07/owl#maxCardinality -->

    <owl:AnnotationProperty rdf:about="http://www.w3.org/2002/07/owl#maxCardinality"/>
    


    <!-- http://www.w3.org/2002/07/owl#versionInfo -->

    <owl:AnnotationProperty rdf:about="http://www.w3.org/2002/07/owl#versionInfo"/>
    


    <!-- http://www.w3.org/2003/06/sw-vocab-status/ns#term_status -->

    <owl:AnnotationProperty rdf:about="http://www.w3.org/2003/06/sw-vocab-status/ns#term_status"/>
    


    <!-- http://www.w3.org/ns/oa#cachedSource -->

    <rdf:Description rdf:about="http://www.w3.org/ns/oa#cachedSource">
        <rdfs:comment>A object of the relationship is a copy of the Source resource&apos;s representation, appropriate for the Annotation.</rdfs:comment>
        <rdfs:isDefinedBy rdf:resource="http://www.w3.org/ns/oa#"/>
        <rdfs:label>cachedSource</rdfs:label>
        <rdfs:domain rdf:resource="http://www.w3.org/ns/oa#TimeState"/>
    </rdf:Description>
    


    <!-- http://www.w3.org/ns/oa#hasBody -->

    <rdf:Description rdf:about="http://www.w3.org/ns/oa#hasBody">
        <rdfs:comment>The object of the relationship is a resource that is a body of the Annotation.</rdfs:comment>
        <rdfs:isDefinedBy rdf:resource="http://www.w3.org/ns/oa#"/>
        <rdfs:label>hasBody</rdfs:label>
        <rdfs:domain rdf:resource="http://www.w3.org/ns/oa#Annotation"/>
    </rdf:Description>
    


    <!-- http://www.w3.org/ns/oa#hasScope -->

    <rdf:Description rdf:about="http://www.w3.org/ns/oa#hasScope">
        <rdfs:comment>The scope or context in which the resource is used within the Annotation.</rdfs:comment>
        <rdfs:isDefinedBy rdf:resource="http://www.w3.org/ns/oa#"/>
        <rdfs:label>hasScope</rdfs:label>
        <rdfs:domain rdf:resource="http://www.w3.org/ns/oa#SpecificResource"/>
    </rdf:Description>
    


    <!-- http://www.w3.org/ns/oa#hasSource -->

    <rdf:Description rdf:about="http://www.w3.org/ns/oa#hasSource">
        <rdfs:comment>The resource that the ResourceSelection, or its subclass SpecificResource, is refined from, or more specific than. Please note that the domain ( oa:ResourceSelection ) is not used directly in the Web Annotation model.</rdfs:comment>
        <rdfs:isDefinedBy rdf:resource="http://www.w3.org/ns/oa#"/>
        <rdfs:label>hasSource</rdfs:label>
        <rdfs:domain rdf:resource="http://www.w3.org/ns/oa#ResourceSelection"/>
    </rdf:Description>
    


    <!-- http://www.w3.org/ns/oa#hasTarget -->

    <rdf:Description rdf:about="http://www.w3.org/ns/oa#hasTarget">
        <rdfs:comment>The relationship between an Annotation and its Target.</rdfs:comment>
        <rdfs:isDefinedBy rdf:resource="http://www.w3.org/ns/oa#"/>
        <rdfs:label>hasTarget</rdfs:label>
        <rdfs:domain rdf:resource="http://www.w3.org/ns/oa#Annotation"/>
    </rdf:Description>
    


    <!-- http://www.w3.org/ns/oa#renderedVia -->

    <rdf:Description rdf:about="http://www.w3.org/ns/oa#renderedVia">
        <rdfs:comment>A system that was used by the application that created the Annotation to render the resource.</rdfs:comment>
        <rdfs:isDefinedBy rdf:resource="http://www.w3.org/ns/oa#"/>
        <rdfs:label>renderedVia</rdfs:label>
        <rdfs:domain rdf:resource="http://www.w3.org/ns/oa#SpecificResource"/>
    </rdf:Description>
    


    <!-- http://www.w3.org/ns/prov#aq -->

    <owl:AnnotationProperty rdf:about="http://www.w3.org/ns/prov#aq">
        <rdfs:isDefinedBy rdf:resource="http://www.w3.org/ns/prov-o#"/>
        <rdfs:subPropertyOf rdf:resource="http://www.w3.org/2000/01/rdf-schema#seeAlso"/>
    </owl:AnnotationProperty>
    


    <!-- http://www.w3.org/ns/prov#category -->

    <owl:AnnotationProperty rdf:about="http://www.w3.org/ns/prov#category">
        <rdfs:comment xml:lang="en">Classify prov-o terms into three categories, including &apos;starting-point&apos;, &apos;qualifed&apos;, and &apos;extended&apos;. This classification is used by the prov-o html document to gently introduce prov-o terms to its users. </rdfs:comment>
        <rdfs:isDefinedBy rdf:resource="http://www.w3.org/ns/prov-o#"/>
    </owl:AnnotationProperty>
    


    <!-- http://www.w3.org/ns/prov#component -->

    <owl:AnnotationProperty rdf:about="http://www.w3.org/ns/prov#component">
        <rdfs:comment xml:lang="en">Classify prov-o terms into six components according to prov-dm, including &apos;agents-responsibility&apos;, &apos;alternate&apos;, &apos;annotations&apos;, &apos;collections&apos;, &apos;derivations&apos;, and &apos;entities-activities&apos;. This classification is used so that readers of prov-o specification can find its correspondence with the prov-dm specification.</rdfs:comment>
        <rdfs:isDefinedBy rdf:resource="http://www.w3.org/ns/prov-o#"/>
    </owl:AnnotationProperty>
    


    <!-- http://www.w3.org/ns/prov#constraints -->

    <owl:AnnotationProperty rdf:about="http://www.w3.org/ns/prov#constraints">
        <rdfs:comment xml:lang="en">A reference to the principal section of the PROV-CONSTRAINTS document that describes this concept.</rdfs:comment>
        <rdfs:isDefinedBy rdf:resource="http://www.w3.org/ns/prov-o#"/>
        <rdfs:subPropertyOf rdf:resource="http://www.w3.org/2000/01/rdf-schema#seeAlso"/>
    </owl:AnnotationProperty>
    


    <!-- http://www.w3.org/ns/prov#definition -->

    <owl:AnnotationProperty rdf:about="http://www.w3.org/ns/prov#definition">
        <rdfs:comment xml:lang="en">A definition quoted from PROV-DM or PROV-CONSTRAINTS that describes the concept expressed with this OWL term.</rdfs:comment>
        <rdfs:isDefinedBy rdf:resource="http://www.w3.org/ns/prov-o#"/>
    </owl:AnnotationProperty>
    


    <!-- http://www.w3.org/ns/prov#dm -->

    <owl:AnnotationProperty rdf:about="http://www.w3.org/ns/prov#dm">
        <rdfs:comment xml:lang="en">A reference to the principal section of the PROV-DM document that describes this concept.</rdfs:comment>
        <rdfs:isDefinedBy rdf:resource="http://www.w3.org/ns/prov-o#"/>
        <rdfs:subPropertyOf rdf:resource="http://www.w3.org/2000/01/rdf-schema#seeAlso"/>
    </owl:AnnotationProperty>
    


    <!-- http://www.w3.org/ns/prov#editorialNote -->

    <owl:AnnotationProperty rdf:about="http://www.w3.org/ns/prov#editorialNote">
        <rdfs:comment xml:lang="en">A note by the OWL development team about how this term expresses the PROV-DM concept, or how it should be used in context of semantic web or linked data.</rdfs:comment>
        <rdfs:isDefinedBy rdf:resource="http://www.w3.org/ns/prov-o#"/>
    </owl:AnnotationProperty>
    


    <!-- http://www.w3.org/ns/prov#editorsDefinition -->

    <owl:AnnotationProperty rdf:about="http://www.w3.org/ns/prov#editorsDefinition">
        <rdfs:comment xml:lang="en">When the prov-o term does not have a definition drawn from prov-dm, and the prov-o editor provides one.</rdfs:comment>
        <rdfs:isDefinedBy rdf:resource="http://www.w3.org/ns/prov-o#"/>
        <rdfs:subPropertyOf rdf:resource="http://www.w3.org/ns/prov#definition"/>
    </owl:AnnotationProperty>
    


    <!-- http://www.w3.org/ns/prov#inverse -->

    <owl:AnnotationProperty rdf:about="http://www.w3.org/ns/prov#inverse">
        <rdfs:comment xml:lang="en">PROV-O does not define all property inverses. The directionalities defined in PROV-O should be given preference over those not defined. However, if users wish to name the inverse of a PROV-O property, the local name given by prov:inverse should be used.</rdfs:comment>
        <rdfs:isDefinedBy rdf:resource="http://www.w3.org/ns/prov-o#"/>
        <rdfs:seeAlso rdf:resource="http://www.w3.org/TR/prov-o/#names-of-inverse-properties"/>
    </owl:AnnotationProperty>
    


    <!-- http://www.w3.org/ns/prov#n -->

    <owl:AnnotationProperty rdf:about="http://www.w3.org/ns/prov#n">
        <rdfs:comment xml:lang="en">A reference to the principal section of the PROV-DM document that describes this concept.</rdfs:comment>
        <rdfs:isDefinedBy rdf:resource="http://www.w3.org/ns/prov-o#"/>
        <rdfs:subPropertyOf rdf:resource="http://www.w3.org/2000/01/rdf-schema#seeAlso"/>
    </owl:AnnotationProperty>
    


    <!-- http://www.w3.org/ns/prov#order -->

    <owl:AnnotationProperty rdf:about="http://www.w3.org/ns/prov#order">
        <rdfs:comment xml:lang="en">The position that this OWL term should be listed within documentation. The scope of the documentation (e.g., among all terms, among terms within a prov:category, among properties applying to a particular class, etc.) is unspecified.</rdfs:comment>
        <rdfs:isDefinedBy rdf:resource="http://www.w3.org/ns/prov-o#"/>
    </owl:AnnotationProperty>
    


    <!-- http://www.w3.org/ns/prov#qualifiedForm -->

    <owl:AnnotationProperty rdf:about="http://www.w3.org/ns/prov#qualifiedForm">
        <rdfs:comment xml:lang="en">This annotation property links a subproperty of prov:wasInfluencedBy with the subclass of prov:Influence and the qualifying property that are used to qualify it. 

Example annotation:

    prov:wasGeneratedBy prov:qualifiedForm prov:qualifiedGeneration, prov:Generation .

Then this unqualified assertion:

    :entity1 prov:wasGeneratedBy :activity1 .

can be qualified by adding:

   :entity1 prov:qualifiedGeneration :entity1Gen .
   :entity1Gen 
       a prov:Generation, prov:Influence;
       prov:activity :activity1;
       :customValue 1337 .

Note how the value of the unqualified influence (prov:wasGeneratedBy :activity1) is mirrored as the value of the prov:activity (or prov:entity, or prov:agent) property on the influence class.</rdfs:comment>
        <rdfs:isDefinedBy rdf:resource="http://www.w3.org/ns/prov-o#"/>
        <rdfs:subPropertyOf rdf:resource="http://www.w3.org/2000/01/rdf-schema#seeAlso"/>
    </owl:AnnotationProperty>
    


    <!-- http://www.w3.org/ns/prov#sharesDefinitionWith -->

    <owl:AnnotationProperty rdf:about="http://www.w3.org/ns/prov#sharesDefinitionWith">
        <rdfs:isDefinedBy rdf:resource="http://www.w3.org/ns/prov-o#"/>
        <rdfs:subPropertyOf rdf:resource="http://www.w3.org/2000/01/rdf-schema#seeAlso"/>
    </owl:AnnotationProperty>
    


    <!-- http://www.w3.org/ns/prov#specializationOf -->

    <owl:AnnotationProperty rdf:about="http://www.w3.org/ns/prov#specializationOf">
        <rdfs:range rdf:resource="http://www.w3.org/ns/prov#Entity"/>
    </owl:AnnotationProperty>
    


    <!-- http://www.w3.org/ns/prov#todo -->

    <owl:AnnotationProperty rdf:about="http://www.w3.org/ns/prov#todo"/>
    


    <!-- http://www.w3.org/ns/prov#unqualifiedForm -->

    <owl:AnnotationProperty rdf:about="http://www.w3.org/ns/prov#unqualifiedForm">
        <rdfs:comment xml:lang="en">Classes and properties used to qualify relationships are annotated with prov:unqualifiedForm to indicate the property used to assert an unqualified provenance relation.</rdfs:comment>
        <rdfs:isDefinedBy rdf:resource="http://www.w3.org/ns/prov-o#"/>
        <rdfs:subPropertyOf rdf:resource="http://www.w3.org/2000/01/rdf-schema#seeAlso"/>
    </owl:AnnotationProperty>
    


    <!-- http://www.w3.org/ns/prov#wasRevisionOf -->

    <owl:AnnotationProperty rdf:about="http://www.w3.org/ns/prov#wasRevisionOf">
        <rdfs:range rdf:resource="http://www.w3.org/ns/prov#Entity"/>
    </owl:AnnotationProperty>
    


    <!-- http://xmlns.com/foaf/0.1/membershipClass -->

    <owl:AnnotationProperty rdf:about="http://xmlns.com/foaf/0.1/membershipClass">
        <rdfs:comment>Indicates the class of individuals that are a member of a Group</rdfs:comment>
        <rdfs:isDefinedBy rdf:resource="http://xmlns.com/foaf/0.1/"/>
        <rdfs:label>membershipClass</rdfs:label>
        <ns:term_status>unstable</ns:term_status>
    </owl:AnnotationProperty>
    


    <!-- http://xmlns.com/foaf/0.1/name -->

    <owl:AnnotationProperty rdf:about="http://xmlns.com/foaf/0.1/name">
        <rdfs:subPropertyOf rdf:resource="http://www.w3.org/2000/01/rdf-schema#label"/>
        <rdfs:range rdf:resource="http://www.w3.org/2000/01/rdf-schema#Literal"/>
    </owl:AnnotationProperty>
    


    <!-- http://xmlns.com/wot/0.1/assurance -->

    <owl:AnnotationProperty rdf:about="http://xmlns.com/wot/0.1/assurance"/>
    


    <!-- http://xmlns.com/wot/0.1/src_assurance -->

    <owl:AnnotationProperty rdf:about="http://xmlns.com/wot/0.1/src_assurance"/>
    


    <!-- 
    ///////////////////////////////////////////////////////////////////////////////////////
    //
    // Object Properties
    //
    ///////////////////////////////////////////////////////////////////////////////////////
     -->

    


    <!-- http://rdfs.org/ns/void#class -->

    <rdf:Description rdf:about="http://rdfs.org/ns/void#class">
        <rdf:type rdf:resource="http://www.w3.org/2002/07/owl#FunctionalProperty"/>
        <rdfs:domain rdf:resource="http://rdfs.org/ns/void#Dataset"/>
        <rdfs:range rdf:resource="http://www.w3.org/2000/01/rdf-schema#Class"/>
        <rdfs:comment>The rdfs:Class that is the rdf:type of all entities in a class-based partition.</rdfs:comment>
        <rdfs:label>class</rdfs:label>
    </rdf:Description>
    


    <!-- http://rdfs.org/ns/void#classPartition -->

    <owl:ObjectProperty rdf:about="http://rdfs.org/ns/void#classPartition">
        <rdfs:subPropertyOf rdf:resource="http://rdfs.org/ns/void#subset"/>
        <rdfs:domain rdf:resource="http://rdfs.org/ns/void#Dataset"/>
        <rdfs:range rdf:resource="http://rdfs.org/ns/void#Dataset"/>
        <rdfs:comment>A subset of a void:Dataset that contains only the entities of a certain rdfs:Class.</rdfs:comment>
        <rdfs:label>class partition</rdfs:label>
    </owl:ObjectProperty>
    


    <!-- http://rdfs.org/ns/void#dataDump -->

    <owl:ObjectProperty rdf:about="http://rdfs.org/ns/void#dataDump">
        <rdfs:domain rdf:resource="http://rdfs.org/ns/void#Dataset"/>
        <rdfs:range rdf:resource="http://www.w3.org/2000/01/rdf-schema#Resource"/>
        <rdfs:comment>An RDF dump, partial or complete, of a void:Dataset.</rdfs:comment>
        <rdfs:label>Data Dump</rdfs:label>
    </owl:ObjectProperty>
    


    <!-- http://rdfs.org/ns/void#exampleResource -->

    <owl:ObjectProperty rdf:about="http://rdfs.org/ns/void#exampleResource">
        <rdfs:domain rdf:resource="http://rdfs.org/ns/void#Dataset"/>
        <rdfs:range rdf:resource="http://www.w3.org/2000/01/rdf-schema#Resource"/>
        <rdfs:label>example resource of dataset</rdfs:label>
    </owl:ObjectProperty>
    


    <!-- http://rdfs.org/ns/void#feature -->

    <owl:ObjectProperty rdf:about="http://rdfs.org/ns/void#feature">
        <rdfs:domain rdf:resource="http://rdfs.org/ns/void#Dataset"/>
        <rdfs:range rdf:resource="http://rdfs.org/ns/void#TechnicalFeature"/>
        <rdfs:label>feature</rdfs:label>
    </owl:ObjectProperty>
    


    <!-- http://rdfs.org/ns/void#inDataset -->

    <owl:ObjectProperty rdf:about="http://rdfs.org/ns/void#inDataset">
        <rdfs:domain rdf:resource="http://xmlns.com/foaf/0.1/Document"/>
        <rdfs:range rdf:resource="http://rdfs.org/ns/void#Dataset"/>
        <rdfs:comment>Points to the void:Dataset that a document is a part of.</rdfs:comment>
        <rdfs:label>in dataset</rdfs:label>
    </owl:ObjectProperty>
    


    <!-- http://rdfs.org/ns/void#linkPredicate -->

    <owl:ObjectProperty rdf:about="http://rdfs.org/ns/void#linkPredicate">
        <rdfs:domain rdf:resource="http://rdfs.org/ns/void#Linkset"/>
        <rdfs:range rdf:resource="http://www.w3.org/1999/02/22-rdf-syntax-ns#Property"/>
        <rdfs:label>a link predicate</rdfs:label>
    </owl:ObjectProperty>
    


    <!-- http://rdfs.org/ns/void#objectsTarget -->

    <rdf:Description rdf:about="http://rdfs.org/ns/void#objectsTarget">
        <rdfs:subPropertyOf rdf:resource="http://rdfs.org/ns/void#target"/>
        <rdf:type rdf:resource="http://www.w3.org/2002/07/owl#FunctionalProperty"/>
        <rdfs:domain rdf:resource="http://rdfs.org/ns/void#Linkset"/>
        <rdfs:range rdf:resource="http://rdfs.org/ns/void#Dataset"/>
        <rdfs:comment>The dataset describing the objects of the triples contained in the Linkset.</rdfs:comment>
        <rdfs:label>Objects Target</rdfs:label>
    </rdf:Description>
    


    <!-- http://rdfs.org/ns/void#openSearchDescription -->

    <owl:ObjectProperty rdf:about="http://rdfs.org/ns/void#openSearchDescription">
        <rdfs:domain rdf:resource="http://rdfs.org/ns/void#Dataset"/>
        <rdfs:range rdf:resource="http://xmlns.com/foaf/0.1/Document"/>
        <rdfs:comment>An OpenSearch description document for a free-text search service over a void:Dataset.</rdfs:comment>
        <rdfs:label>open search description</rdfs:label>
    </owl:ObjectProperty>
    


    <!-- http://rdfs.org/ns/void#property -->

    <rdf:Description rdf:about="http://rdfs.org/ns/void#property">
        <rdf:type rdf:resource="http://www.w3.org/2002/07/owl#FunctionalProperty"/>
        <rdfs:domain rdf:resource="http://rdfs.org/ns/void#Dataset"/>
        <rdfs:range rdf:resource="http://www.w3.org/1999/02/22-rdf-syntax-ns#Property"/>
        <rdfs:comment>The rdf:Property that is the predicate of all triples in a property-based partition.</rdfs:comment>
        <rdfs:label>property</rdfs:label>
    </rdf:Description>
    


    <!-- http://rdfs.org/ns/void#propertyPartition -->

    <owl:ObjectProperty rdf:about="http://rdfs.org/ns/void#propertyPartition">
        <rdfs:subPropertyOf rdf:resource="http://rdfs.org/ns/void#subset"/>
        <rdfs:domain rdf:resource="http://rdfs.org/ns/void#Dataset"/>
        <rdfs:range rdf:resource="http://rdfs.org/ns/void#Dataset"/>
        <rdfs:comment>A subset of a void:Dataset that contains only the triples of a certain rdf:Property.</rdfs:comment>
        <rdfs:label>property partition</rdfs:label>
    </owl:ObjectProperty>
    


    <!-- http://rdfs.org/ns/void#rootResource -->

    <owl:ObjectProperty rdf:about="http://rdfs.org/ns/void#rootResource">
        <rdfs:domain rdf:resource="http://rdfs.org/ns/void#Dataset"/>
        <rdfs:comment>A top concept or entry point for a void:Dataset that is structured in a tree-like fashion. All resources in a dataset can be reached by following links from its root resources in a small number of steps.</rdfs:comment>
        <rdfs:label>root resource</rdfs:label>
    </owl:ObjectProperty>
    


    <!-- http://rdfs.org/ns/void#sparqlEndpoint -->

    <owl:ObjectProperty rdf:about="http://rdfs.org/ns/void#sparqlEndpoint">
        <rdfs:domain rdf:resource="http://rdfs.org/ns/void#Dataset"/>
        <rdfs:label>has a SPARQL endpoint at</rdfs:label>
    </owl:ObjectProperty>
    


    <!-- http://rdfs.org/ns/void#subjectsTarget -->

    <rdf:Description rdf:about="http://rdfs.org/ns/void#subjectsTarget">
        <rdfs:subPropertyOf rdf:resource="http://rdfs.org/ns/void#target"/>
        <rdf:type rdf:resource="http://www.w3.org/2002/07/owl#FunctionalProperty"/>
        <rdfs:domain rdf:resource="http://rdfs.org/ns/void#Linkset"/>
        <rdfs:range rdf:resource="http://rdfs.org/ns/void#Dataset"/>
        <rdfs:comment>The dataset describing the subjects of triples contained in the Linkset.</rdfs:comment>
        <rdfs:label>Subjects Target</rdfs:label>
    </rdf:Description>
    


    <!-- http://rdfs.org/ns/void#subset -->

    <owl:ObjectProperty rdf:about="http://rdfs.org/ns/void#subset">
        <rdfs:domain rdf:resource="http://rdfs.org/ns/void#Dataset"/>
        <rdfs:range rdf:resource="http://rdfs.org/ns/void#Dataset"/>
        <rdfs:label>has subset</rdfs:label>
    </owl:ObjectProperty>
    


    <!-- http://rdfs.org/ns/void#target -->

    <owl:ObjectProperty rdf:about="http://rdfs.org/ns/void#target">
        <rdfs:domain rdf:resource="http://rdfs.org/ns/void#Linkset"/>
        <rdfs:range rdf:resource="http://rdfs.org/ns/void#Dataset"/>
        <rdfs:comment>One of the two datasets linked by the Linkset.</rdfs:comment>
        <rdfs:label>Target</rdfs:label>
    </owl:ObjectProperty>
    


    <!-- http://rdfs.org/ns/void#uriLookupEndpoint -->

    <owl:ObjectProperty rdf:about="http://rdfs.org/ns/void#uriLookupEndpoint">
        <rdfs:domain rdf:resource="http://rdfs.org/ns/void#Dataset"/>
        <rdfs:comment>Defines a simple URI look-up protocol for accessing a dataset.</rdfs:comment>
        <rdfs:label>has an URI look-up endpoint at</rdfs:label>
    </owl:ObjectProperty>
    


    <!-- http://rdfs.org/ns/void#vocabulary -->

    <owl:ObjectProperty rdf:about="http://rdfs.org/ns/void#vocabulary">
        <rdfs:domain rdf:resource="http://rdfs.org/ns/void#Dataset"/>
        <rdfs:comment>A vocabulary that is used in the dataset.</rdfs:comment>
        <rdfs:label>vocabulary</rdfs:label>
    </owl:ObjectProperty>
    


    <!-- http://trdf.sourceforge.net/trustvocab#truster -->

    <owl:ObjectProperty rdf:about="http://trdf.sourceforge.net/trustvocab#truster">
        <rdfs:domain rdf:resource="http://trdf.sourceforge.net/trustvocab#TrustValue"/>
        <rdfs:comment xml:lang="en">This property specifies the information consumer for whom the trust value holds. We did not specify a range; ; thus giving applications a choice. However, we propose to represent information consumers as instances of foaf:Agent.</rdfs:comment>
    </owl:ObjectProperty>
    


    <!-- http://trdf.sourceforge.net/trustvocab#trustworthiness -->

    <owl:ObjectProperty rdf:about="http://trdf.sourceforge.net/trustvocab#trustworthiness">
        <rdfs:domain rdf:resource="http://rdfs.org/ns/void#Dataset"/>
        <rdfs:domain rdf:resource="https://schema.org/Organization"/>
        <rdfs:domain rdf:resource="https://schema.org/Person"/>
        <rdfs:range rdf:resource="http://trdf.sourceforge.net/trustvocab#TrustValue"/>
        <rdfs:comment xml:lang="en">This property associates an RDF statement (i.e. a reified triple) with a trust value. Thus, the intended domain of this property is rdf:Statement. However, to permit the application of this vocabulary to other use cases we do not explicitly prescribe the domain of this property. For instance, it is possible to use this property as the property of a named graph.</rdfs:comment>
    </owl:ObjectProperty>
    


    <!-- http://www.semanticweb.org/k_mil/ontologies/2021/8/EvalLOD#belongsTo -->

    <owl:ObjectProperty rdf:about="http://www.semanticweb.org/k_mil/ontologies/2021/8/EvalLOD#belongsTo">
        <owl:inverseOf rdf:resource="http://www.semanticweb.org/k_mil/ontologies/2021/8/EvalLOD#contains"/>
        <rdfs:domain rdf:resource="https://schema.org/Person"/>
        <rdfs:range rdf:resource="http://www.semanticweb.org/k_mil/ontologies/2021/8/EvalLOD#BlackList"/>
        <rdfs:range rdf:resource="http://www.semanticweb.org/k_mil/ontologies/2021/8/EvalLOD#WhiteList"/>
    </owl:ObjectProperty>
    


    <!-- http://www.semanticweb.org/k_mil/ontologies/2021/8/EvalLOD#contains -->

    <owl:ObjectProperty rdf:about="http://www.semanticweb.org/k_mil/ontologies/2021/8/EvalLOD#contains">
        <rdfs:domain rdf:resource="http://www.semanticweb.org/k_mil/ontologies/2021/8/EvalLOD#BlackList"/>
        <rdfs:domain rdf:resource="http://www.semanticweb.org/k_mil/ontologies/2021/8/EvalLOD#WhiteList"/>
        <rdfs:range rdf:resource="https://schema.org/Person"/>
    </owl:ObjectProperty>
    


    <!-- http://www.semanticweb.org/k_mil/ontologies/2021/8/EvalLOD#isVerifiable -->

    <owl:ObjectProperty rdf:about="http://www.semanticweb.org/k_mil/ontologies/2021/8/EvalLOD#isVerifiable">
        <rdfs:domain rdf:resource="http://rdfs.org/ns/void#Dataset"/>
    </owl:ObjectProperty>
    


    <!-- http://www.semanticweb.org/k_mil/ontologies/2021/8/EvalLOD#publishedBy -->

    <owl:ObjectProperty rdf:about="http://www.semanticweb.org/k_mil/ontologies/2021/8/EvalLOD#publishedBy">
        <owl:inverseOf rdf:resource="http://xmlns.com/foaf/0.1/publications"/>
        <rdfs:domain rdf:resource="http://rdfs.org/ns/void#Dataset"/>
        <rdfs:range rdf:resource="https://schema.org/Organization"/>
        <rdfs:range rdf:resource="https://schema.org/Person"/>
    </owl:ObjectProperty>
    


    <!-- http://www.w3.org/ns/oa#hasEndSelector -->

    <rdf:Description rdf:about="http://www.w3.org/ns/oa#hasEndSelector">
        <rdfs:domain rdf:resource="http://www.w3.org/ns/oa#RangeSelector"/>
        <rdfs:range rdf:resource="http://www.w3.org/ns/oa#Selector"/>
        <rdfs:comment>The relationship between a RangeSelector and the Selector that describes the end position of the range. </rdfs:comment>
        <rdfs:isDefinedBy rdf:resource="http://www.w3.org/ns/oa#"/>
        <rdfs:label>hasEndSelector</rdfs:label>
    </rdf:Description>
    


    <!-- http://www.w3.org/ns/oa#hasPurpose -->

    <rdf:Description rdf:about="http://www.w3.org/ns/oa#hasPurpose">
        <rdfs:range rdf:resource="http://www.w3.org/ns/oa#Motivation"/>
        <rdfs:comment>The purpose served by the resource in the Annotation.</rdfs:comment>
        <rdfs:isDefinedBy rdf:resource="http://www.w3.org/ns/oa#"/>
        <rdfs:label>hasPurpose</rdfs:label>
    </rdf:Description>
    


    <!-- http://www.w3.org/ns/oa#hasSelector -->

    <rdf:Description rdf:about="http://www.w3.org/ns/oa#hasSelector">
        <rdfs:domain rdf:resource="http://www.w3.org/ns/oa#ResourceSelection"/>
        <rdfs:range rdf:resource="http://www.w3.org/ns/oa#Selector"/>
        <rdfs:comment>The object of the relationship is a Selector that describes the segment or region of interest within the source resource.  Please note that the domain ( oa:ResourceSelection ) is not used directly in the Web Annotation model.</rdfs:comment>
        <rdfs:isDefinedBy rdf:resource="http://www.w3.org/ns/oa#"/>
        <rdfs:label>hasSelector</rdfs:label>
    </rdf:Description>
    


    <!-- http://www.w3.org/ns/oa#hasStartSelector -->

    <rdf:Description rdf:about="http://www.w3.org/ns/oa#hasStartSelector">
        <rdfs:domain rdf:resource="http://www.w3.org/ns/oa#RangeSelector"/>
        <rdfs:range rdf:resource="http://www.w3.org/ns/oa#Selector"/>
        <rdfs:comment>The relationship between a RangeSelector and the Selector that describes the start position of the range. </rdfs:comment>
        <rdfs:isDefinedBy rdf:resource="http://www.w3.org/ns/oa#"/>
        <rdfs:label>hasStartSelector</rdfs:label>
    </rdf:Description>
    


    <!-- http://www.w3.org/ns/oa#hasState -->

    <rdf:Description rdf:about="http://www.w3.org/ns/oa#hasState">
        <rdfs:domain rdf:resource="http://www.w3.org/ns/oa#ResourceSelection"/>
        <rdfs:range rdf:resource="http://www.w3.org/ns/oa#State"/>
        <rdfs:comment>The relationship between the ResourceSelection, or its subclass SpecificResource, and a State resource. Please note that the domain ( oa:ResourceSelection ) is not used directly in the Web Annotation model.</rdfs:comment>
        <rdfs:isDefinedBy rdf:resource="http://www.w3.org/ns/oa#"/>
        <rdfs:label>hasState</rdfs:label>
    </rdf:Description>
    


    <!-- http://www.w3.org/ns/oa#motivatedBy -->

    <rdf:Description rdf:about="http://www.w3.org/ns/oa#motivatedBy">
        <rdfs:domain rdf:resource="http://www.w3.org/ns/oa#Annotation"/>
        <rdfs:range rdf:resource="http://www.w3.org/ns/oa#Motivation"/>
        <rdfs:comment>The relationship between an Annotation and a Motivation that describes the reason for the Annotation&apos;s creation.</rdfs:comment>
        <rdfs:isDefinedBy rdf:resource="http://www.w3.org/ns/oa#"/>
        <rdfs:label>motivatedBy</rdfs:label>
    </rdf:Description>
    


    <!-- http://www.w3.org/ns/oa#styledBy -->

    <rdf:Description rdf:about="http://www.w3.org/ns/oa#styledBy">
        <rdfs:domain rdf:resource="http://www.w3.org/ns/oa#Annotation"/>
        <rdfs:range rdf:resource="http://www.w3.org/ns/oa#Style"/>
        <rdfs:comment>A reference to a Stylesheet that should be used to apply styles to the Annotation rendering.</rdfs:comment>
        <rdfs:isDefinedBy rdf:resource="http://www.w3.org/ns/oa#"/>
        <rdfs:label>styledBy</rdfs:label>
    </rdf:Description>
    


    <!-- http://www.w3.org/ns/oa#textDirection -->

    <rdf:Description rdf:about="http://www.w3.org/ns/oa#textDirection">
        <rdfs:range rdf:resource="http://www.w3.org/ns/oa#Direction"/>
        <rdfs:comment>The direction of the text of the subject resource. There MUST only be one text direction associated with any given resource.</rdfs:comment>
        <rdfs:isDefinedBy rdf:resource="http://www.w3.org/ns/oa#"/>
        <rdfs:label>textDirection</rdfs:label>
    </rdf:Description>
    


    <!-- http://www.w3.org/ns/prov#actedOnBehalfOf -->

    <owl:ObjectProperty rdf:about="http://www.w3.org/ns/prov#actedOnBehalfOf">
        <rdfs:subPropertyOf rdf:resource="http://www.w3.org/ns/prov#wasInfluencedBy"/>
        <rdfs:domain rdf:resource="http://www.w3.org/ns/prov#Agent"/>
        <rdfs:range rdf:resource="http://www.w3.org/ns/prov#Agent"/>
        <owl:propertyChainAxiom rdf:parseType="Collection">
            <rdf:Description rdf:about="http://www.w3.org/ns/prov#qualifiedDelegation"/>
            <rdf:Description rdf:about="http://www.w3.org/ns/prov#agent"/>
        </owl:propertyChainAxiom>
        <rdfs:comment xml:lang="en">An object property to express the accountability of an agent towards another agent. The subordinate agent acted on behalf of the responsible agent in an actual activity. </rdfs:comment>
        <rdfs:isDefinedBy rdf:resource="http://www.w3.org/ns/prov-o#"/>
        <rdfs:label>actedOnBehalfOf</rdfs:label>
        <prov:category>starting-point</prov:category>
        <prov:component>agents-responsibility</prov:component>
        <prov:inverse>hadDelegate</prov:inverse>
        <prov:qualifiedForm rdf:resource="http://www.w3.org/ns/prov#Delegation"/>
        <prov:qualifiedForm rdf:resource="http://www.w3.org/ns/prov#qualifiedDelegation"/>
    </owl:ObjectProperty>
    


    <!-- http://www.w3.org/ns/prov#activity -->

    <owl:ObjectProperty rdf:about="http://www.w3.org/ns/prov#activity">
        <rdfs:subPropertyOf rdf:resource="http://www.w3.org/ns/prov#influencer"/>
        <rdfs:domain rdf:resource="http://www.w3.org/ns/prov#ActivityInfluence"/>
        <rdfs:range rdf:resource="http://www.w3.org/ns/prov#Activity"/>
        <rdfs:isDefinedBy rdf:resource="http://www.w3.org/ns/prov-o#"/>
        <rdfs:label>activity</rdfs:label>
        <prov:category>qualified</prov:category>
        <prov:editorialNote xml:lang="en">This property behaves in spirit like rdf:object; it references the object of a prov:wasInfluencedBy triple.</prov:editorialNote>
        <prov:editorsDefinition>The prov:activity property references an prov:Activity which influenced a resource. This property applies to an prov:ActivityInfluence, which is given by a subproperty of prov:qualifiedInfluence from the influenced prov:Entity, prov:Activity or prov:Agent.</prov:editorsDefinition>
        <prov:inverse>activityOfInfluence</prov:inverse>
    </owl:ObjectProperty>
    


    <!-- http://www.w3.org/ns/prov#agent -->

    <owl:ObjectProperty rdf:about="http://www.w3.org/ns/prov#agent">
        <rdfs:subPropertyOf rdf:resource="http://www.w3.org/ns/prov#influencer"/>
        <rdfs:domain rdf:resource="http://www.w3.org/ns/prov#AgentInfluence"/>
        <rdfs:range rdf:resource="http://www.w3.org/ns/prov#Agent"/>
        <rdfs:isDefinedBy rdf:resource="http://www.w3.org/ns/prov-o#"/>
        <rdfs:label>agent</rdfs:label>
        <prov:category>qualified</prov:category>
        <prov:editorialNote xml:lang="en">This property behaves in spirit like rdf:object; it references the object of a prov:wasInfluencedBy triple.</prov:editorialNote>
        <prov:editorsDefinition xml:lang="en">The prov:agent property references an prov:Agent which influenced a resource. This property applies to an prov:AgentInfluence, which is given by a subproperty of prov:qualifiedInfluence from the influenced prov:Entity, prov:Activity or prov:Agent.</prov:editorsDefinition>
        <prov:inverse>agentOfInfluence</prov:inverse>
    </owl:ObjectProperty>
    


    <!-- http://www.w3.org/ns/prov#alternateOf -->

    <owl:ObjectProperty rdf:about="http://www.w3.org/ns/prov#alternateOf">
        <rdfs:domain rdf:resource="http://www.w3.org/ns/prov#Entity"/>
        <rdfs:range rdf:resource="http://www.w3.org/ns/prov#Entity"/>
        <rdfs:isDefinedBy rdf:resource="http://www.w3.org/ns/prov-o#"/>
        <rdfs:label>alternateOf</rdfs:label>
        <rdfs:seeAlso rdf:resource="http://www.w3.org/ns/prov#specializationOf"/>
        <prov:category>expanded</prov:category>
        <prov:component>alternate</prov:component>
        <prov:constraints rdf:datatype="http://www.w3.org/2001/XMLSchema#anyURI">http://www.w3.org/TR/2013/REC-prov-constraints-20130430/#prov-dm-constraints-fig</prov:constraints>
        <prov:definition xml:lang="en">Two alternate entities present aspects of the same thing. These aspects may be the same or different, and the alternate entities may or may not overlap in time.</prov:definition>
        <prov:dm rdf:datatype="http://www.w3.org/2001/XMLSchema#anyURI">http://www.w3.org/TR/2013/REC-prov-dm-20130430/#term-alternate</prov:dm>
        <prov:inverse>alternateOf</prov:inverse>
        <prov:n rdf:datatype="http://www.w3.org/2001/XMLSchema#anyURI">http://www.w3.org/TR/2013/REC-prov-n-20130430/#expression-alternate</prov:n>
    </owl:ObjectProperty>
    


    <!-- http://www.w3.org/ns/prov#atLocation -->

    <owl:ObjectProperty rdf:about="http://www.w3.org/ns/prov#atLocation">
        <rdfs:domain>
            <owl:Class>
                <owl:unionOf rdf:parseType="Collection">
                    <rdf:Description rdf:about="http://www.w3.org/ns/prov#Activity"/>
                    <rdf:Description rdf:about="http://www.w3.org/ns/prov#Agent"/>
                    <rdf:Description rdf:about="http://www.w3.org/ns/prov#Entity"/>
                    <rdf:Description rdf:about="http://www.w3.org/ns/prov#InstantaneousEvent"/>
                </owl:unionOf>
            </owl:Class>
        </rdfs:domain>
        <rdfs:range rdf:resource="http://www.w3.org/ns/prov#Location"/>
        <rdfs:comment xml:lang="en">The Location of any resource.</rdfs:comment>
        <rdfs:comment>This property has multiple RDFS domains to suit multiple OWL Profiles. See &lt;a href=&quot;#owl-profile&quot;&gt;PROV-O OWL Profile&lt;/a&gt;.</rdfs:comment>
        <rdfs:isDefinedBy rdf:resource="http://www.w3.org/ns/prov-o#"/>
        <rdfs:label>atLocation</rdfs:label>
        <prov:category>expanded</prov:category>
        <prov:editorialNote xml:lang="en">The naming of prov:atLocation parallels prov:atTime, and is not named prov:hadLocation to avoid conflicting with the convention that prov:had* properties are used on prov:Influence classes.</prov:editorialNote>
        <prov:editorialNote xml:lang="en">This property is not functional because the many values could be at a variety of granularies (In this building, in this room, in that chair).</prov:editorialNote>
        <prov:inverse>locationOf</prov:inverse>
        <prov:sharesDefinitionWith rdf:resource="http://www.w3.org/ns/prov#Location"/>
    </owl:ObjectProperty>
    


    <!-- http://www.w3.org/ns/prov#entity -->

    <owl:ObjectProperty rdf:about="http://www.w3.org/ns/prov#entity">
        <rdfs:subPropertyOf rdf:resource="http://www.w3.org/ns/prov#influencer"/>
        <rdfs:domain rdf:resource="http://www.w3.org/ns/prov#EntityInfluence"/>
        <rdfs:range rdf:resource="http://www.w3.org/ns/prov#Entity"/>
        <rdfs:isDefinedBy rdf:resource="http://www.w3.org/ns/prov-o#"/>
        <rdfs:label>entity</rdfs:label>
        <prov:category>qualified</prov:category>
        <prov:editorialNote xml:lang="en">This property behaves in spirit like rdf:object; it references the object of a prov:wasInfluencedBy triple.</prov:editorialNote>
        <prov:editorsDefinition>The prov:entity property references an prov:Entity which influenced a resource. This property applies to an prov:EntityInfluence, which is given by a subproperty of prov:qualifiedInfluence from the influenced prov:Entity, prov:Activity or prov:Agent.</prov:editorsDefinition>
        <prov:inverse>entityOfInfluence</prov:inverse>
    </owl:ObjectProperty>
    


    <!-- http://www.w3.org/ns/prov#generated -->

    <owl:ObjectProperty rdf:about="http://www.w3.org/ns/prov#generated">
        <rdfs:subPropertyOf rdf:resource="http://www.w3.org/ns/prov#influenced"/>
        <owl:inverseOf rdf:resource="http://www.w3.org/ns/prov#wasGeneratedBy"/>
        <rdfs:domain rdf:resource="http://www.w3.org/ns/prov#Activity"/>
        <rdfs:range rdf:resource="http://www.w3.org/ns/prov#Entity"/>
        <rdfs:isDefinedBy rdf:resource="http://www.w3.org/ns/prov-o#"/>
        <rdfs:label>generated</rdfs:label>
        <prov:category>expanded</prov:category>
        <prov:component>entities-activities</prov:component>
        <prov:editorialNote xml:lang="en">prov:generated is one of few inverse property defined, to allow Activity-oriented assertions in addition to Entity-oriented assertions.</prov:editorialNote>
        <prov:inverse>wasGeneratedBy</prov:inverse>
        <prov:sharesDefinitionWith rdf:resource="http://www.w3.org/ns/prov#Generation"/>
    </owl:ObjectProperty>
    


    <!-- http://www.w3.org/ns/prov#hadActivity -->

    <owl:ObjectProperty rdf:about="http://www.w3.org/ns/prov#hadActivity">
        <rdfs:domain rdf:resource="http://www.w3.org/ns/prov#Influence"/>
        <rdfs:domain>
            <owl:Class>
                <owl:unionOf rdf:parseType="Collection">
                    <rdf:Description rdf:about="http://www.w3.org/ns/prov#Delegation"/>
                    <rdf:Description rdf:about="http://www.w3.org/ns/prov#Derivation"/>
                    <rdf:Description rdf:about="http://www.w3.org/ns/prov#End"/>
                    <rdf:Description rdf:about="http://www.w3.org/ns/prov#Start"/>
                </owl:unionOf>
            </owl:Class>
        </rdfs:domain>
        <rdfs:range rdf:resource="http://www.w3.org/ns/prov#Activity"/>
        <rdfs:comment xml:lang="en">The _optional_ Activity of an Influence, which used, generated, invalidated, or was the responsibility of some Entity. This property is _not_ used by ActivityInfluence (use prov:activity instead).</rdfs:comment>
        <rdfs:comment>This property has multiple RDFS domains to suit multiple OWL Profiles. See &lt;a href=&quot;#owl-profile&quot;&gt;PROV-O OWL Profile&lt;/a&gt;.</rdfs:comment>
        <rdfs:isDefinedBy rdf:resource="http://www.w3.org/ns/prov-o#"/>
        <rdfs:label>hadActivity</rdfs:label>
        <prov:category>qualified</prov:category>
        <prov:component>derivations</prov:component>
        <prov:editorialNote xml:lang="en">The multiple rdfs:domain assertions are intended. One is simpler and works for OWL-RL, the union is more specific but is not recognized by OWL-RL.</prov:editorialNote>
        <prov:inverse>wasActivityOfInfluence</prov:inverse>
        <prov:sharesDefinitionWith rdf:resource="http://www.w3.org/ns/prov#Activity"/>
    </owl:ObjectProperty>
    


    <!-- http://www.w3.org/ns/prov#hadGeneration -->

    <owl:ObjectProperty rdf:about="http://www.w3.org/ns/prov#hadGeneration">
        <rdfs:domain rdf:resource="http://www.w3.org/ns/prov#Derivation"/>
        <rdfs:range rdf:resource="http://www.w3.org/ns/prov#Generation"/>
        <rdfs:comment xml:lang="en">The _optional_ Generation involved in an Entity&apos;s Derivation.</rdfs:comment>
        <rdfs:isDefinedBy rdf:resource="http://www.w3.org/ns/prov-o#"/>
        <rdfs:label>hadGeneration</rdfs:label>
        <prov:category>qualified</prov:category>
        <prov:component>derivations</prov:component>
        <prov:inverse>generatedAsDerivation</prov:inverse>
        <prov:sharesDefinitionWith rdf:resource="http://www.w3.org/ns/prov#Generation"/>
    </owl:ObjectProperty>
    


    <!-- http://www.w3.org/ns/prov#hadMember -->

    <owl:ObjectProperty rdf:about="http://www.w3.org/ns/prov#hadMember">
        <rdfs:subPropertyOf rdf:resource="http://www.w3.org/ns/prov#wasInfluencedBy"/>
        <rdfs:domain rdf:resource="http://www.w3.org/ns/prov#Collection"/>
        <rdfs:range rdf:resource="http://www.w3.org/ns/prov#Entity"/>
        <rdfs:isDefinedBy rdf:resource="http://www.w3.org/ns/prov-o#"/>
        <rdfs:label>hadMember</rdfs:label>
        <prov:category>expanded</prov:category>
        <prov:component>expanded</prov:component>
        <prov:inverse>wasMemberOf</prov:inverse>
        <prov:sharesDefinitionWith rdf:resource="http://www.w3.org/ns/prov#Collection"/>
    </owl:ObjectProperty>
    <owl:Axiom>
        <owl:annotatedSource rdf:resource="http://www.w3.org/ns/prov#hadMember"/>
        <owl:annotatedProperty rdf:resource="http://www.w3.org/2000/01/rdf-schema#range"/>
        <owl:annotatedTarget rdf:resource="http://www.w3.org/ns/prov#Entity"/>
        <rdfs:comment xml:lang="en">A collection is an entity that provides a structure to some constituents, which are themselves entities. These constituents are said to be member of the collections.</rdfs:comment>
        <prov:dm>http://www.w3.org/TR/2013/REC-prov-dm-20130430/#term-collection</prov:dm>
    </owl:Axiom>
    


    <!-- http://www.w3.org/ns/prov#hadPlan -->

    <owl:ObjectProperty rdf:about="http://www.w3.org/ns/prov#hadPlan">
        <rdfs:domain rdf:resource="http://www.w3.org/ns/prov#Association"/>
        <rdfs:range rdf:resource="http://www.w3.org/ns/prov#Plan"/>
        <rdfs:comment xml:lang="en">The _optional_ Plan adopted by an Agent in Association with some Activity. Plan specifications are out of the scope of this specification.</rdfs:comment>
        <rdfs:isDefinedBy rdf:resource="http://www.w3.org/ns/prov-o#"/>
        <rdfs:label>hadPlan</rdfs:label>
        <prov:category>qualified</prov:category>
        <prov:component>agents-responsibility</prov:component>
        <prov:inverse>wasPlanOf</prov:inverse>
        <prov:sharesDefinitionWith rdf:resource="http://www.w3.org/ns/prov#Plan"/>
    </owl:ObjectProperty>
    


    <!-- http://www.w3.org/ns/prov#hadPrimarySource -->

    <owl:ObjectProperty rdf:about="http://www.w3.org/ns/prov#hadPrimarySource">
        <rdfs:subPropertyOf rdf:resource="http://www.w3.org/ns/prov#wasDerivedFrom"/>
        <rdfs:domain rdf:resource="http://www.w3.org/ns/prov#Entity"/>
        <rdfs:range rdf:resource="http://www.w3.org/ns/prov#Entity"/>
        <owl:propertyChainAxiom rdf:parseType="Collection">
            <rdf:Description rdf:about="http://www.w3.org/ns/prov#qualifiedPrimarySource"/>
            <rdf:Description rdf:about="http://www.w3.org/ns/prov#entity"/>
        </owl:propertyChainAxiom>
        <rdfs:isDefinedBy rdf:resource="http://www.w3.org/ns/prov-o#"/>
        <rdfs:label>hadPrimarySource</rdfs:label>
        <prov:category>expanded</prov:category>
        <prov:component>derivations</prov:component>
        <prov:inverse>wasPrimarySourceOf</prov:inverse>
        <prov:qualifiedForm rdf:resource="http://www.w3.org/ns/prov#PrimarySource"/>
        <prov:qualifiedForm rdf:resource="http://www.w3.org/ns/prov#qualifiedPrimarySource"/>
    </owl:ObjectProperty>
    <owl:Axiom>
        <owl:annotatedSource rdf:resource="http://www.w3.org/ns/prov#hadPrimarySource"/>
        <owl:annotatedProperty rdf:resource="http://www.w3.org/2000/01/rdf-schema#subPropertyOf"/>
        <owl:annotatedTarget rdf:resource="http://www.w3.org/ns/prov#wasDerivedFrom"/>
        <rdfs:comment>hadPrimarySource property is a particular case of wasDerivedFrom (see http://www.w3.org/TR/prov-dm/#term-original-source) that aims to give credit to the source that originated some information.</rdfs:comment>
    </owl:Axiom>
    


    <!-- http://www.w3.org/ns/prov#hadRole -->

    <owl:ObjectProperty rdf:about="http://www.w3.org/ns/prov#hadRole">
        <rdfs:domain rdf:resource="http://www.w3.org/ns/prov#Influence"/>
        <rdfs:domain>
            <owl:Class>
                <owl:unionOf rdf:parseType="Collection">
                    <rdf:Description rdf:about="http://www.w3.org/ns/prov#Association"/>
                    <rdf:Description rdf:about="http://www.w3.org/ns/prov#InstantaneousEvent"/>
                </owl:unionOf>
            </owl:Class>
        </rdfs:domain>
        <rdfs:range rdf:resource="http://www.w3.org/ns/prov#Role"/>
        <rdfs:comment xml:lang="en">The _optional_ Role that an Entity assumed in the context of an Activity. For example, :baking prov:used :spoon; prov:qualified [ a prov:Usage; prov:entity :spoon; prov:hadRole roles:mixing_implement ].</rdfs:comment>
        <rdfs:comment>This property has multiple RDFS domains to suit multiple OWL Profiles. See &lt;a href=&quot;#owl-profile&quot;&gt;PROV-O OWL Profile&lt;/a&gt;.</rdfs:comment>
        <rdfs:isDefinedBy rdf:resource="http://www.w3.org/ns/prov-o#"/>
        <rdfs:label>hadRole</rdfs:label>
        <prov:category>qualified</prov:category>
        <prov:component>agents-responsibility</prov:component>
        <prov:editorsDefinition xml:lang="en">prov:hadRole references the Role (i.e. the function of an entity with respect to an activity), in the context of an instantaneous usage, generation, association, start, and end.</prov:editorsDefinition>
        <prov:inverse>wasRoleIn</prov:inverse>
        <prov:sharesDefinitionWith rdf:resource="http://www.w3.org/ns/prov#Role"/>
    </owl:ObjectProperty>
    


    <!-- http://www.w3.org/ns/prov#hadUsage -->

    <owl:ObjectProperty rdf:about="http://www.w3.org/ns/prov#hadUsage">
        <rdfs:domain rdf:resource="http://www.w3.org/ns/prov#Derivation"/>
        <rdfs:range rdf:resource="http://www.w3.org/ns/prov#Usage"/>
        <rdfs:comment xml:lang="en">The _optional_ Usage involved in an Entity&apos;s Derivation.</rdfs:comment>
        <rdfs:isDefinedBy rdf:resource="http://www.w3.org/ns/prov-o#"/>
        <rdfs:label>hadUsage</rdfs:label>
        <prov:category>qualified</prov:category>
        <prov:component>derivations</prov:component>
        <prov:inverse>wasUsedInDerivation</prov:inverse>
        <prov:sharesDefinitionWith rdf:resource="http://www.w3.org/ns/prov#Usage"/>
    </owl:ObjectProperty>
    


    <!-- http://www.w3.org/ns/prov#influenced -->

    <owl:ObjectProperty rdf:about="http://www.w3.org/ns/prov#influenced">
        <owl:inverseOf rdf:resource="http://www.w3.org/ns/prov#wasInfluencedBy"/>
        <rdfs:isDefinedBy rdf:resource="http://www.w3.org/ns/prov-o#"/>
        <rdfs:label>influenced</rdfs:label>
        <prov:category>expanded</prov:category>
        <prov:component>agents-responsibility</prov:component>
        <prov:inverse>wasInfluencedBy</prov:inverse>
        <prov:sharesDefinitionWith rdf:resource="http://www.w3.org/ns/prov#Influence"/>
    </owl:ObjectProperty>
    


    <!-- http://www.w3.org/ns/prov#influencer -->

    <owl:ObjectProperty rdf:about="http://www.w3.org/ns/prov#influencer">
        <rdfs:domain rdf:resource="http://www.w3.org/ns/prov#Influence"/>
        <rdfs:range rdf:resource="http://www.w3.org/2002/07/owl#Thing"/>
        <rdfs:comment xml:lang="en">Subproperties of prov:influencer are used to cite the object of an unqualified PROV-O triple whose predicate is a subproperty of prov:wasInfluencedBy (e.g. prov:used, prov:wasGeneratedBy). prov:influencer is used much like rdf:object is used.</rdfs:comment>
        <rdfs:isDefinedBy rdf:resource="http://www.w3.org/ns/prov-o#"/>
        <rdfs:label>influencer</rdfs:label>
        <prov:category>qualified</prov:category>
        <prov:dm rdf:datatype="http://www.w3.org/2001/XMLSchema#anyURI">http://www.w3.org/TR/2013/REC-prov-dm-20130430/#term-influence</prov:dm>
        <prov:editorialNote xml:lang="en">This property and its subproperties are used in the same way as the rdf:object property, i.e. to reference the object of an unqualified prov:wasInfluencedBy or prov:influenced triple.</prov:editorialNote>
        <prov:editorsDefinition xml:lang="en">This property is used as part of the qualified influence pattern. Subclasses of prov:Influence use these subproperties to reference the resource (Entity, Agent, or Activity) whose influence is being qualified.</prov:editorsDefinition>
        <prov:inverse>hadInfluence</prov:inverse>
    </owl:ObjectProperty>
    


    <!-- http://www.w3.org/ns/prov#invalidated -->

    <owl:ObjectProperty rdf:about="http://www.w3.org/ns/prov#invalidated">
        <rdfs:subPropertyOf rdf:resource="http://www.w3.org/ns/prov#influenced"/>
        <owl:inverseOf rdf:resource="http://www.w3.org/ns/prov#wasInvalidatedBy"/>
        <rdfs:domain rdf:resource="http://www.w3.org/ns/prov#Activity"/>
        <rdfs:range rdf:resource="http://www.w3.org/ns/prov#Entity"/>
        <rdfs:isDefinedBy rdf:resource="http://www.w3.org/ns/prov-o#"/>
        <rdfs:label>invalidated</rdfs:label>
        <prov:category>expanded</prov:category>
        <prov:component>entities-activities</prov:component>
        <prov:editorialNote xml:lang="en">prov:invalidated is one of few inverse property defined, to allow Activity-oriented assertions in addition to Entity-oriented assertions.</prov:editorialNote>
        <prov:inverse>wasInvalidatedBy</prov:inverse>
        <prov:sharesDefinitionWith rdf:resource="http://www.w3.org/ns/prov#Invalidation"/>
    </owl:ObjectProperty>
    


    <!-- http://www.w3.org/ns/prov#qualifiedAssociation -->

    <owl:ObjectProperty rdf:about="http://www.w3.org/ns/prov#qualifiedAssociation">
        <rdfs:subPropertyOf rdf:resource="http://www.w3.org/ns/prov#qualifiedInfluence"/>
        <rdfs:domain rdf:resource="http://www.w3.org/ns/prov#Activity"/>
        <rdfs:range rdf:resource="http://www.w3.org/ns/prov#Association"/>
        <rdfs:comment xml:lang="en">If this Activity prov:wasAssociatedWith Agent :ag, then it can qualify the Association using prov:qualifiedAssociation [ a prov:Association;  prov:agent :ag; :foo :bar ].</rdfs:comment>
        <rdfs:isDefinedBy rdf:resource="http://www.w3.org/ns/prov-o#"/>
        <rdfs:label>qualifiedAssociation</rdfs:label>
        <prov:category>qualified</prov:category>
        <prov:component>agents-responsibility</prov:component>
        <prov:inverse>qualifiedAssociationOf</prov:inverse>
        <prov:sharesDefinitionWith rdf:resource="http://www.w3.org/ns/prov#Association"/>
        <prov:unqualifiedForm rdf:resource="http://www.w3.org/ns/prov#wasAssociatedWith"/>
    </owl:ObjectProperty>
    


    <!-- http://www.w3.org/ns/prov#qualifiedAttribution -->

    <owl:ObjectProperty rdf:about="http://www.w3.org/ns/prov#qualifiedAttribution">
        <rdfs:subPropertyOf rdf:resource="http://www.w3.org/ns/prov#qualifiedInfluence"/>
        <rdfs:domain rdf:resource="http://www.w3.org/ns/prov#Entity"/>
        <rdfs:range rdf:resource="http://www.w3.org/ns/prov#Attribution"/>
        <rdfs:comment xml:lang="en">If this Entity prov:wasAttributedTo Agent :ag, then it can qualify how it was influenced using prov:qualifiedAttribution [ a prov:Attribution;  prov:agent :ag; :foo :bar ].</rdfs:comment>
        <rdfs:isDefinedBy rdf:resource="http://www.w3.org/ns/prov-o#"/>
        <rdfs:label>qualifiedAttribution</rdfs:label>
        <prov:category>qualified</prov:category>
        <prov:component>agents-responsibility</prov:component>
        <prov:inverse>qualifiedAttributionOf</prov:inverse>
        <prov:sharesDefinitionWith rdf:resource="http://www.w3.org/ns/prov#Attribution"/>
        <prov:unqualifiedForm rdf:resource="http://www.w3.org/ns/prov#wasAttributedTo"/>
    </owl:ObjectProperty>
    


    <!-- http://www.w3.org/ns/prov#qualifiedCommunication -->

    <owl:ObjectProperty rdf:about="http://www.w3.org/ns/prov#qualifiedCommunication">
        <rdfs:subPropertyOf rdf:resource="http://www.w3.org/ns/prov#qualifiedInfluence"/>
        <rdfs:domain rdf:resource="http://www.w3.org/ns/prov#Activity"/>
        <rdfs:range rdf:resource="http://www.w3.org/ns/prov#Communication"/>
        <rdfs:comment xml:lang="en">If this Activity prov:wasInformedBy Activity :a, then it can qualify how it was influenced using prov:qualifiedCommunication [ a prov:Communication;  prov:activity :a; :foo :bar ].</rdfs:comment>
        <rdfs:isDefinedBy rdf:resource="http://www.w3.org/ns/prov-o#"/>
        <rdfs:label>qualifiedCommunication</rdfs:label>
        <prov:category>qualified</prov:category>
        <prov:component>entities-activities</prov:component>
        <prov:inverse>qualifiedCommunicationOf</prov:inverse>
        <prov:qualifiedForm rdf:resource="http://www.w3.org/ns/prov#Communication"/>
        <prov:sharesDefinitionWith rdf:resource="http://www.w3.org/ns/prov#Communication"/>
    </owl:ObjectProperty>
    


    <!-- http://www.w3.org/ns/prov#qualifiedDelegation -->

    <owl:ObjectProperty rdf:about="http://www.w3.org/ns/prov#qualifiedDelegation">
        <rdfs:subPropertyOf rdf:resource="http://www.w3.org/ns/prov#qualifiedInfluence"/>
        <rdfs:domain rdf:resource="http://www.w3.org/ns/prov#Agent"/>
        <rdfs:range rdf:resource="http://www.w3.org/ns/prov#Delegation"/>
        <rdfs:comment xml:lang="en">If this Agent prov:actedOnBehalfOf Agent :ag, then it can qualify how with prov:qualifiedResponsibility [ a prov:Responsibility;  prov:agent :ag; :foo :bar ].</rdfs:comment>
        <rdfs:isDefinedBy rdf:resource="http://www.w3.org/ns/prov-o#"/>
        <rdfs:label>qualifiedDelegation</rdfs:label>
        <prov:category>qualified</prov:category>
        <prov:component>agents-responsibility</prov:component>
        <prov:inverse>qualifiedDelegationOf</prov:inverse>
        <prov:sharesDefinitionWith rdf:resource="http://www.w3.org/ns/prov#Delegation"/>
        <prov:unqualifiedForm rdf:resource="http://www.w3.org/ns/prov#actedOnBehalfOf"/>
    </owl:ObjectProperty>
    


    <!-- http://www.w3.org/ns/prov#qualifiedDerivation -->

    <owl:ObjectProperty rdf:about="http://www.w3.org/ns/prov#qualifiedDerivation">
        <rdfs:subPropertyOf rdf:resource="http://www.w3.org/ns/prov#qualifiedInfluence"/>
        <rdfs:domain rdf:resource="http://www.w3.org/ns/prov#Entity"/>
        <rdfs:range rdf:resource="http://www.w3.org/ns/prov#Derivation"/>
        <rdfs:comment xml:lang="en">If this Entity prov:wasDerivedFrom Entity :e, then it can qualify how it was derived using prov:qualifiedDerivation [ a prov:Derivation;  prov:entity :e; :foo :bar ].</rdfs:comment>
        <rdfs:isDefinedBy rdf:resource="http://www.w3.org/ns/prov-o#"/>
        <rdfs:label>qualifiedDerivation</rdfs:label>
        <prov:category>qualified</prov:category>
        <prov:component>derivations</prov:component>
        <prov:inverse>qualifiedDerivationOf</prov:inverse>
        <prov:sharesDefinitionWith rdf:resource="http://www.w3.org/ns/prov#Derivation"/>
        <prov:unqualifiedForm rdf:resource="http://www.w3.org/ns/prov#wasDerivedFrom"/>
    </owl:ObjectProperty>
    


    <!-- http://www.w3.org/ns/prov#qualifiedEnd -->

    <owl:ObjectProperty rdf:about="http://www.w3.org/ns/prov#qualifiedEnd">
        <rdfs:subPropertyOf rdf:resource="http://www.w3.org/ns/prov#qualifiedInfluence"/>
        <rdfs:domain rdf:resource="http://www.w3.org/ns/prov#Activity"/>
        <rdfs:range rdf:resource="http://www.w3.org/ns/prov#End"/>
        <rdfs:comment xml:lang="en">If this Activity prov:wasEndedBy Entity :e1, then it can qualify how it was ended using prov:qualifiedEnd [ a prov:End;  prov:entity :e1; :foo :bar ].</rdfs:comment>
        <rdfs:isDefinedBy rdf:resource="http://www.w3.org/ns/prov-o#"/>
        <rdfs:label>qualifiedEnd</rdfs:label>
        <prov:category>qualified</prov:category>
        <prov:component>entities-activities</prov:component>
        <prov:inverse>qualifiedEndOf</prov:inverse>
        <prov:sharesDefinitionWith rdf:resource="http://www.w3.org/ns/prov#End"/>
        <prov:unqualifiedForm rdf:resource="http://www.w3.org/ns/prov#wasEndedBy"/>
    </owl:ObjectProperty>
    


    <!-- http://www.w3.org/ns/prov#qualifiedGeneration -->

    <owl:ObjectProperty rdf:about="http://www.w3.org/ns/prov#qualifiedGeneration">
        <rdfs:subPropertyOf rdf:resource="http://www.w3.org/ns/prov#qualifiedInfluence"/>
        <rdfs:domain rdf:resource="http://www.w3.org/ns/prov#Entity"/>
        <rdfs:range rdf:resource="http://www.w3.org/ns/prov#Generation"/>
        <rdfs:comment xml:lang="en">If this Activity prov:generated Entity :e, then it can qualify how it performed the Generation using prov:qualifiedGeneration [ a prov:Generation;  prov:entity :e; :foo :bar ].</rdfs:comment>
        <rdfs:isDefinedBy rdf:resource="http://www.w3.org/ns/prov-o#"/>
        <rdfs:label>qualifiedGeneration</rdfs:label>
        <prov:category>qualified</prov:category>
        <prov:component>entities-activities</prov:component>
        <prov:inverse>qualifiedGenerationOf</prov:inverse>
        <prov:sharesDefinitionWith rdf:resource="http://www.w3.org/ns/prov#Generation"/>
        <prov:unqualifiedForm rdf:resource="http://www.w3.org/ns/prov#wasGeneratedBy"/>
    </owl:ObjectProperty>
    


    <!-- http://www.w3.org/ns/prov#qualifiedInfluence -->

    <owl:ObjectProperty rdf:about="http://www.w3.org/ns/prov#qualifiedInfluence">
        <rdfs:domain>
            <owl:Class>
                <owl:unionOf rdf:parseType="Collection">
                    <rdf:Description rdf:about="http://www.w3.org/ns/prov#Activity"/>
                    <rdf:Description rdf:about="http://www.w3.org/ns/prov#Agent"/>
                    <rdf:Description rdf:about="http://www.w3.org/ns/prov#Entity"/>
                </owl:unionOf>
            </owl:Class>
        </rdfs:domain>
        <rdfs:range rdf:resource="http://www.w3.org/ns/prov#Influence"/>
        <rdfs:comment xml:lang="en">Because prov:qualifiedInfluence is a broad relation, the more specific relations (qualifiedCommunication, qualifiedDelegation, qualifiedEnd, etc.) should be used when applicable.</rdfs:comment>
        <rdfs:isDefinedBy rdf:resource="http://www.w3.org/ns/prov-o#"/>
        <rdfs:label>qualifiedInfluence</rdfs:label>
        <prov:category>qualified</prov:category>
        <prov:component>derivations</prov:component>
        <prov:inverse>qualifiedInfluenceOf</prov:inverse>
        <prov:sharesDefinitionWith rdf:resource="http://www.w3.org/ns/prov#Influence"/>
        <prov:unqualifiedForm rdf:resource="http://www.w3.org/ns/prov#wasInfluencedBy"/>
    </owl:ObjectProperty>
    


    <!-- http://www.w3.org/ns/prov#qualifiedInvalidation -->

    <owl:ObjectProperty rdf:about="http://www.w3.org/ns/prov#qualifiedInvalidation">
        <rdfs:subPropertyOf rdf:resource="http://www.w3.org/ns/prov#qualifiedInfluence"/>
        <rdfs:domain rdf:resource="http://www.w3.org/ns/prov#Entity"/>
        <rdfs:range rdf:resource="http://www.w3.org/ns/prov#Invalidation"/>
        <rdfs:comment xml:lang="en">If this Entity prov:wasInvalidatedBy Activity :a, then it can qualify how it was invalidated using prov:qualifiedInvalidation [ a prov:Invalidation;  prov:activity :a; :foo :bar ].</rdfs:comment>
        <rdfs:isDefinedBy rdf:resource="http://www.w3.org/ns/prov-o#"/>
        <rdfs:label>qualifiedInvalidation</rdfs:label>
        <prov:category>qualified</prov:category>
        <prov:component>entities-activities</prov:component>
        <prov:inverse>qualifiedInvalidationOf</prov:inverse>
        <prov:sharesDefinitionWith rdf:resource="http://www.w3.org/ns/prov#Invalidation"/>
        <prov:unqualifiedForm rdf:resource="http://www.w3.org/ns/prov#wasInvalidatedBy"/>
    </owl:ObjectProperty>
    


    <!-- http://www.w3.org/ns/prov#qualifiedPrimarySource -->

    <owl:ObjectProperty rdf:about="http://www.w3.org/ns/prov#qualifiedPrimarySource">
        <rdfs:subPropertyOf rdf:resource="http://www.w3.org/ns/prov#qualifiedInfluence"/>
        <rdfs:domain rdf:resource="http://www.w3.org/ns/prov#Entity"/>
        <rdfs:range rdf:resource="http://www.w3.org/ns/prov#PrimarySource"/>
        <rdfs:comment xml:lang="en">If this Entity prov:hadPrimarySource Entity :e, then it can qualify how using prov:qualifiedPrimarySource [ a prov:PrimarySource; prov:entity :e; :foo :bar ].</rdfs:comment>
        <rdfs:isDefinedBy rdf:resource="http://www.w3.org/ns/prov-o#"/>
        <rdfs:label>qualifiedPrimarySource</rdfs:label>
        <prov:category>qualified</prov:category>
        <prov:component>derivations</prov:component>
        <prov:inverse>qualifiedSourceOf</prov:inverse>
        <prov:sharesDefinitionWith rdf:resource="http://www.w3.org/ns/prov#PrimarySource"/>
        <prov:unqualifiedForm rdf:resource="http://www.w3.org/ns/prov#hadPrimarySource"/>
    </owl:ObjectProperty>
    


    <!-- http://www.w3.org/ns/prov#qualifiedQuotation -->

    <owl:ObjectProperty rdf:about="http://www.w3.org/ns/prov#qualifiedQuotation">
        <rdfs:subPropertyOf rdf:resource="http://www.w3.org/ns/prov#qualifiedInfluence"/>
        <rdfs:domain rdf:resource="http://www.w3.org/ns/prov#Entity"/>
        <rdfs:range rdf:resource="http://www.w3.org/ns/prov#Quotation"/>
        <rdfs:comment xml:lang="en">If this Entity prov:wasQuotedFrom Entity :e, then it can qualify how using prov:qualifiedQuotation [ a prov:Quotation;  prov:entity :e; :foo :bar ].</rdfs:comment>
        <rdfs:isDefinedBy rdf:resource="http://www.w3.org/ns/prov-o#"/>
        <rdfs:label>qualifiedQuotation</rdfs:label>
        <prov:category>qualified</prov:category>
        <prov:component>derivations</prov:component>
        <prov:inverse>qualifiedQuotationOf</prov:inverse>
        <prov:sharesDefinitionWith rdf:resource="http://www.w3.org/ns/prov#Quotation"/>
        <prov:unqualifiedForm rdf:resource="http://www.w3.org/ns/prov#wasQuotedFrom"/>
    </owl:ObjectProperty>
    


    <!-- http://www.w3.org/ns/prov#qualifiedRevision -->

    <owl:ObjectProperty rdf:about="http://www.w3.org/ns/prov#qualifiedRevision">
        <rdfs:subPropertyOf rdf:resource="http://www.w3.org/ns/prov#qualifiedInfluence"/>
        <rdfs:domain rdf:resource="http://www.w3.org/ns/prov#Entity"/>
        <rdfs:range rdf:resource="http://www.w3.org/ns/prov#Revision"/>
        <rdfs:comment xml:lang="en">If this Entity prov:wasRevisionOf Entity :e, then it can qualify how it was revised using prov:qualifiedRevision [ a prov:Revision;  prov:entity :e; :foo :bar ].</rdfs:comment>
        <rdfs:isDefinedBy rdf:resource="http://www.w3.org/ns/prov-o#"/>
        <rdfs:label>qualifiedRevision</rdfs:label>
        <prov:category>qualified</prov:category>
        <prov:component>derivations</prov:component>
        <prov:inverse>revisedEntity</prov:inverse>
        <prov:sharesDefinitionWith rdf:resource="http://www.w3.org/ns/prov#Revision"/>
        <prov:unqualifiedForm rdf:resource="http://www.w3.org/ns/prov#wasRevisionOf"/>
    </owl:ObjectProperty>
    


    <!-- http://www.w3.org/ns/prov#qualifiedStart -->

    <owl:ObjectProperty rdf:about="http://www.w3.org/ns/prov#qualifiedStart">
        <rdfs:subPropertyOf rdf:resource="http://www.w3.org/ns/prov#qualifiedInfluence"/>
        <rdfs:domain rdf:resource="http://www.w3.org/ns/prov#Activity"/>
        <rdfs:range rdf:resource="http://www.w3.org/ns/prov#Start"/>
        <rdfs:comment xml:lang="en">If this Activity prov:wasStartedBy Entity :e1, then it can qualify how it was started using prov:qualifiedStart [ a prov:Start;  prov:entity :e1; :foo :bar ].</rdfs:comment>
        <rdfs:isDefinedBy rdf:resource="http://www.w3.org/ns/prov-o#"/>
        <rdfs:label>qualifiedStart</rdfs:label>
        <prov:category>qualified</prov:category>
        <prov:component>entities-activities</prov:component>
        <prov:inverse>qualifiedStartOf</prov:inverse>
        <prov:sharesDefinitionWith rdf:resource="http://www.w3.org/ns/prov#Start"/>
        <prov:unqualifiedForm rdf:resource="http://www.w3.org/ns/prov#wasStartedBy"/>
    </owl:ObjectProperty>
    


    <!-- http://www.w3.org/ns/prov#qualifiedUsage -->

    <owl:ObjectProperty rdf:about="http://www.w3.org/ns/prov#qualifiedUsage">
        <rdfs:subPropertyOf rdf:resource="http://www.w3.org/ns/prov#qualifiedInfluence"/>
        <rdfs:domain rdf:resource="http://www.w3.org/ns/prov#Activity"/>
        <rdfs:range rdf:resource="http://www.w3.org/ns/prov#Usage"/>
        <rdfs:comment xml:lang="en">If this Activity prov:used Entity :e, then it can qualify how it used it using prov:qualifiedUsage [ a prov:Usage; prov:entity :e; :foo :bar ].</rdfs:comment>
        <rdfs:isDefinedBy rdf:resource="http://www.w3.org/ns/prov-o#"/>
        <rdfs:label>qualifiedUsage</rdfs:label>
        <prov:category>qualified</prov:category>
        <prov:component>entities-activities</prov:component>
        <prov:inverse>qualifiedUsingActivity</prov:inverse>
        <prov:sharesDefinitionWith rdf:resource="http://www.w3.org/ns/prov#Usage"/>
        <prov:unqualifiedForm rdf:resource="http://www.w3.org/ns/prov#used"/>
    </owl:ObjectProperty>
    


    <!-- http://www.w3.org/ns/prov#specializationOf -->

    <owl:ObjectProperty rdf:about="http://www.w3.org/ns/prov#specializationOf">
        <rdfs:subPropertyOf rdf:resource="http://www.w3.org/ns/prov#alternateOf"/>
        <rdfs:domain rdf:resource="http://www.w3.org/ns/prov#Entity"/>
    </owl:ObjectProperty>
    


    <!-- http://www.w3.org/ns/prov#used -->

    <owl:ObjectProperty rdf:about="http://www.w3.org/ns/prov#used">
        <rdfs:subPropertyOf rdf:resource="http://www.w3.org/ns/prov#wasInfluencedBy"/>
        <rdfs:domain rdf:resource="http://www.w3.org/ns/prov#Activity"/>
        <rdfs:range rdf:resource="http://www.w3.org/ns/prov#Entity"/>
        <owl:propertyChainAxiom rdf:parseType="Collection">
            <rdf:Description rdf:about="http://www.w3.org/ns/prov#qualifiedUsage"/>
            <rdf:Description rdf:about="http://www.w3.org/ns/prov#entity"/>
        </owl:propertyChainAxiom>
        <rdfs:comment xml:lang="en">A prov:Entity that was used by this prov:Activity. For example, :baking prov:used :spoon, :egg, :oven .</rdfs:comment>
        <rdfs:isDefinedBy rdf:resource="http://www.w3.org/ns/prov-o#"/>
        <rdfs:label>used</rdfs:label>
        <prov:category>starting-point</prov:category>
        <prov:component>entities-activities</prov:component>
        <prov:inverse>wasUsedBy</prov:inverse>
        <prov:qualifiedForm rdf:resource="http://www.w3.org/ns/prov#Usage"/>
        <prov:qualifiedForm rdf:resource="http://www.w3.org/ns/prov#qualifiedUsage"/>
    </owl:ObjectProperty>
    


    <!-- http://www.w3.org/ns/prov#wasAssociatedWith -->

    <owl:ObjectProperty rdf:about="http://www.w3.org/ns/prov#wasAssociatedWith">
        <rdfs:subPropertyOf rdf:resource="http://www.w3.org/ns/prov#wasInfluencedBy"/>
        <rdfs:domain rdf:resource="http://www.w3.org/ns/prov#Activity"/>
        <rdfs:range rdf:resource="http://www.w3.org/ns/prov#Agent"/>
        <owl:propertyChainAxiom rdf:parseType="Collection">
            <rdf:Description rdf:about="http://www.w3.org/ns/prov#qualifiedAssociation"/>
            <rdf:Description rdf:about="http://www.w3.org/ns/prov#agent"/>
        </owl:propertyChainAxiom>
        <rdfs:comment xml:lang="en">An prov:Agent that had some (unspecified) responsibility for the occurrence of this prov:Activity.</rdfs:comment>
        <rdfs:isDefinedBy rdf:resource="http://www.w3.org/ns/prov-o#"/>
        <rdfs:label>wasAssociatedWith</rdfs:label>
        <prov:category>starting-point</prov:category>
        <prov:component>agents-responsibility</prov:component>
        <prov:inverse>wasAssociateFor</prov:inverse>
        <prov:qualifiedForm rdf:resource="http://www.w3.org/ns/prov#Association"/>
        <prov:qualifiedForm rdf:resource="http://www.w3.org/ns/prov#qualifiedAssociation"/>
    </owl:ObjectProperty>
    


    <!-- http://www.w3.org/ns/prov#wasAttributedTo -->

    <owl:ObjectProperty rdf:about="http://www.w3.org/ns/prov#wasAttributedTo">
        <rdfs:subPropertyOf rdf:resource="http://www.w3.org/ns/prov#wasInfluencedBy"/>
        <rdfs:domain rdf:resource="http://www.w3.org/ns/prov#Entity"/>
        <rdfs:range rdf:resource="http://www.w3.org/ns/prov#Agent"/>
        <owl:propertyChainAxiom rdf:parseType="Collection">
            <rdf:Description rdf:about="http://www.w3.org/ns/prov#qualifiedAttribution"/>
            <rdf:Description rdf:about="http://www.w3.org/ns/prov#agent"/>
        </owl:propertyChainAxiom>
        <rdfs:comment xml:lang="en">Attribution is the ascribing of an entity to an agent.</rdfs:comment>
        <rdfs:isDefinedBy rdf:resource="http://www.w3.org/ns/prov-o#"/>
        <rdfs:label>wasAttributedTo</rdfs:label>
        <prov:category>starting-point</prov:category>
        <prov:component>agents-responsibility</prov:component>
        <prov:definition xml:lang="en">Attribution is the ascribing of an entity to an agent.</prov:definition>
        <prov:inverse>contributed</prov:inverse>
        <prov:qualifiedForm rdf:resource="http://www.w3.org/ns/prov#Attribution"/>
        <prov:qualifiedForm rdf:resource="http://www.w3.org/ns/prov#qualifiedAttribution"/>
    </owl:ObjectProperty>
    <owl:Axiom>
        <owl:annotatedSource rdf:resource="http://www.w3.org/ns/prov#wasAttributedTo"/>
        <owl:annotatedProperty rdf:resource="http://www.w3.org/2000/01/rdf-schema#subPropertyOf"/>
        <owl:annotatedTarget rdf:resource="http://www.w3.org/ns/prov#wasInfluencedBy"/>
        <rdfs:comment>Attribution is a particular case of trace (see http://www.w3.org/TR/prov-dm/#concept-trace), in the sense that it links an entity to the agent that ascribed it.</rdfs:comment>
        <prov:definition>IF wasAttributedTo(e2,ag1,aAttr) holds, THEN wasInfluencedBy(e2,ag1) also holds. </prov:definition>
    </owl:Axiom>
    


    <!-- http://www.w3.org/ns/prov#wasDerivedFrom -->

    <owl:ObjectProperty rdf:about="http://www.w3.org/ns/prov#wasDerivedFrom">
        <rdfs:subPropertyOf rdf:resource="http://www.w3.org/ns/prov#wasInfluencedBy"/>
        <rdfs:domain rdf:resource="http://www.w3.org/ns/prov#Entity"/>
        <rdfs:range rdf:resource="http://www.w3.org/ns/prov#Entity"/>
        <owl:propertyChainAxiom rdf:parseType="Collection">
            <rdf:Description rdf:about="http://www.w3.org/ns/prov#qualifiedDerivation"/>
            <rdf:Description rdf:about="http://www.w3.org/ns/prov#entity"/>
        </owl:propertyChainAxiom>
        <rdfs:comment xml:lang="en">The more specific subproperties of prov:wasDerivedFrom (i.e., prov:wasQuotedFrom, prov:wasRevisionOf, prov:hadPrimarySource) should be used when applicable.</rdfs:comment>
        <rdfs:isDefinedBy rdf:resource="http://www.w3.org/ns/prov-o#"/>
        <rdfs:label>wasDerivedFrom</rdfs:label>
        <prov:category>starting-point</prov:category>
        <prov:component>derivations</prov:component>
        <prov:definition xml:lang="en">A derivation is a transformation of an entity into another, an update of an entity resulting in a new one, or the construction of a new entity based on a pre-existing entity.</prov:definition>
        <prov:inverse>hadDerivation</prov:inverse>
        <prov:qualifiedForm rdf:resource="http://www.w3.org/ns/prov#Derivation"/>
        <prov:qualifiedForm rdf:resource="http://www.w3.org/ns/prov#qualifiedDerivation"/>
    </owl:ObjectProperty>
    <owl:Axiom>
        <owl:annotatedSource rdf:resource="http://www.w3.org/ns/prov#wasDerivedFrom"/>
        <owl:annotatedProperty rdf:resource="http://www.w3.org/2000/01/rdf-schema#subPropertyOf"/>
        <owl:annotatedTarget rdf:resource="http://www.w3.org/ns/prov#wasInfluencedBy"/>
        <rdfs:comment>Derivation is a particular case of trace (see http://www.w3.org/TR/prov-dm/#term-trace), since it links an entity to another entity that contributed to its existence.</rdfs:comment>
    </owl:Axiom>
    


    <!-- http://www.w3.org/ns/prov#wasEndedBy -->

    <owl:ObjectProperty rdf:about="http://www.w3.org/ns/prov#wasEndedBy">
        <rdfs:subPropertyOf rdf:resource="http://www.w3.org/ns/prov#wasInfluencedBy"/>
        <rdfs:domain rdf:resource="http://www.w3.org/ns/prov#Activity"/>
        <rdfs:range rdf:resource="http://www.w3.org/ns/prov#Entity"/>
        <owl:propertyChainAxiom rdf:parseType="Collection">
            <rdf:Description rdf:about="http://www.w3.org/ns/prov#qualifiedEnd"/>
            <rdf:Description rdf:about="http://www.w3.org/ns/prov#entity"/>
        </owl:propertyChainAxiom>
        <rdfs:comment xml:lang="en">End is when an activity is deemed to have ended. An end may refer to an entity, known as trigger, that terminated the activity.</rdfs:comment>
        <rdfs:isDefinedBy rdf:resource="http://www.w3.org/ns/prov-o#"/>
        <rdfs:label>wasEndedBy</rdfs:label>
        <prov:category>expanded</prov:category>
        <prov:component>entities-activities</prov:component>
        <prov:inverse>ended</prov:inverse>
        <prov:qualifiedForm rdf:resource="http://www.w3.org/ns/prov#End"/>
        <prov:qualifiedForm rdf:resource="http://www.w3.org/ns/prov#qualifiedEnd"/>
    </owl:ObjectProperty>
    


    <!-- http://www.w3.org/ns/prov#wasGeneratedBy -->

    <owl:ObjectProperty rdf:about="http://www.w3.org/ns/prov#wasGeneratedBy">
        <rdfs:subPropertyOf rdf:resource="http://www.w3.org/ns/prov#wasInfluencedBy"/>
        <rdfs:domain rdf:resource="http://www.w3.org/ns/prov#Entity"/>
        <rdfs:range rdf:resource="http://www.w3.org/ns/prov#Activity"/>
        <owl:propertyChainAxiom rdf:parseType="Collection">
            <rdf:Description rdf:about="http://www.w3.org/ns/prov#qualifiedGeneration"/>
            <rdf:Description rdf:about="http://www.w3.org/ns/prov#activity"/>
        </owl:propertyChainAxiom>
        <rdfs:isDefinedBy rdf:resource="http://www.w3.org/ns/prov-o#"/>
        <rdfs:label>wasGeneratedBy</rdfs:label>
        <prov:category>starting-point</prov:category>
        <prov:component>entities-activities</prov:component>
        <prov:inverse>generated</prov:inverse>
        <prov:qualifiedForm rdf:resource="http://www.w3.org/ns/prov#Generation"/>
        <prov:qualifiedForm rdf:resource="http://www.w3.org/ns/prov#qualifiedGeneration"/>
    </owl:ObjectProperty>
    


    <!-- http://www.w3.org/ns/prov#wasInfluencedBy -->

    <owl:ObjectProperty rdf:about="http://www.w3.org/ns/prov#wasInfluencedBy">
        <rdfs:domain rdf:nodeID="genid50"/>
        <rdfs:range rdf:nodeID="genid55"/>
        <rdfs:comment xml:lang="en">Because prov:wasInfluencedBy is a broad relation, its more specific subproperties (e.g. prov:wasInformedBy, prov:actedOnBehalfOf, prov:wasEndedBy, etc.) should be used when applicable.</rdfs:comment>
        <rdfs:comment>This property has multiple RDFS domains to suit multiple OWL Profiles. See &lt;a href=&quot;#owl-profile&quot;&gt;PROV-O OWL Profile&lt;/a&gt;.</rdfs:comment>
        <rdfs:isDefinedBy rdf:resource="http://www.w3.org/ns/prov-o#"/>
        <rdfs:label>wasInfluencedBy</rdfs:label>
        <prov:category>qualified</prov:category>
        <prov:component>agents-responsibility</prov:component>
        <prov:editorialNote xml:lang="en">The sub-properties of prov:wasInfluencedBy can be elaborated in more detail using the Qualification Pattern. For example, the binary relation :baking prov:used :spoon can be qualified by asserting :baking prov:qualifiedUsage [ a prov:Usage; prov:entity :spoon; prov:atLocation :kitchen ] .

Subproperties of prov:wasInfluencedBy may also be asserted directly without being qualified.

prov:wasInfluencedBy should not be used without also using one of its subproperties. 
</prov:editorialNote>
        <prov:inverse>influenced</prov:inverse>
        <prov:qualifiedForm rdf:resource="http://www.w3.org/ns/prov#Influence"/>
        <prov:qualifiedForm rdf:resource="http://www.w3.org/ns/prov#qualifiedInfluence"/>
        <prov:sharesDefinitionWith rdf:resource="http://www.w3.org/ns/prov#Influence"/>
    </owl:ObjectProperty>
    <owl:Class rdf:nodeID="genid50">
        <owl:unionOf rdf:parseType="Collection">
            <rdf:Description rdf:about="http://www.w3.org/ns/prov#Activity"/>
            <rdf:Description rdf:about="http://www.w3.org/ns/prov#Agent"/>
            <rdf:Description rdf:about="http://www.w3.org/ns/prov#Entity"/>
        </owl:unionOf>
    </owl:Class>
    <owl:Class rdf:nodeID="genid55">
        <owl:unionOf rdf:parseType="Collection">
            <rdf:Description rdf:about="http://www.w3.org/ns/prov#Activity"/>
            <rdf:Description rdf:about="http://www.w3.org/ns/prov#Agent"/>
            <rdf:Description rdf:about="http://www.w3.org/ns/prov#Entity"/>
        </owl:unionOf>
    </owl:Class>
    <owl:Axiom>
        <owl:annotatedSource rdf:resource="http://www.w3.org/ns/prov#wasInfluencedBy"/>
        <owl:annotatedProperty rdf:resource="http://www.w3.org/2000/01/rdf-schema#domain"/>
        <owl:annotatedTarget rdf:nodeID="genid50"/>
        <prov:definition>influencee: an identifier (o2) for an entity, activity, or agent; </prov:definition>
        <prov:dm>http://www.w3.org/TR/2013/REC-prov-dm-20130430/#term-influence</prov:dm>
    </owl:Axiom>
    <owl:Axiom>
        <owl:annotatedSource rdf:resource="http://www.w3.org/ns/prov#wasInfluencedBy"/>
        <owl:annotatedProperty rdf:resource="http://www.w3.org/2000/01/rdf-schema#range"/>
        <owl:annotatedTarget rdf:nodeID="genid55"/>
        <prov:definition>influencer: an identifier (o1) for an ancestor entity, activity, or agent that the former depends on;</prov:definition>
        <prov:dm>http://www.w3.org/TR/2013/REC-prov-dm-20130430/#term-influence</prov:dm>
    </owl:Axiom>
    


    <!-- http://www.w3.org/ns/prov#wasInformedBy -->

    <owl:ObjectProperty rdf:about="http://www.w3.org/ns/prov#wasInformedBy">
        <rdfs:subPropertyOf rdf:resource="http://www.w3.org/ns/prov#wasInfluencedBy"/>
        <rdfs:domain rdf:resource="http://www.w3.org/ns/prov#Activity"/>
        <rdfs:range rdf:resource="http://www.w3.org/ns/prov#Activity"/>
        <owl:propertyChainAxiom rdf:parseType="Collection">
            <rdf:Description rdf:about="http://www.w3.org/ns/prov#qualifiedCommunication"/>
            <rdf:Description rdf:about="http://www.w3.org/ns/prov#activity"/>
        </owl:propertyChainAxiom>
        <rdfs:comment xml:lang="en">An activity a2 is dependent on or informed by another activity a1, by way of some unspecified entity that is generated by a1 and used by a2.</rdfs:comment>
        <rdfs:isDefinedBy rdf:resource="http://www.w3.org/ns/prov-o#"/>
        <rdfs:label>wasInformedBy</rdfs:label>
        <prov:category>starting-point</prov:category>
        <prov:component>entities-activities</prov:component>
        <prov:inverse>informed</prov:inverse>
        <prov:qualifiedForm rdf:resource="http://www.w3.org/ns/prov#Communication"/>
        <prov:qualifiedForm rdf:resource="http://www.w3.org/ns/prov#qualifiedCommunication"/>
    </owl:ObjectProperty>
    


    <!-- http://www.w3.org/ns/prov#wasInvalidatedBy -->

    <owl:ObjectProperty rdf:about="http://www.w3.org/ns/prov#wasInvalidatedBy">
        <rdfs:subPropertyOf rdf:resource="http://www.w3.org/ns/prov#wasInfluencedBy"/>
        <rdfs:domain rdf:resource="http://www.w3.org/ns/prov#Entity"/>
        <rdfs:range rdf:resource="http://www.w3.org/ns/prov#Activity"/>
        <owl:propertyChainAxiom rdf:parseType="Collection">
            <rdf:Description rdf:about="http://www.w3.org/ns/prov#qualifiedInvalidation"/>
            <rdf:Description rdf:about="http://www.w3.org/ns/prov#activity"/>
        </owl:propertyChainAxiom>
        <rdfs:isDefinedBy rdf:resource="http://www.w3.org/ns/prov-o#"/>
        <rdfs:label>wasInvalidatedBy</rdfs:label>
        <prov:category>expanded</prov:category>
        <prov:component>entities-activities</prov:component>
        <prov:inverse>invalidated</prov:inverse>
        <prov:qualifiedForm rdf:resource="http://www.w3.org/ns/prov#Invalidation"/>
        <prov:qualifiedForm rdf:resource="http://www.w3.org/ns/prov#qualifiedInvalidation"/>
    </owl:ObjectProperty>
    


    <!-- http://www.w3.org/ns/prov#wasQuotedFrom -->

    <owl:ObjectProperty rdf:about="http://www.w3.org/ns/prov#wasQuotedFrom">
        <rdfs:subPropertyOf rdf:resource="http://www.w3.org/ns/prov#wasDerivedFrom"/>
        <rdfs:domain rdf:resource="http://www.w3.org/ns/prov#Entity"/>
        <rdfs:range rdf:resource="http://www.w3.org/ns/prov#Entity"/>
        <owl:propertyChainAxiom rdf:parseType="Collection">
            <rdf:Description rdf:about="http://www.w3.org/ns/prov#qualifiedQuotation"/>
            <rdf:Description rdf:about="http://www.w3.org/ns/prov#entity"/>
        </owl:propertyChainAxiom>
        <rdfs:comment xml:lang="en">An entity is derived from an original entity by copying, or &apos;quoting&apos;, some or all of it.</rdfs:comment>
        <rdfs:isDefinedBy rdf:resource="http://www.w3.org/ns/prov-o#"/>
        <rdfs:label>wasQuotedFrom</rdfs:label>
        <prov:category>expanded</prov:category>
        <prov:component>derivations</prov:component>
        <prov:inverse>quotedAs</prov:inverse>
        <prov:qualifiedForm rdf:resource="http://www.w3.org/ns/prov#Quotation"/>
        <prov:qualifiedForm rdf:resource="http://www.w3.org/ns/prov#qualifiedQuotation"/>
    </owl:ObjectProperty>
    <owl:Axiom>
        <owl:annotatedSource rdf:resource="http://www.w3.org/ns/prov#wasQuotedFrom"/>
        <owl:annotatedProperty rdf:resource="http://www.w3.org/2000/01/rdf-schema#subPropertyOf"/>
        <owl:annotatedTarget rdf:resource="http://www.w3.org/ns/prov#wasDerivedFrom"/>
        <rdfs:comment>Quotation is a particular case of derivation (see http://www.w3.org/TR/prov-dm/#term-quotation) in which an entity is derived from an original entity by copying, or &quot;quoting&quot;, some or all of it. </rdfs:comment>
    </owl:Axiom>
    


    <!-- http://www.w3.org/ns/prov#wasRevisionOf -->

    <owl:ObjectProperty rdf:about="http://www.w3.org/ns/prov#wasRevisionOf">
        <rdfs:subPropertyOf rdf:resource="http://www.w3.org/ns/prov#wasDerivedFrom"/>
        <rdfs:domain rdf:resource="http://www.w3.org/ns/prov#Entity"/>
        <owl:propertyChainAxiom rdf:parseType="Collection">
            <rdf:Description rdf:about="http://www.w3.org/ns/prov#qualifiedRevision"/>
            <rdf:Description rdf:about="http://www.w3.org/ns/prov#entity"/>
        </owl:propertyChainAxiom>
    </owl:ObjectProperty>
    <owl:Axiom>
        <owl:annotatedSource rdf:resource="http://www.w3.org/ns/prov#wasRevisionOf"/>
        <owl:annotatedProperty rdf:resource="http://www.w3.org/2000/01/rdf-schema#subPropertyOf"/>
        <owl:annotatedTarget rdf:resource="http://www.w3.org/ns/prov#wasDerivedFrom"/>
        <rdfs:comment>Revision is a derivation (see http://www.w3.org/TR/prov-dm/#term-Revision). Moreover, according to 
http://www.w3.org/TR/2013/REC-prov-constraints-20130430/#term-Revision 23 April 2012 &apos;wasRevisionOf is a strict sub-relation of wasDerivedFrom since two entities e2 and e1 may satisfy wasDerivedFrom(e2,e1) without being a variant of each other.&apos;</rdfs:comment>
    </owl:Axiom>
    


    <!-- http://www.w3.org/ns/prov#wasStartedBy -->

    <owl:ObjectProperty rdf:about="http://www.w3.org/ns/prov#wasStartedBy">
        <rdfs:subPropertyOf rdf:resource="http://www.w3.org/ns/prov#wasInfluencedBy"/>
        <rdfs:domain rdf:resource="http://www.w3.org/ns/prov#Activity"/>
        <rdfs:range rdf:resource="http://www.w3.org/ns/prov#Entity"/>
        <owl:propertyChainAxiom rdf:parseType="Collection">
            <rdf:Description rdf:about="http://www.w3.org/ns/prov#qualifiedStart"/>
            <rdf:Description rdf:about="http://www.w3.org/ns/prov#entity"/>
        </owl:propertyChainAxiom>
        <rdfs:comment xml:lang="en">Start is when an activity is deemed to have started. A start may refer to an entity, known as trigger, that initiated the activity.</rdfs:comment>
        <rdfs:isDefinedBy rdf:resource="http://www.w3.org/ns/prov-o#"/>
        <rdfs:label>wasStartedBy</rdfs:label>
        <prov:category>expanded</prov:category>
        <prov:component>entities-activities</prov:component>
        <prov:inverse>started</prov:inverse>
        <prov:qualifiedForm rdf:resource="http://www.w3.org/ns/prov#Start"/>
        <prov:qualifiedForm rdf:resource="http://www.w3.org/ns/prov#qualifiedStart"/>
    </owl:ObjectProperty>
    


    <!-- http://xmlns.com/foaf/0.1/account -->

    <owl:ObjectProperty rdf:about="http://xmlns.com/foaf/0.1/account">
        <rdfs:domain rdf:resource="http://xmlns.com/foaf/0.1/Agent"/>
        <rdfs:range rdf:resource="http://xmlns.com/foaf/0.1/OnlineAccount"/>
        <rdfs:comment>Indicates an account held by this agent.</rdfs:comment>
        <rdfs:isDefinedBy rdf:resource="http://xmlns.com/foaf/0.1/"/>
        <rdfs:label>account</rdfs:label>
        <ns:term_status>testing</ns:term_status>
    </owl:ObjectProperty>
    


    <!-- http://xmlns.com/foaf/0.1/accountServiceHomepage -->

    <owl:ObjectProperty rdf:about="http://xmlns.com/foaf/0.1/accountServiceHomepage">
        <rdfs:domain rdf:resource="http://xmlns.com/foaf/0.1/OnlineAccount"/>
        <rdfs:range rdf:resource="http://xmlns.com/foaf/0.1/Document"/>
        <rdfs:comment>Indicates a homepage of the service provide for this online account.</rdfs:comment>
        <rdfs:isDefinedBy rdf:resource="http://xmlns.com/foaf/0.1/"/>
        <rdfs:label>account service homepage</rdfs:label>
        <ns:term_status>testing</ns:term_status>
    </owl:ObjectProperty>
    


    <!-- http://xmlns.com/foaf/0.1/aimChatID -->

    <owl:ObjectProperty rdf:about="http://xmlns.com/foaf/0.1/aimChatID">
        <rdfs:subPropertyOf rdf:resource="http://xmlns.com/foaf/0.1/nick"/>
        <rdf:type rdf:resource="http://www.w3.org/2002/07/owl#InverseFunctionalProperty"/>
        <rdfs:domain rdf:resource="http://xmlns.com/foaf/0.1/Agent"/>
    </owl:ObjectProperty>
    


    <!-- http://xmlns.com/foaf/0.1/based_near -->

    <owl:ObjectProperty rdf:about="http://xmlns.com/foaf/0.1/based_near">
        <rdfs:domain rdf:resource="http://www.w3.org/2003/01/geo/wgs84_pos#SpatialThing"/>
        <rdfs:range rdf:resource="http://www.w3.org/2003/01/geo/wgs84_pos#SpatialThing"/>
        <rdfs:comment>A location that something is based near, for some broadly human notion of near.</rdfs:comment>
        <rdfs:isDefinedBy rdf:resource="http://xmlns.com/foaf/0.1/"/>
        <rdfs:label>based near</rdfs:label>
        <ns:term_status>testing</ns:term_status>
    </owl:ObjectProperty>
    


    <!-- http://xmlns.com/foaf/0.1/currentProject -->

    <owl:ObjectProperty rdf:about="http://xmlns.com/foaf/0.1/currentProject">
        <rdfs:domain rdf:resource="http://xmlns.com/foaf/0.1/Person"/>
        <rdfs:range rdf:resource="http://www.w3.org/2002/07/owl#Thing"/>
        <rdfs:comment>A current project this person works on.</rdfs:comment>
        <rdfs:isDefinedBy rdf:resource="http://xmlns.com/foaf/0.1/"/>
        <rdfs:label>current project</rdfs:label>
        <ns:term_status>testing</ns:term_status>
    </owl:ObjectProperty>
    


    <!-- http://xmlns.com/foaf/0.1/depiction -->

    <owl:ObjectProperty rdf:about="http://xmlns.com/foaf/0.1/depiction">
        <owl:inverseOf rdf:resource="http://xmlns.com/foaf/0.1/depicts"/>
        <rdfs:domain rdf:resource="http://www.w3.org/2002/07/owl#Thing"/>
        <rdfs:range rdf:resource="http://xmlns.com/foaf/0.1/Image"/>
        <rdfs:comment>A depiction of some thing.</rdfs:comment>
        <rdfs:isDefinedBy rdf:resource="http://xmlns.com/foaf/0.1/"/>
        <rdfs:label>depiction</rdfs:label>
        <ns:term_status>testing</ns:term_status>
    </owl:ObjectProperty>
    


    <!-- http://xmlns.com/foaf/0.1/depicts -->

    <owl:ObjectProperty rdf:about="http://xmlns.com/foaf/0.1/depicts">
        <rdfs:domain rdf:resource="http://xmlns.com/foaf/0.1/Image"/>
        <rdfs:range rdf:resource="http://www.w3.org/2002/07/owl#Thing"/>
        <rdfs:comment>A thing depicted in this representation.</rdfs:comment>
        <rdfs:isDefinedBy rdf:resource="http://xmlns.com/foaf/0.1/"/>
        <rdfs:label>depicts</rdfs:label>
        <ns:term_status>testing</ns:term_status>
    </owl:ObjectProperty>
    


    <!-- http://xmlns.com/foaf/0.1/focus -->

    <owl:ObjectProperty rdf:about="http://xmlns.com/foaf/0.1/focus">
        <rdfs:domain rdf:resource="http://www.w3.org/2004/02/skos/core#Concept"/>
        <rdfs:range rdf:resource="http://www.w3.org/2002/07/owl#Thing"/>
        <rdfs:comment>The underlying or &apos;focal&apos; entity associated with some SKOS-described concept.</rdfs:comment>
        <rdfs:isDefinedBy rdf:resource="http://xmlns.com/foaf/0.1/"/>
        <rdfs:label>focus</rdfs:label>
        <ns:term_status>testing</ns:term_status>
    </owl:ObjectProperty>
    


    <!-- http://xmlns.com/foaf/0.1/fundedBy -->

    <owl:ObjectProperty rdf:about="http://xmlns.com/foaf/0.1/fundedBy">
        <rdfs:domain rdf:resource="http://www.w3.org/2002/07/owl#Thing"/>
        <rdfs:range rdf:resource="http://www.w3.org/2002/07/owl#Thing"/>
        <rdfs:comment>An organization funding a project or person.</rdfs:comment>
        <rdfs:isDefinedBy rdf:resource="http://xmlns.com/foaf/0.1/"/>
        <rdfs:label>funded by</rdfs:label>
        <ns:term_status>archaic</ns:term_status>
    </owl:ObjectProperty>
    


    <!-- http://xmlns.com/foaf/0.1/holdsAccount -->

    <owl:ObjectProperty rdf:about="http://xmlns.com/foaf/0.1/holdsAccount">
        <rdfs:domain rdf:resource="http://xmlns.com/foaf/0.1/Agent"/>
        <rdfs:range rdf:resource="http://xmlns.com/foaf/0.1/OnlineAccount"/>
        <rdfs:comment>Indicates an account held by this agent.</rdfs:comment>
        <rdfs:isDefinedBy rdf:resource="http://xmlns.com/foaf/0.1/"/>
        <rdfs:label>account</rdfs:label>
        <ns:term_status>archaic</ns:term_status>
    </owl:ObjectProperty>
    


    <!-- http://xmlns.com/foaf/0.1/homepage -->

    <owl:ObjectProperty rdf:about="http://xmlns.com/foaf/0.1/homepage">
        <rdfs:subPropertyOf rdf:resource="http://xmlns.com/foaf/0.1/isPrimaryTopicOf"/>
        <rdfs:subPropertyOf rdf:resource="http://xmlns.com/foaf/0.1/page"/>
        <rdf:type rdf:resource="http://www.w3.org/2002/07/owl#InverseFunctionalProperty"/>
        <rdfs:domain rdf:resource="http://www.w3.org/2002/07/owl#Thing"/>
        <rdfs:range rdf:resource="http://xmlns.com/foaf/0.1/Document"/>
        <rdfs:comment>A homepage for some thing.</rdfs:comment>
        <rdfs:isDefinedBy rdf:resource="http://xmlns.com/foaf/0.1/"/>
        <rdfs:label>homepage</rdfs:label>
        <ns:term_status>stable</ns:term_status>
    </owl:ObjectProperty>
    


    <!-- http://xmlns.com/foaf/0.1/icqChatID -->

    <owl:ObjectProperty rdf:about="http://xmlns.com/foaf/0.1/icqChatID">
        <rdfs:subPropertyOf rdf:resource="http://xmlns.com/foaf/0.1/nick"/>
        <rdf:type rdf:resource="http://www.w3.org/2002/07/owl#InverseFunctionalProperty"/>
        <rdfs:domain rdf:resource="http://xmlns.com/foaf/0.1/Agent"/>
    </owl:ObjectProperty>
    


    <!-- http://xmlns.com/foaf/0.1/img -->

    <owl:ObjectProperty rdf:about="http://xmlns.com/foaf/0.1/img">
        <rdfs:subPropertyOf rdf:resource="http://xmlns.com/foaf/0.1/depiction"/>
        <rdfs:domain rdf:resource="http://xmlns.com/foaf/0.1/Person"/>
        <rdfs:range rdf:resource="http://xmlns.com/foaf/0.1/Image"/>
        <rdfs:comment>An image that can be used to represent some thing (ie. those depictions which are particularly representative of something, eg. one&apos;s photo on a homepage).</rdfs:comment>
        <rdfs:isDefinedBy rdf:resource="http://xmlns.com/foaf/0.1/"/>
        <rdfs:label>image</rdfs:label>
        <ns:term_status>testing</ns:term_status>
    </owl:ObjectProperty>
    


    <!-- http://xmlns.com/foaf/0.1/interest -->

    <owl:ObjectProperty rdf:about="http://xmlns.com/foaf/0.1/interest">
        <rdfs:domain rdf:resource="http://xmlns.com/foaf/0.1/Agent"/>
        <rdfs:range rdf:resource="http://xmlns.com/foaf/0.1/Document"/>
        <rdfs:comment>A page about a topic of interest to this person.</rdfs:comment>
        <rdfs:isDefinedBy rdf:resource="http://xmlns.com/foaf/0.1/"/>
        <rdfs:label>interest</rdfs:label>
        <ns:term_status>testing</ns:term_status>
    </owl:ObjectProperty>
    


    <!-- http://xmlns.com/foaf/0.1/isPrimaryTopicOf -->

    <owl:ObjectProperty rdf:about="http://xmlns.com/foaf/0.1/isPrimaryTopicOf">
        <rdfs:subPropertyOf rdf:resource="http://xmlns.com/foaf/0.1/page"/>
        <owl:inverseOf rdf:resource="http://xmlns.com/foaf/0.1/primaryTopic"/>
        <rdf:type rdf:resource="http://www.w3.org/2002/07/owl#InverseFunctionalProperty"/>
        <rdfs:domain rdf:resource="http://www.w3.org/2002/07/owl#Thing"/>
        <rdfs:range rdf:resource="http://xmlns.com/foaf/0.1/Document"/>
        <rdfs:comment>A document that this thing is the primary topic of.</rdfs:comment>
        <rdfs:isDefinedBy rdf:resource="http://xmlns.com/foaf/0.1/"/>
        <rdfs:label>is primary topic of</rdfs:label>
        <ns:term_status>stable</ns:term_status>
    </owl:ObjectProperty>
    


    <!-- http://xmlns.com/foaf/0.1/jabberID -->

    <owl:ObjectProperty rdf:about="http://xmlns.com/foaf/0.1/jabberID">
        <rdf:type rdf:resource="http://www.w3.org/2002/07/owl#InverseFunctionalProperty"/>
        <rdfs:domain rdf:resource="http://xmlns.com/foaf/0.1/Agent"/>
    </owl:ObjectProperty>
    


    <!-- http://xmlns.com/foaf/0.1/knows -->

    <owl:ObjectProperty rdf:about="http://xmlns.com/foaf/0.1/knows">
        <rdfs:domain rdf:resource="http://xmlns.com/foaf/0.1/Person"/>
        <rdfs:range rdf:resource="http://xmlns.com/foaf/0.1/Person"/>
        <rdfs:comment>A person known by this person (indicating some level of reciprocated interaction between the parties).</rdfs:comment>
        <rdfs:isDefinedBy rdf:resource="http://xmlns.com/foaf/0.1/"/>
        <rdfs:label>knows</rdfs:label>
        <ns:term_status>stable</ns:term_status>
    </owl:ObjectProperty>
    


    <!-- http://xmlns.com/foaf/0.1/logo -->

    <owl:ObjectProperty rdf:about="http://xmlns.com/foaf/0.1/logo">
        <rdf:type rdf:resource="http://www.w3.org/2002/07/owl#InverseFunctionalProperty"/>
        <rdfs:domain rdf:resource="http://www.w3.org/2002/07/owl#Thing"/>
        <rdfs:range rdf:resource="http://www.w3.org/2002/07/owl#Thing"/>
        <rdfs:comment>A logo representing some thing.</rdfs:comment>
        <rdfs:isDefinedBy rdf:resource="http://xmlns.com/foaf/0.1/"/>
        <rdfs:label>logo</rdfs:label>
        <ns:term_status>testing</ns:term_status>
    </owl:ObjectProperty>
    


    <!-- http://xmlns.com/foaf/0.1/made -->

    <owl:ObjectProperty rdf:about="http://xmlns.com/foaf/0.1/made">
        <owl:inverseOf rdf:resource="http://xmlns.com/foaf/0.1/maker"/>
        <rdfs:domain rdf:resource="http://xmlns.com/foaf/0.1/Agent"/>
        <rdfs:range rdf:resource="http://www.w3.org/2002/07/owl#Thing"/>
        <rdfs:comment>Something that was made by this agent.</rdfs:comment>
        <rdfs:isDefinedBy rdf:resource="http://xmlns.com/foaf/0.1/"/>
        <rdfs:label>made</rdfs:label>
        <ns:term_status>stable</ns:term_status>
    </owl:ObjectProperty>
    


    <!-- http://xmlns.com/foaf/0.1/maker -->

    <owl:ObjectProperty rdf:about="http://xmlns.com/foaf/0.1/maker">
        <rdfs:domain rdf:resource="http://www.w3.org/2002/07/owl#Thing"/>
        <rdfs:range rdf:resource="http://xmlns.com/foaf/0.1/Agent"/>
        <rdfs:comment>An agent that  made this thing.</rdfs:comment>
        <rdfs:isDefinedBy rdf:resource="http://xmlns.com/foaf/0.1/"/>
        <rdfs:label>maker</rdfs:label>
        <ns:term_status>stable</ns:term_status>
    </owl:ObjectProperty>
    


    <!-- http://xmlns.com/foaf/0.1/mbox -->

    <owl:ObjectProperty rdf:about="http://xmlns.com/foaf/0.1/mbox">
        <rdf:type rdf:resource="http://www.w3.org/2002/07/owl#InverseFunctionalProperty"/>
        <rdfs:domain rdf:resource="http://xmlns.com/foaf/0.1/Agent"/>
        <rdfs:range rdf:resource="http://www.w3.org/2002/07/owl#Thing"/>
        <rdfs:comment>A  personal mailbox, ie. an Internet mailbox associated with exactly one owner, the first owner of this mailbox. This is a &apos;static inverse functional property&apos;, in that  there is (across time and change) at most one individual that ever has any particular value for foaf:mbox.</rdfs:comment>
        <rdfs:isDefinedBy rdf:resource="http://xmlns.com/foaf/0.1/"/>
        <rdfs:label>personal mailbox</rdfs:label>
        <ns:term_status>stable</ns:term_status>
    </owl:ObjectProperty>
    


    <!-- http://xmlns.com/foaf/0.1/member -->

    <owl:ObjectProperty rdf:about="http://xmlns.com/foaf/0.1/member">
        <rdfs:domain rdf:resource="http://xmlns.com/foaf/0.1/Group"/>
        <rdfs:range rdf:resource="http://xmlns.com/foaf/0.1/Agent"/>
        <rdfs:comment>Indicates a member of a Group</rdfs:comment>
        <rdfs:isDefinedBy rdf:resource="http://xmlns.com/foaf/0.1/"/>
        <rdfs:label>member</rdfs:label>
        <ns:term_status>stable</ns:term_status>
    </owl:ObjectProperty>
    


    <!-- http://xmlns.com/foaf/0.1/msnChatID -->

    <owl:ObjectProperty rdf:about="http://xmlns.com/foaf/0.1/msnChatID">
        <rdfs:subPropertyOf rdf:resource="http://xmlns.com/foaf/0.1/nick"/>
        <rdf:type rdf:resource="http://www.w3.org/2002/07/owl#InverseFunctionalProperty"/>
        <rdfs:domain rdf:resource="http://xmlns.com/foaf/0.1/Agent"/>
    </owl:ObjectProperty>
    


    <!-- http://xmlns.com/foaf/0.1/openid -->

    <owl:ObjectProperty rdf:about="http://xmlns.com/foaf/0.1/openid">
        <rdfs:subPropertyOf rdf:resource="http://xmlns.com/foaf/0.1/isPrimaryTopicOf"/>
        <rdf:type rdf:resource="http://www.w3.org/2002/07/owl#InverseFunctionalProperty"/>
        <rdfs:domain rdf:resource="http://xmlns.com/foaf/0.1/Agent"/>
        <rdfs:range rdf:resource="http://xmlns.com/foaf/0.1/Document"/>
        <rdfs:comment>An OpenID for an Agent.</rdfs:comment>
        <rdfs:isDefinedBy rdf:resource="http://xmlns.com/foaf/0.1/"/>
        <rdfs:label>openid</rdfs:label>
        <ns:term_status>testing</ns:term_status>
    </owl:ObjectProperty>
    


    <!-- http://xmlns.com/foaf/0.1/page -->

    <owl:ObjectProperty rdf:about="http://xmlns.com/foaf/0.1/page">
        <owl:inverseOf rdf:resource="http://xmlns.com/foaf/0.1/topic"/>
        <rdfs:domain rdf:resource="http://www.w3.org/2002/07/owl#Thing"/>
        <rdfs:range rdf:resource="http://xmlns.com/foaf/0.1/Document"/>
        <rdfs:comment>A page or document about this thing.</rdfs:comment>
        <rdfs:isDefinedBy rdf:resource="http://xmlns.com/foaf/0.1/"/>
        <rdfs:label>page</rdfs:label>
        <ns:term_status>stable</ns:term_status>
    </owl:ObjectProperty>
    


    <!-- http://xmlns.com/foaf/0.1/pastProject -->

    <owl:ObjectProperty rdf:about="http://xmlns.com/foaf/0.1/pastProject">
        <rdfs:domain rdf:resource="http://xmlns.com/foaf/0.1/Person"/>
        <rdfs:range rdf:resource="http://www.w3.org/2002/07/owl#Thing"/>
        <rdfs:comment>A project this person has previously worked on.</rdfs:comment>
        <rdfs:isDefinedBy rdf:resource="http://xmlns.com/foaf/0.1/"/>
        <rdfs:label>past project</rdfs:label>
        <ns:term_status>testing</ns:term_status>
    </owl:ObjectProperty>
    


    <!-- http://xmlns.com/foaf/0.1/phone -->

    <owl:ObjectProperty rdf:about="http://xmlns.com/foaf/0.1/phone">
        <rdfs:comment>A phone,  specified using fully qualified tel: URI scheme (refs: http://www.w3.org/Addressing/schemes.html#tel).</rdfs:comment>
        <rdfs:isDefinedBy rdf:resource="http://xmlns.com/foaf/0.1/"/>
        <rdfs:label>phone</rdfs:label>
        <ns:term_status>testing</ns:term_status>
    </owl:ObjectProperty>
    


    <!-- http://xmlns.com/foaf/0.1/primaryTopic -->

    <owl:ObjectProperty rdf:about="http://xmlns.com/foaf/0.1/primaryTopic">
        <rdf:type rdf:resource="http://www.w3.org/2002/07/owl#FunctionalProperty"/>
        <rdfs:domain rdf:resource="http://xmlns.com/foaf/0.1/Document"/>
        <rdfs:range rdf:resource="http://www.w3.org/2002/07/owl#Thing"/>
        <rdfs:comment>The primary topic of some page or document.</rdfs:comment>
        <rdfs:isDefinedBy rdf:resource="http://xmlns.com/foaf/0.1/"/>
        <rdfs:label>primary topic</rdfs:label>
        <ns:term_status>stable</ns:term_status>
    </owl:ObjectProperty>
    


    <!-- http://xmlns.com/foaf/0.1/publications -->

    <owl:ObjectProperty rdf:about="http://xmlns.com/foaf/0.1/publications">
        <rdfs:domain rdf:resource="http://xmlns.com/foaf/0.1/Person"/>
        <rdfs:range rdf:resource="http://rdfs.org/ns/void#Dataset"/>
        <rdfs:range rdf:resource="http://xmlns.com/foaf/0.1/Document"/>
        <rdfs:comment>A link to the publications of this person.</rdfs:comment>
        <rdfs:isDefinedBy rdf:resource="http://xmlns.com/foaf/0.1/"/>
        <rdfs:label>publications</rdfs:label>
        <ns:term_status>testing</ns:term_status>
    </owl:ObjectProperty>
    


    <!-- http://xmlns.com/foaf/0.1/schoolHomepage -->

    <owl:ObjectProperty rdf:about="http://xmlns.com/foaf/0.1/schoolHomepage">
        <rdfs:domain rdf:resource="http://xmlns.com/foaf/0.1/Person"/>
        <rdfs:range rdf:resource="http://xmlns.com/foaf/0.1/Document"/>
        <rdfs:comment>A homepage of a school attended by the person.</rdfs:comment>
        <rdfs:isDefinedBy rdf:resource="http://xmlns.com/foaf/0.1/"/>
        <rdfs:label>schoolHomepage</rdfs:label>
        <ns:term_status>testing</ns:term_status>
    </owl:ObjectProperty>
    


    <!-- http://xmlns.com/foaf/0.1/skypeID -->

    <owl:ObjectProperty rdf:about="http://xmlns.com/foaf/0.1/skypeID">
        <rdfs:subPropertyOf rdf:resource="http://xmlns.com/foaf/0.1/nick"/>
        <rdfs:domain rdf:resource="http://xmlns.com/foaf/0.1/Agent"/>
    </owl:ObjectProperty>
    


    <!-- http://xmlns.com/foaf/0.1/theme -->

    <owl:ObjectProperty rdf:about="http://xmlns.com/foaf/0.1/theme">
        <rdfs:domain rdf:resource="http://www.w3.org/2002/07/owl#Thing"/>
        <rdfs:range rdf:resource="http://www.w3.org/2002/07/owl#Thing"/>
        <rdfs:comment>A theme.</rdfs:comment>
        <rdfs:isDefinedBy rdf:resource="http://xmlns.com/foaf/0.1/"/>
        <rdfs:label>theme</rdfs:label>
        <ns:term_status>archaic</ns:term_status>
    </owl:ObjectProperty>
    


    <!-- http://xmlns.com/foaf/0.1/thumbnail -->

    <owl:ObjectProperty rdf:about="http://xmlns.com/foaf/0.1/thumbnail">
        <rdfs:domain rdf:resource="http://xmlns.com/foaf/0.1/Image"/>
        <rdfs:range rdf:resource="http://xmlns.com/foaf/0.1/Image"/>
        <rdfs:comment>A derived thumbnail image.</rdfs:comment>
        <rdfs:isDefinedBy rdf:resource="http://xmlns.com/foaf/0.1/"/>
        <rdfs:label>thumbnail</rdfs:label>
        <ns:term_status>testing</ns:term_status>
    </owl:ObjectProperty>
    


    <!-- http://xmlns.com/foaf/0.1/tipjar -->

    <owl:ObjectProperty rdf:about="http://xmlns.com/foaf/0.1/tipjar">
        <rdfs:subPropertyOf rdf:resource="http://xmlns.com/foaf/0.1/page"/>
        <rdfs:domain rdf:resource="http://xmlns.com/foaf/0.1/Agent"/>
        <rdfs:range rdf:resource="http://xmlns.com/foaf/0.1/Document"/>
        <rdfs:comment>A tipjar document for this agent, describing means for payment and reward.</rdfs:comment>
        <rdfs:isDefinedBy rdf:resource="http://xmlns.com/foaf/0.1/"/>
        <rdfs:label>tipjar</rdfs:label>
        <ns:term_status>testing</ns:term_status>
    </owl:ObjectProperty>
    


    <!-- http://xmlns.com/foaf/0.1/topic -->

    <owl:ObjectProperty rdf:about="http://xmlns.com/foaf/0.1/topic">
        <rdfs:domain rdf:resource="http://xmlns.com/foaf/0.1/Document"/>
        <rdfs:range rdf:resource="http://www.w3.org/2002/07/owl#Thing"/>
        <rdfs:comment>A topic of some page or document.</rdfs:comment>
        <rdfs:isDefinedBy rdf:resource="http://xmlns.com/foaf/0.1/"/>
        <rdfs:label>topic</rdfs:label>
        <ns:term_status>testing</ns:term_status>
    </owl:ObjectProperty>
    


    <!-- http://xmlns.com/foaf/0.1/topic_interest -->

    <owl:ObjectProperty rdf:about="http://xmlns.com/foaf/0.1/topic_interest">
        <rdfs:domain rdf:resource="http://xmlns.com/foaf/0.1/Agent"/>
        <rdfs:range rdf:resource="http://www.w3.org/2002/07/owl#Thing"/>
        <rdfs:comment>A thing of interest to this person.</rdfs:comment>
        <rdfs:isDefinedBy rdf:resource="http://xmlns.com/foaf/0.1/"/>
        <rdfs:label>topic_interest</rdfs:label>
        <ns:term_status>testing</ns:term_status>
    </owl:ObjectProperty>
    


    <!-- http://xmlns.com/foaf/0.1/weblog -->

    <owl:ObjectProperty rdf:about="http://xmlns.com/foaf/0.1/weblog">
        <rdfs:subPropertyOf rdf:resource="http://xmlns.com/foaf/0.1/page"/>
        <rdf:type rdf:resource="http://www.w3.org/2002/07/owl#InverseFunctionalProperty"/>
        <rdfs:domain rdf:resource="http://xmlns.com/foaf/0.1/Agent"/>
        <rdfs:range rdf:resource="http://xmlns.com/foaf/0.1/Document"/>
        <rdfs:comment>A weblog of some thing (whether person, group, company etc.).</rdfs:comment>
        <rdfs:isDefinedBy rdf:resource="http://xmlns.com/foaf/0.1/"/>
        <rdfs:label>weblog</rdfs:label>
        <ns:term_status>stable</ns:term_status>
    </owl:ObjectProperty>
    


    <!-- http://xmlns.com/foaf/0.1/workInfoHomepage -->

    <owl:ObjectProperty rdf:about="http://xmlns.com/foaf/0.1/workInfoHomepage">
        <rdfs:domain rdf:resource="http://xmlns.com/foaf/0.1/Person"/>
        <rdfs:range rdf:resource="http://xmlns.com/foaf/0.1/Document"/>
        <rdfs:comment>A work info homepage of some person; a page about their work for some organization.</rdfs:comment>
        <rdfs:isDefinedBy rdf:resource="http://xmlns.com/foaf/0.1/"/>
        <rdfs:label>work info homepage</rdfs:label>
        <ns:term_status>testing</ns:term_status>
    </owl:ObjectProperty>
    


    <!-- http://xmlns.com/foaf/0.1/workplaceHomepage -->

    <owl:ObjectProperty rdf:about="http://xmlns.com/foaf/0.1/workplaceHomepage">
        <rdfs:domain rdf:resource="http://xmlns.com/foaf/0.1/Person"/>
        <rdfs:range rdf:resource="http://xmlns.com/foaf/0.1/Document"/>
        <rdfs:comment>A workplace homepage of some person; the homepage of an organization they work for.</rdfs:comment>
        <rdfs:isDefinedBy rdf:resource="http://xmlns.com/foaf/0.1/"/>
        <rdfs:label>workplace homepage</rdfs:label>
        <ns:term_status>testing</ns:term_status>
    </owl:ObjectProperty>
    


    <!-- http://xmlns.com/foaf/0.1/yahooChatID -->

    <owl:ObjectProperty rdf:about="http://xmlns.com/foaf/0.1/yahooChatID">
        <rdfs:subPropertyOf rdf:resource="http://xmlns.com/foaf/0.1/nick"/>
        <rdf:type rdf:resource="http://www.w3.org/2002/07/owl#InverseFunctionalProperty"/>
        <rdfs:domain rdf:resource="http://xmlns.com/foaf/0.1/Agent"/>
    </owl:ObjectProperty>
    


    <!-- 
    ///////////////////////////////////////////////////////////////////////////////////////
    //
    // Data properties
    //
    ///////////////////////////////////////////////////////////////////////////////////////
     -->

    


    <!-- http://rdfs.org/ns/void#classes -->

    <owl:DatatypeProperty rdf:about="http://rdfs.org/ns/void#classes">
        <rdfs:domain rdf:resource="http://rdfs.org/ns/void#Dataset"/>
        <rdfs:range rdf:resource="http://www.w3.org/2001/XMLSchema#integer"/>
        <rdfs:comment>The total number of distinct classes in a void:Dataset. In other words, the number of distinct resources occuring as objects of rdf:type triples in the dataset.</rdfs:comment>
        <rdfs:label>classes</rdfs:label>
    </owl:DatatypeProperty>
    


    <!-- http://rdfs.org/ns/void#distinctObjects -->

    <owl:DatatypeProperty rdf:about="http://rdfs.org/ns/void#distinctObjects">
        <rdfs:domain rdf:resource="http://rdfs.org/ns/void#Dataset"/>
        <rdfs:range rdf:resource="http://www.w3.org/2001/XMLSchema#integer"/>
        <rdfs:comment>The total number of distinct objects in a void:Dataset. In other words, the number of distinct resources that occur in the object position of triples in the dataset. Literals are included in this count.</rdfs:comment>
        <rdfs:label>distinct objects</rdfs:label>
    </owl:DatatypeProperty>
    


    <!-- http://rdfs.org/ns/void#distinctSubjects -->

    <owl:DatatypeProperty rdf:about="http://rdfs.org/ns/void#distinctSubjects">
        <rdfs:domain rdf:resource="http://rdfs.org/ns/void#Dataset"/>
        <rdfs:range rdf:resource="http://www.w3.org/2001/XMLSchema#integer"/>
        <rdfs:comment>The total number of distinct subjects in a void:Dataset. In other words, the number of distinct resources that occur in the subject position of triples in the dataset.</rdfs:comment>
        <rdfs:label>distinct subjects</rdfs:label>
    </owl:DatatypeProperty>
    


    <!-- http://rdfs.org/ns/void#documents -->

    <owl:DatatypeProperty rdf:about="http://rdfs.org/ns/void#documents">
        <rdfs:domain rdf:resource="http://rdfs.org/ns/void#Dataset"/>
        <rdfs:range rdf:resource="http://www.w3.org/2001/XMLSchema#integer"/>
        <rdfs:comment>The total number of documents, for datasets that are published as a set of individual documents, such as RDF/XML documents or RDFa-annotated web pages. Non-RDF documents, such as web pages in HTML or images, are usually not included in this count. This property is intended for datasets where the total number of triples or entities is hard to determine. void:triples or void:entities should be preferred where practical.</rdfs:comment>
        <rdfs:label>number of documents</rdfs:label>
    </owl:DatatypeProperty>
    


    <!-- http://rdfs.org/ns/void#entities -->

    <owl:DatatypeProperty rdf:about="http://rdfs.org/ns/void#entities">
        <rdfs:domain rdf:resource="http://rdfs.org/ns/void#Dataset"/>
        <rdfs:range rdf:resource="http://www.w3.org/2001/XMLSchema#integer"/>
        <rdfs:comment>The total number of entities that are described in a void:Dataset.</rdfs:comment>
        <rdfs:label>number of entities</rdfs:label>
    </owl:DatatypeProperty>
    


    <!-- http://rdfs.org/ns/void#properties -->

    <owl:DatatypeProperty rdf:about="http://rdfs.org/ns/void#properties">
        <rdfs:domain rdf:resource="http://rdfs.org/ns/void#Dataset"/>
        <rdfs:range rdf:resource="http://www.w3.org/2001/XMLSchema#integer"/>
        <rdfs:comment>The total number of distinct properties in a void:Dataset. In other words, the number of distinct resources that occur in the predicate position of triples in the dataset.</rdfs:comment>
        <rdfs:label>number of properties</rdfs:label>
    </owl:DatatypeProperty>
    


    <!-- http://rdfs.org/ns/void#triples -->

    <owl:DatatypeProperty rdf:about="http://rdfs.org/ns/void#triples">
        <rdfs:domain rdf:resource="http://rdfs.org/ns/void#Dataset"/>
        <rdfs:range rdf:resource="http://www.w3.org/2001/XMLSchema#integer"/>
        <rdfs:comment>The total number of triples contained in a void:Dataset.</rdfs:comment>
        <rdfs:label>number of triples</rdfs:label>
    </owl:DatatypeProperty>
    


    <!-- http://rdfs.org/ns/void#uriSpace -->

    <owl:DatatypeProperty rdf:about="http://rdfs.org/ns/void#uriSpace">
        <rdfs:domain rdf:resource="http://rdfs.org/ns/void#Dataset"/>
        <rdfs:range rdf:resource="http://www.w3.org/2000/01/rdf-schema#Literal"/>
        <rdfs:comment>A URI that is a common string prefix of all the entity URIs in a void:Dataset.</rdfs:comment>
        <rdfs:label>URI space</rdfs:label>
    </owl:DatatypeProperty>
    


    <!-- http://www.semanticweb.org/k_mil/ontologies/2021/8/EvalLOD#hasLicense -->

    <owl:DatatypeProperty rdf:about="http://www.semanticweb.org/k_mil/ontologies/2021/8/EvalLOD#hasLicense">
        <rdfs:domain rdf:resource="http://rdfs.org/ns/void#Dataset"/>
        <rdfs:range rdf:resource="http://www.w3.org/2001/XMLSchema#int"/>
    </owl:DatatypeProperty>
    


    <!-- http://www.semanticweb.org/k_mil/ontologies/2021/8/EvalLOD#hasProvenance -->

    <owl:DatatypeProperty rdf:about="http://www.semanticweb.org/k_mil/ontologies/2021/8/EvalLOD#hasProvenance">
        <rdfs:domain rdf:resource="http://rdfs.org/ns/void#Dataset"/>
        <rdfs:range rdf:resource="http://www.w3.org/2001/XMLSchema#int"/>
    </owl:DatatypeProperty>
    


    <!-- http://www.semanticweb.org/k_mil/ontologies/2021/8/EvalLOD#isTrusworthy -->

    <owl:DatatypeProperty rdf:about="http://www.semanticweb.org/k_mil/ontologies/2021/8/EvalLOD#isTrusworthy">
        <rdfs:domain rdf:resource="http://rdfs.org/ns/void#Dataset"/>
        <rdfs:range rdf:resource="http://www.w3.org/2001/XMLSchema#int"/>
    </owl:DatatypeProperty>
    


    <!-- http://www.semanticweb.org/k_mil/ontologies/2021/8/EvalLOD#isVerifiable -->

    <owl:DatatypeProperty rdf:about="http://www.semanticweb.org/k_mil/ontologies/2021/8/EvalLOD#isVerifiable">
        <rdfs:domain rdf:resource="http://rdfs.org/ns/void#Dataset"/>
        <rdfs:range rdf:resource="http://www.w3.org/2001/XMLSchema#int"/>
    </owl:DatatypeProperty>
    


    <!-- http://www.semanticweb.org/k_mil/ontologies/2021/8/EvalLOD#reputationScore -->

    <owl:DatatypeProperty rdf:about="http://www.semanticweb.org/k_mil/ontologies/2021/8/EvalLOD#reputationScore">
        <rdfs:subPropertyOf rdf:resource="http://www.w3.org/2002/07/owl#topDataProperty"/>
        <rdfs:domain rdf:resource="http://rdfs.org/ns/void#Dataset"/>
        <rdfs:range rdf:resource="http://www.w3.org/2001/XMLSchema#int"/>
    </owl:DatatypeProperty>
    


    <!-- http://www.w3.org/ns/oa#bodyValue -->

    <rdf:Description rdf:about="http://www.w3.org/ns/oa#bodyValue">
        <rdfs:domain rdf:resource="http://www.w3.org/ns/oa#Annotation"/>
        <rdfs:range rdf:resource="http://www.w3.org/2001/XMLSchema#string"/>
        <rdfs:comment>The object of the predicate is a plain text string to be used as the content of the body of the Annotation.  The value MUST be an  xsd:string  and that data type MUST NOT be expressed in the serialization. Note that language MUST NOT be associated with the value either as a language tag, as that is only available for  rdf:langString .
  </rdfs:comment>
        <rdfs:isDefinedBy rdf:resource="http://www.w3.org/ns/oa#"/>
        <rdfs:label>bodyValue</rdfs:label>
    </rdf:Description>
    


    <!-- http://www.w3.org/ns/oa#end -->

    <rdf:Description rdf:about="http://www.w3.org/ns/oa#end">
        <rdfs:range rdf:resource="http://www.w3.org/2001/XMLSchema#nonNegativeInteger"/>
        <rdfs:comment>The end property is used to convey the 0-based index of the end position of a range of content.</rdfs:comment>
        <rdfs:isDefinedBy rdf:resource="http://www.w3.org/ns/oa#"/>
        <rdfs:label>end</rdfs:label>
    </rdf:Description>
    


    <!-- http://www.w3.org/ns/oa#exact -->

    <rdf:Description rdf:about="http://www.w3.org/ns/oa#exact">
        <rdfs:range rdf:resource="http://www.w3.org/2001/XMLSchema#string"/>
        <rdfs:comment>The object of the predicate is a copy of the text which is being selected, after normalization.</rdfs:comment>
        <rdfs:isDefinedBy rdf:resource="http://www.w3.org/ns/oa#"/>
        <rdfs:label>exact</rdfs:label>
    </rdf:Description>
    


    <!-- http://www.w3.org/ns/oa#prefix -->

    <rdf:Description rdf:about="http://www.w3.org/ns/oa#prefix">
        <rdfs:range rdf:resource="http://www.w3.org/2001/XMLSchema#string"/>
        <rdfs:comment>The object of the property is a snippet of content that occurs immediately before the content which is being selected by the Selector.</rdfs:comment>
        <rdfs:isDefinedBy rdf:resource="http://www.w3.org/ns/oa#"/>
        <rdfs:label>prefix</rdfs:label>
    </rdf:Description>
    


    <!-- http://www.w3.org/ns/oa#processingLanguage -->

    <rdf:Description rdf:about="http://www.w3.org/ns/oa#processingLanguage">
        <rdfs:range rdf:resource="http://www.w3.org/2001/XMLSchema#string"/>
        <rdfs:comment>The object of the property is the language that should be used for textual processing algorithms when dealing with the content of the resource, including hyphenation, line breaking, which font to use for rendering and so forth.  The value must follow the recommendations of BCP47.</rdfs:comment>
        <rdfs:isDefinedBy rdf:resource="http://www.w3.org/ns/oa#"/>
        <rdfs:label>processingLanguage</rdfs:label>
    </rdf:Description>
    


    <!-- http://www.w3.org/ns/oa#sourceDate -->

    <rdf:Description rdf:about="http://www.w3.org/ns/oa#sourceDate">
        <rdfs:domain rdf:resource="http://www.w3.org/ns/oa#TimeState"/>
        <rdfs:range rdf:resource="http://www.w3.org/2001/XMLSchema#dateTime"/>
        <rdfs:comment>The timestamp at which the Source resource should be interpreted as being applicable to the Annotation.</rdfs:comment>
        <rdfs:isDefinedBy rdf:resource="http://www.w3.org/ns/oa#"/>
        <rdfs:label>sourceDate</rdfs:label>
    </rdf:Description>
    


    <!-- http://www.w3.org/ns/oa#sourceDateEnd -->

    <rdf:Description rdf:about="http://www.w3.org/ns/oa#sourceDateEnd">
        <rdfs:domain rdf:resource="http://www.w3.org/ns/oa#TimeState"/>
        <rdfs:range rdf:resource="http://www.w3.org/2001/XMLSchema#dateTime"/>
        <rdfs:comment>The end timestamp of the interval over which the Source resource should be interpreted as being applicable to the Annotation.</rdfs:comment>
        <rdfs:isDefinedBy rdf:resource="http://www.w3.org/ns/oa#"/>
        <rdfs:label>sourceDateEnd</rdfs:label>
    </rdf:Description>
    


    <!-- http://www.w3.org/ns/oa#sourceDateStart -->

    <rdf:Description rdf:about="http://www.w3.org/ns/oa#sourceDateStart">
        <rdfs:domain rdf:resource="http://www.w3.org/ns/oa#TimeState"/>
        <rdfs:range rdf:resource="http://www.w3.org/2001/XMLSchema#dateTime"/>
        <rdfs:comment>The start timestamp of the interval over which the Source resource should be interpreted as being applicable to the Annotation.</rdfs:comment>
        <rdfs:isDefinedBy rdf:resource="http://www.w3.org/ns/oa#"/>
        <rdfs:label>sourceDateStart</rdfs:label>
    </rdf:Description>
    


    <!-- http://www.w3.org/ns/oa#start -->

    <rdf:Description rdf:about="http://www.w3.org/ns/oa#start">
        <rdfs:range rdf:resource="http://www.w3.org/2001/XMLSchema#nonNegativeInteger"/>
        <rdfs:comment>The start position in a 0-based index at which a range of content is selected from the data in the source resource.</rdfs:comment>
        <rdfs:isDefinedBy rdf:resource="http://www.w3.org/ns/oa#"/>
        <rdfs:label>start</rdfs:label>
    </rdf:Description>
    


    <!-- http://www.w3.org/ns/oa#styleClass -->

    <rdf:Description rdf:about="http://www.w3.org/ns/oa#styleClass">
        <rdfs:domain rdf:resource="http://www.w3.org/ns/oa#SpecificResource"/>
        <rdfs:range rdf:resource="http://www.w3.org/2001/XMLSchema#string"/>
        <rdfs:comment>The name of the class used in the CSS description referenced from the Annotation that should be applied to the Specific Resource.</rdfs:comment>
        <rdfs:isDefinedBy rdf:resource="http://www.w3.org/ns/oa#"/>
        <rdfs:label>styleClass</rdfs:label>
    </rdf:Description>
    


    <!-- http://www.w3.org/ns/oa#suffix -->

    <rdf:Description rdf:about="http://www.w3.org/ns/oa#suffix">
        <rdfs:range rdf:resource="http://www.w3.org/2001/XMLSchema#string"/>
        <rdfs:comment>The snippet of text that occurs immediately after the text which is being selected.</rdfs:comment>
        <rdfs:isDefinedBy rdf:resource="http://www.w3.org/ns/oa#"/>
        <rdfs:label>suffix</rdfs:label>
    </rdf:Description>
    


    <!-- http://www.w3.org/ns/prov#atTime -->

    <owl:DatatypeProperty rdf:about="http://www.w3.org/ns/prov#atTime">
        <rdfs:domain rdf:resource="http://www.w3.org/ns/prov#InstantaneousEvent"/>
        <rdfs:range rdf:resource="http://www.w3.org/2001/XMLSchema#dateTime"/>
        <rdfs:comment xml:lang="en">The time at which an InstantaneousEvent occurred, in the form of xsd:dateTime.</rdfs:comment>
        <rdfs:isDefinedBy rdf:resource="http://www.w3.org/ns/prov-o#"/>
        <rdfs:label>atTime</rdfs:label>
        <prov:category>qualified</prov:category>
        <prov:component>entities-activities</prov:component>
        <prov:sharesDefinitionWith rdf:resource="http://www.w3.org/ns/prov#InstantaneousEvent"/>
        <prov:unqualifiedForm rdf:resource="http://www.w3.org/ns/prov#endedAtTime"/>
        <prov:unqualifiedForm rdf:resource="http://www.w3.org/ns/prov#generatedAtTime"/>
        <prov:unqualifiedForm rdf:resource="http://www.w3.org/ns/prov#invalidatedAtTime"/>
        <prov:unqualifiedForm rdf:resource="http://www.w3.org/ns/prov#startedAtTime"/>
    </owl:DatatypeProperty>
    


    <!-- http://www.w3.org/ns/prov#endedAtTime -->

    <owl:DatatypeProperty rdf:about="http://www.w3.org/ns/prov#endedAtTime">
        <rdfs:domain rdf:resource="http://www.w3.org/ns/prov#Activity"/>
        <rdfs:range rdf:resource="http://www.w3.org/2001/XMLSchema#dateTime"/>
        <rdfs:comment xml:lang="en">The time at which an activity ended. See also prov:startedAtTime.</rdfs:comment>
        <rdfs:isDefinedBy rdf:resource="http://www.w3.org/ns/prov-o#"/>
        <rdfs:label>endedAtTime</rdfs:label>
        <prov:category>starting-point</prov:category>
        <prov:component>entities-activities</prov:component>
        <prov:editorialNote xml:lang="en">It is the intent that the property chain holds: (prov:qualifiedEnd o prov:atTime) rdfs:subPropertyOf prov:endedAtTime.</prov:editorialNote>
        <prov:qualifiedForm rdf:resource="http://www.w3.org/ns/prov#End"/>
        <prov:qualifiedForm rdf:resource="http://www.w3.org/ns/prov#atTime"/>
    </owl:DatatypeProperty>
    


    <!-- http://www.w3.org/ns/prov#generatedAtTime -->

    <owl:DatatypeProperty rdf:about="http://www.w3.org/ns/prov#generatedAtTime">
        <rdfs:domain rdf:resource="http://www.w3.org/ns/prov#Entity"/>
        <rdfs:range rdf:resource="http://www.w3.org/2001/XMLSchema#dateTime"/>
        <rdfs:comment xml:lang="en">The time at which an entity was completely created and is available for use.</rdfs:comment>
        <rdfs:isDefinedBy rdf:resource="http://www.w3.org/ns/prov-o#"/>
        <rdfs:label>generatedAtTime</rdfs:label>
        <prov:category>expanded</prov:category>
        <prov:component>entities-activities</prov:component>
        <prov:editorialNote xml:lang="en">It is the intent that the property chain holds: (prov:qualifiedGeneration o prov:atTime) rdfs:subPropertyOf prov:generatedAtTime.</prov:editorialNote>
        <prov:qualifiedForm rdf:resource="http://www.w3.org/ns/prov#Generation"/>
        <prov:qualifiedForm rdf:resource="http://www.w3.org/ns/prov#atTime"/>
    </owl:DatatypeProperty>
    


    <!-- http://www.w3.org/ns/prov#invalidatedAtTime -->

    <owl:DatatypeProperty rdf:about="http://www.w3.org/ns/prov#invalidatedAtTime">
        <rdfs:domain rdf:resource="http://www.w3.org/ns/prov#Entity"/>
        <rdfs:range rdf:resource="http://www.w3.org/2001/XMLSchema#dateTime"/>
        <rdfs:comment xml:lang="en">The time at which an entity was invalidated (i.e., no longer usable).</rdfs:comment>
        <rdfs:isDefinedBy rdf:resource="http://www.w3.org/ns/prov-o#"/>
        <rdfs:label>invalidatedAtTime</rdfs:label>
        <prov:category>expanded</prov:category>
        <prov:component>entities-activities</prov:component>
        <prov:editorialNote xml:lang="en">It is the intent that the property chain holds: (prov:qualifiedInvalidation o prov:atTime) rdfs:subPropertyOf prov:invalidatedAtTime.</prov:editorialNote>
        <prov:qualifiedForm rdf:resource="http://www.w3.org/ns/prov#Invalidation"/>
        <prov:qualifiedForm rdf:resource="http://www.w3.org/ns/prov#atTime"/>
    </owl:DatatypeProperty>
    


    <!-- http://www.w3.org/ns/prov#startedAtTime -->

    <owl:DatatypeProperty rdf:about="http://www.w3.org/ns/prov#startedAtTime">
        <rdfs:domain rdf:resource="http://www.w3.org/ns/prov#Activity"/>
        <rdfs:range rdf:resource="http://www.w3.org/2001/XMLSchema#dateTime"/>
        <rdfs:comment xml:lang="en">The time at which an activity started. See also prov:endedAtTime.</rdfs:comment>
        <rdfs:isDefinedBy rdf:resource="http://www.w3.org/ns/prov-o#"/>
        <rdfs:label>startedAtTime</rdfs:label>
        <prov:category>starting-point</prov:category>
        <prov:component>entities-activities</prov:component>
        <prov:editorialNote xml:lang="en">It is the intent that the property chain holds: (prov:qualifiedStart o prov:atTime) rdfs:subPropertyOf prov:startedAtTime.</prov:editorialNote>
        <prov:qualifiedForm rdf:resource="http://www.w3.org/ns/prov#Start"/>
        <prov:qualifiedForm rdf:resource="http://www.w3.org/ns/prov#atTime"/>
    </owl:DatatypeProperty>
    


    <!-- http://www.w3.org/ns/prov#value -->

    <owl:DatatypeProperty rdf:about="http://www.w3.org/ns/prov#value">
        <rdfs:domain rdf:resource="http://www.w3.org/ns/prov#Entity"/>
        <rdfs:isDefinedBy rdf:resource="http://www.w3.org/ns/prov-o#"/>
        <rdfs:label>value</rdfs:label>
        <prov:category>expanded</prov:category>
        <prov:component>entities-activities</prov:component>
        <prov:definition xml:lang="en">Provides a value that is a direct representation of an entity.</prov:definition>
        <prov:dm rdf:datatype="http://www.w3.org/2001/XMLSchema#anyURI">http://www.w3.org/TR/2013/REC-prov-dm-20130430/#term-attribute-value</prov:dm>
        <prov:editorialNote>The editor&apos;s definition comes from http://www.w3.org/TR/rdf-primer/#rdfvalue</prov:editorialNote>
        <prov:editorialNote xml:lang="en">This property serves the same purpose as rdf:value, but has been reintroduced to avoid some of the definitional ambiguity in the RDF specification (specifically, &apos;may be used in describing structured values&apos;).</prov:editorialNote>
    </owl:DatatypeProperty>
    


    <!-- http://xmlns.com/foaf/0.1/accountName -->

    <owl:DatatypeProperty rdf:about="http://xmlns.com/foaf/0.1/accountName">
        <rdfs:domain rdf:resource="http://xmlns.com/foaf/0.1/OnlineAccount"/>
        <rdfs:range rdf:resource="http://www.w3.org/2000/01/rdf-schema#Literal"/>
        <rdfs:comment>Indicates the name (identifier) associated with this online account.</rdfs:comment>
        <rdfs:isDefinedBy rdf:resource="http://xmlns.com/foaf/0.1/"/>
        <rdfs:label>account name</rdfs:label>
        <ns:term_status>testing</ns:term_status>
    </owl:DatatypeProperty>
    


    <!-- http://xmlns.com/foaf/0.1/age -->

    <owl:DatatypeProperty rdf:about="http://xmlns.com/foaf/0.1/age">
        <rdf:type rdf:resource="http://www.w3.org/2002/07/owl#FunctionalProperty"/>
        <rdfs:domain rdf:resource="http://xmlns.com/foaf/0.1/Agent"/>
        <rdfs:range rdf:resource="http://www.w3.org/2000/01/rdf-schema#Literal"/>
        <rdfs:comment>The age in years of some agent.</rdfs:comment>
        <rdfs:isDefinedBy rdf:resource="http://xmlns.com/foaf/0.1/"/>
        <rdfs:label>age</rdfs:label>
        <ns:term_status>unstable</ns:term_status>
    </owl:DatatypeProperty>
    


    <!-- http://xmlns.com/foaf/0.1/birthday -->

    <owl:DatatypeProperty rdf:about="http://xmlns.com/foaf/0.1/birthday">
        <rdf:type rdf:resource="http://www.w3.org/2002/07/owl#FunctionalProperty"/>
        <rdfs:domain rdf:resource="http://xmlns.com/foaf/0.1/Agent"/>
        <rdfs:range rdf:resource="http://www.w3.org/2000/01/rdf-schema#Literal"/>
        <rdfs:comment>The birthday of this Agent, represented in mm-dd string form, eg. &apos;12-31&apos;.</rdfs:comment>
        <rdfs:isDefinedBy rdf:resource="http://xmlns.com/foaf/0.1/"/>
        <rdfs:label>birthday</rdfs:label>
        <ns:term_status>unstable</ns:term_status>
    </owl:DatatypeProperty>
    


    <!-- http://xmlns.com/foaf/0.1/dnaChecksum -->

    <owl:DatatypeProperty rdf:about="http://xmlns.com/foaf/0.1/dnaChecksum">
        <rdfs:range rdf:resource="http://www.w3.org/2000/01/rdf-schema#Literal"/>
        <rdfs:comment>A checksum for the DNA of some thing. Joke.</rdfs:comment>
        <rdfs:isDefinedBy rdf:resource="http://xmlns.com/foaf/0.1/"/>
        <rdfs:label>DNA checksum</rdfs:label>
        <ns:term_status>archaic</ns:term_status>
    </owl:DatatypeProperty>
    


    <!-- http://xmlns.com/foaf/0.1/familyName -->

    <owl:DatatypeProperty rdf:about="http://xmlns.com/foaf/0.1/familyName">
        <rdfs:domain rdf:resource="http://xmlns.com/foaf/0.1/Person"/>
        <rdfs:range rdf:resource="http://www.w3.org/2000/01/rdf-schema#Literal"/>
        <rdfs:comment>The family name of some person.</rdfs:comment>
        <rdfs:isDefinedBy rdf:resource="http://xmlns.com/foaf/0.1/"/>
        <rdfs:label>familyName</rdfs:label>
        <ns:term_status>testing</ns:term_status>
    </owl:DatatypeProperty>
    


    <!-- http://xmlns.com/foaf/0.1/family_name -->

    <owl:DatatypeProperty rdf:about="http://xmlns.com/foaf/0.1/family_name">
        <rdfs:domain rdf:resource="http://xmlns.com/foaf/0.1/Person"/>
        <rdfs:range rdf:resource="http://www.w3.org/2000/01/rdf-schema#Literal"/>
        <rdfs:comment>The family name of some person.</rdfs:comment>
        <rdfs:isDefinedBy rdf:resource="http://xmlns.com/foaf/0.1/"/>
        <rdfs:label>family_name</rdfs:label>
        <ns:term_status>archaic</ns:term_status>
    </owl:DatatypeProperty>
    


    <!-- http://xmlns.com/foaf/0.1/firstName -->

    <owl:DatatypeProperty rdf:about="http://xmlns.com/foaf/0.1/firstName">
        <rdfs:domain rdf:resource="http://xmlns.com/foaf/0.1/Person"/>
        <rdfs:range rdf:resource="http://www.w3.org/2000/01/rdf-schema#Literal"/>
        <rdfs:comment>The first name of a person.</rdfs:comment>
        <rdfs:isDefinedBy rdf:resource="http://xmlns.com/foaf/0.1/"/>
        <rdfs:label>firstName</rdfs:label>
        <ns:term_status>testing</ns:term_status>
    </owl:DatatypeProperty>
    


    <!-- http://xmlns.com/foaf/0.1/geekcode -->

    <owl:DatatypeProperty rdf:about="http://xmlns.com/foaf/0.1/geekcode">
        <rdfs:domain rdf:resource="http://xmlns.com/foaf/0.1/Person"/>
        <rdfs:range rdf:resource="http://www.w3.org/2000/01/rdf-schema#Literal"/>
        <rdfs:comment>A textual geekcode for this person, see http://www.geekcode.com/geek.html</rdfs:comment>
        <rdfs:isDefinedBy rdf:resource="http://xmlns.com/foaf/0.1/"/>
        <rdfs:label>geekcode</rdfs:label>
        <ns:term_status>archaic</ns:term_status>
    </owl:DatatypeProperty>
    


    <!-- http://xmlns.com/foaf/0.1/gender -->

    <owl:DatatypeProperty rdf:about="http://xmlns.com/foaf/0.1/gender">
        <rdf:type rdf:resource="http://www.w3.org/2002/07/owl#FunctionalProperty"/>
        <rdfs:domain rdf:resource="http://xmlns.com/foaf/0.1/Agent"/>
        <rdfs:range rdf:resource="http://www.w3.org/2000/01/rdf-schema#Literal"/>
        <rdfs:comment>The gender of this Agent (typically but not necessarily &apos;male&apos; or &apos;female&apos;).</rdfs:comment>
        <rdfs:isDefinedBy rdf:resource="http://xmlns.com/foaf/0.1/"/>
        <rdfs:label>gender</rdfs:label>
        <ns:term_status>testing</ns:term_status>
    </owl:DatatypeProperty>
    


    <!-- http://xmlns.com/foaf/0.1/givenName -->

    <owl:DatatypeProperty rdf:about="http://xmlns.com/foaf/0.1/givenName">
        <rdfs:comment>The given name of some person.</rdfs:comment>
        <rdfs:isDefinedBy rdf:resource="http://xmlns.com/foaf/0.1/"/>
        <rdfs:label>Given name</rdfs:label>
        <ns:term_status>testing</ns:term_status>
    </owl:DatatypeProperty>
    


    <!-- http://xmlns.com/foaf/0.1/givenname -->

    <owl:DatatypeProperty rdf:about="http://xmlns.com/foaf/0.1/givenname">
        <rdfs:comment>The given name of some person.</rdfs:comment>
        <rdfs:isDefinedBy rdf:resource="http://xmlns.com/foaf/0.1/"/>
        <rdfs:label>Given name</rdfs:label>
        <ns:term_status>archaic</ns:term_status>
    </owl:DatatypeProperty>
    


    <!-- http://xmlns.com/foaf/0.1/lastName -->

    <owl:DatatypeProperty rdf:about="http://xmlns.com/foaf/0.1/lastName">
        <rdfs:domain rdf:resource="http://xmlns.com/foaf/0.1/Person"/>
        <rdfs:range rdf:resource="http://www.w3.org/2000/01/rdf-schema#Literal"/>
        <rdfs:comment>The last name of a person.</rdfs:comment>
        <rdfs:isDefinedBy rdf:resource="http://xmlns.com/foaf/0.1/"/>
        <rdfs:label>lastName</rdfs:label>
        <ns:term_status>testing</ns:term_status>
    </owl:DatatypeProperty>
    


    <!-- http://xmlns.com/foaf/0.1/mbox_sha1sum -->

    <owl:DatatypeProperty rdf:about="http://xmlns.com/foaf/0.1/mbox_sha1sum">
        <rdfs:range rdf:resource="http://www.w3.org/2000/01/rdf-schema#Literal"/>
    </owl:DatatypeProperty>
    


    <!-- http://xmlns.com/foaf/0.1/myersBriggs -->

    <owl:DatatypeProperty rdf:about="http://xmlns.com/foaf/0.1/myersBriggs">
        <rdfs:domain rdf:resource="http://xmlns.com/foaf/0.1/Person"/>
        <rdfs:range rdf:resource="http://www.w3.org/2000/01/rdf-schema#Literal"/>
        <rdfs:comment>A Myers Briggs (MBTI) personality classification.</rdfs:comment>
        <rdfs:isDefinedBy rdf:resource="http://xmlns.com/foaf/0.1/"/>
        <rdfs:label>myersBriggs</rdfs:label>
        <ns:term_status>testing</ns:term_status>
    </owl:DatatypeProperty>
    


    <!-- http://xmlns.com/foaf/0.1/name -->

    <owl:DatatypeProperty rdf:about="http://xmlns.com/foaf/0.1/name">
        <rdfs:domain rdf:resource="http://www.w3.org/2002/07/owl#Thing"/>
    </owl:DatatypeProperty>
    


    <!-- http://xmlns.com/foaf/0.1/nick -->

    <owl:DatatypeProperty rdf:about="http://xmlns.com/foaf/0.1/nick"/>
    


    <!-- http://xmlns.com/foaf/0.1/plan -->

    <owl:DatatypeProperty rdf:about="http://xmlns.com/foaf/0.1/plan">
        <rdfs:domain rdf:resource="http://xmlns.com/foaf/0.1/Person"/>
        <rdfs:range rdf:resource="http://www.w3.org/2000/01/rdf-schema#Literal"/>
        <rdfs:comment>A .plan comment, in the tradition of finger and &apos;.plan&apos; files.</rdfs:comment>
        <rdfs:isDefinedBy rdf:resource="http://xmlns.com/foaf/0.1/"/>
        <rdfs:label>plan</rdfs:label>
        <ns:term_status>testing</ns:term_status>
    </owl:DatatypeProperty>
    


    <!-- http://xmlns.com/foaf/0.1/sha1 -->

    <owl:DatatypeProperty rdf:about="http://xmlns.com/foaf/0.1/sha1">
        <rdfs:domain rdf:resource="http://xmlns.com/foaf/0.1/Document"/>
        <rdfs:comment>A sha1sum hash, in hex.</rdfs:comment>
        <rdfs:isDefinedBy rdf:resource="http://xmlns.com/foaf/0.1/"/>
        <rdfs:label>sha1sum (hex)</rdfs:label>
        <ns:term_status>unstable</ns:term_status>
    </owl:DatatypeProperty>
    


    <!-- http://xmlns.com/foaf/0.1/status -->

    <owl:DatatypeProperty rdf:about="http://xmlns.com/foaf/0.1/status">
        <rdfs:domain rdf:resource="http://xmlns.com/foaf/0.1/Agent"/>
        <rdfs:range rdf:resource="http://www.w3.org/2000/01/rdf-schema#Literal"/>
        <rdfs:comment>A string expressing what the user is happy for the general public (normally) to know about their current activity.</rdfs:comment>
        <rdfs:isDefinedBy rdf:resource="http://xmlns.com/foaf/0.1/"/>
        <rdfs:label>status</rdfs:label>
        <ns:term_status>unstable</ns:term_status>
    </owl:DatatypeProperty>
    


    <!-- http://xmlns.com/foaf/0.1/surname -->

    <owl:DatatypeProperty rdf:about="http://xmlns.com/foaf/0.1/surname">
        <rdfs:domain rdf:resource="http://xmlns.com/foaf/0.1/Person"/>
        <rdfs:range rdf:resource="http://www.w3.org/2000/01/rdf-schema#Literal"/>
        <rdfs:comment>The surname of some person.</rdfs:comment>
        <rdfs:isDefinedBy rdf:resource="http://xmlns.com/foaf/0.1/"/>
        <rdfs:label>Surname</rdfs:label>
        <ns:term_status>archaic</ns:term_status>
    </owl:DatatypeProperty>
    


    <!-- http://xmlns.com/foaf/0.1/title -->

    <owl:DatatypeProperty rdf:about="http://xmlns.com/foaf/0.1/title">
        <rdfs:comment>Title (Mr, Mrs, Ms, Dr. etc)</rdfs:comment>
        <rdfs:isDefinedBy rdf:resource="http://xmlns.com/foaf/0.1/"/>
        <rdfs:label>title</rdfs:label>
        <ns:term_status>testing</ns:term_status>
    </owl:DatatypeProperty>
    


    <!-- 
    ///////////////////////////////////////////////////////////////////////////////////////
    //
    // Classes
    //
    ///////////////////////////////////////////////////////////////////////////////////////
     -->

    


    <!-- http://org.semanticweb.owlapi/error#Error1 -->

    <owl:Class rdf:about="http://org.semanticweb.owlapi/error#Error1"/>
    


    <!-- http://purl.org/dc/terms/Agent -->

    <owl:Class rdf:about="http://purl.org/dc/terms/Agent">
        <owl:equivalentClass rdf:resource="http://xmlns.com/foaf/0.1/Agent"/>
    </owl:Class>
    


    <!-- http://purl.org/dc/terms/DCMIType -->

    <owl:Class rdf:about="http://purl.org/dc/terms/DCMIType">
        <dc:description>
            The DCMI Type Vocabulary provides a general, cross-domain list of
            approved terms that may be used as values for the Resource Type
            element to identify the genre of a resource.
     </dc:description>
        <dc:type rdf:resource="http://dublincore.org/usage/documents/principles/#encoding-scheme"/>
        <terms:hasVersion rdf:resource="http://dublincore.org/usage/terms/history/#DCMIType-002"/>
        <terms:issued>2000-07-11</terms:issued>
        <terms:modified>2002-06-15</terms:modified>
        <rdfs:comment xml:lang="en-us">A list of types used to categorize the nature or genre 
                                            of the content of the resource.</rdfs:comment>
        <rdfs:isDefinedBy rdf:resource="http://purl.org/dc/terms/"/>
        <rdfs:label xml:lang="en-us">DCMI Type Vocabulary</rdfs:label>
        <rdfs:seeAlso rdf:resource="http://dublincore.org/documents/dcmi-type-vocabulary/"/>
    </owl:Class>
    


    <!-- http://purl.org/dc/terms/DateScheme -->

    <owl:Class rdf:about="http://purl.org/dc/terms/DateScheme">
        <terms:issued>2000-07-11</terms:issued>
        <terms:references rdf:resource="http://purl.org/dc/elements/1.1/date"/>
        <terms:references rdf:resource="http://purl.org/dc/terms/temporal"/>
        <rdfs:comment xml:lang="en-us">A set of date encoding schemes and/or formats </rdfs:comment>
        <rdfs:isDefinedBy rdf:resource="http://purl.org/dc/terms/"/>
        <rdfs:label xml:lang="en-us">Date Encoding Schemes</rdfs:label>
    </owl:Class>
    


    <!-- http://purl.org/dc/terms/FormatScheme -->

    <owl:Class rdf:about="http://purl.org/dc/terms/FormatScheme">
        <terms:issued>2000-07-11</terms:issued>
        <terms:references rdf:resource="http://purl.org/dc/elements/1.1/format"/>
        <rdfs:comment xml:lang="en-us">A set of format encoding schemes.</rdfs:comment>
        <rdfs:isDefinedBy rdf:resource="http://purl.org/dc/terms/"/>
        <rdfs:label xml:lang="en-us">Format Encoding Schemes</rdfs:label>
    </owl:Class>
    


    <!-- http://purl.org/dc/terms/IdentifierScheme -->

    <owl:Class rdf:about="http://purl.org/dc/terms/IdentifierScheme">
        <rdfs:subClassOf rdf:resource="http://purl.org/dc/terms/LanguageScheme"/>
        <terms:issued>2000-07-11</terms:issued>
        <terms:references rdf:resource="http://purl.org/dc/elements/1.1/identifier"/>
        <rdfs:comment xml:lang="en-us">A set of resource identifier encoding schemes and/or formats</rdfs:comment>
        <rdfs:isDefinedBy rdf:resource="http://purl.org/dc/terms/"/>
        <rdfs:label xml:lang="en-us">Resource Identifier Encoding Schemes</rdfs:label>
    </owl:Class>
    


    <!-- http://purl.org/dc/terms/LanguageScheme -->

    <owl:Class rdf:about="http://purl.org/dc/terms/LanguageScheme">
        <terms:issued>2000-07-11</terms:issued>
        <terms:references rdf:resource="http://purl.org/dc/elements/1.1/language"/>
        <rdfs:comment xml:lang="en-us">A set of language encoding schemes and/or formats.</rdfs:comment>
        <rdfs:isDefinedBy rdf:resource="http://purl.org/dc/terms/"/>
        <rdfs:label xml:lang="en-us">Language Encoding Schemes</rdfs:label>
    </owl:Class>
    


    <!-- http://purl.org/dc/terms/RelationScheme -->

    <owl:Class rdf:about="http://purl.org/dc/terms/RelationScheme">
        <terms:issued>2000-07-11</terms:issued>
        <terms:references rdf:resource="http://purl.org/dc/elements/1.1/relation"/>
        <rdfs:comment xml:lang="en-us">A set of resource relation encoding schemes and/or formats</rdfs:comment>
        <rdfs:isDefinedBy rdf:resource="http://purl.org/dc/terms/"/>
        <rdfs:label xml:lang="en-us">Resource Relation Encoding Schemes</rdfs:label>
    </owl:Class>
    


    <!-- http://purl.org/dc/terms/SourceScheme -->

    <owl:Class rdf:about="http://purl.org/dc/terms/SourceScheme">
        <terms:issued>2000-07-11</terms:issued>
        <terms:references rdf:resource="http://purl.org/dc/elements/1.1/source"/>
        <rdfs:comment xml:lang="en-us">A set of source encoding schemes and/or formats</rdfs:comment>
        <rdfs:isDefinedBy rdf:resource="http://purl.org/dc/terms/"/>
        <rdfs:label xml:lang="en-us">Source Encoding Schemes</rdfs:label>
    </owl:Class>
    


    <!-- http://purl.org/dc/terms/SpatialScheme -->

    <owl:Class rdf:about="http://purl.org/dc/terms/SpatialScheme">
        <terms:issued>2000-07-11</terms:issued>
        <terms:references rdf:resource="http://purl.org/dc/terms/spatial"/>
        <rdfs:comment xml:lang="en-us">A set of geographic place encoding schemes and/or formats</rdfs:comment>
        <rdfs:isDefinedBy rdf:resource="http://purl.org/dc/terms/"/>
        <rdfs:label xml:lang="en-us">Place Encoding Schemes</rdfs:label>
    </owl:Class>
    


    <!-- http://purl.org/dc/terms/SubjectScheme -->

    <owl:Class rdf:about="http://purl.org/dc/terms/SubjectScheme">
        <terms:issued>2000-07-11</terms:issued>
        <terms:references rdf:resource="http://purl.org/dc/elements/1.1/subject"/>
        <rdfs:comment xml:lang="en-us">A set of subject encoding schemes and/or formats</rdfs:comment>
        <rdfs:isDefinedBy rdf:resource="http://purl.org/dc/terms/"/>
        <rdfs:label xml:lang="en-us">Subject Encoding Schemes</rdfs:label>
    </owl:Class>
    


    <!-- http://purl.org/dc/terms/TemporalScheme -->

    <owl:Class rdf:about="http://purl.org/dc/terms/TemporalScheme">
        <terms:issued>2000-07-11</terms:issued>
        <terms:references rdf:resource="http://purl.org/dc/terms/temporal"/>
        <rdfs:comment xml:lang="en-us">A set of encoding schemes for 
       the coverage qualifier &quot;temporal&quot;</rdfs:comment>
        <rdfs:isDefinedBy rdf:resource="http://purl.org/dc/terms/"/>
        <rdfs:label xml:lang="en-us">Encoding Schemes
        for temporal characteristics</rdfs:label>
    </owl:Class>
    


    <!-- http://purl.org/dc/terms/TypeScheme -->

    <owl:Class rdf:about="http://purl.org/dc/terms/TypeScheme">
        <terms:issued>2000-07-11</terms:issued>
        <terms:references rdf:resource="http://purl.org/dc/elements/1.1/type"/>
        <rdfs:comment xml:lang="en-us">A set of resource type encoding schemes and/or formats</rdfs:comment>
        <rdfs:isDefinedBy rdf:resource="http://purl.org/dc/terms/"/>
        <rdfs:label xml:lang="en-us">Resource Type Encoding Schemes</rdfs:label>
    </owl:Class>
    


    <!-- http://rdfs.org/ns/void#Dataset -->

    <owl:Class rdf:about="http://rdfs.org/ns/void#Dataset">
        <rdfs:subClassOf rdf:resource="http://www.w3.org/2004/02/skos/core#Concept"/>
        <dc:publisher></dc:publisher>
        <dc:title></dc:title>
        <rdfs:comment>A set of RDF triples that are published, maintained or aggregated by a single provider.</rdfs:comment>
        <rdfs:label>dataset</rdfs:label>
    </owl:Class>
    


    <!-- http://rdfs.org/ns/void#DatasetDescription -->

    <owl:Class rdf:about="http://rdfs.org/ns/void#DatasetDescription">
        <rdfs:subClassOf rdf:resource="http://xmlns.com/foaf/0.1/Document"/>
        <rdfs:comment>A web resource whose foaf:primaryTopic or foaf:topics include void:Datasets.</rdfs:comment>
        <rdfs:label>dataset description</rdfs:label>
    </owl:Class>
    


    <!-- http://rdfs.org/ns/void#Linkset -->

    <owl:Class rdf:about="http://rdfs.org/ns/void#Linkset">
        <rdfs:subClassOf rdf:resource="http://rdfs.org/ns/void#Dataset"/>
        <rdfs:comment>A collection of RDF links between two void:Datasets.</rdfs:comment>
        <rdfs:label>linkset</rdfs:label>
    </owl:Class>
    


    <!-- http://rdfs.org/ns/void#TechnicalFeature -->

    <owl:Class rdf:about="http://rdfs.org/ns/void#TechnicalFeature">
        <rdfs:comment>A technical feature of a void:Dataset, such as a supported RDF serialization format.</rdfs:comment>
        <rdfs:label>technical feature</rdfs:label>
    </owl:Class>
    


    <!-- http://schema.org/CreativeWork -->

    <owl:Class rdf:about="http://schema.org/CreativeWork">
        <owl:equivalentClass rdf:resource="http://xmlns.com/foaf/0.1/Document"/>
    </owl:Class>
    


    <!-- http://schema.org/ImageObject -->

    <owl:Class rdf:about="http://schema.org/ImageObject">
        <owl:equivalentClass rdf:resource="http://xmlns.com/foaf/0.1/Image"/>
    </owl:Class>
    


    <!-- http://schema.org/Person -->

    <owl:Class rdf:about="http://schema.org/Person">
        <owl:equivalentClass rdf:resource="http://xmlns.com/foaf/0.1/Person"/>
    </owl:Class>
    


    <!-- http://trdf.sourceforge.net/trustvocab#TrustValue -->

    <owl:Class rdf:about="http://trdf.sourceforge.net/trustvocab#TrustValue">
        <rdfs:subClassOf rdf:resource="http://org.semanticweb.owlapi/error#Error1"/>
        <rdfs:subClassOf rdf:resource="http://www.w3.org/2002/07/owl#Thing"/>
        <rdfs:subClassOf>
            <owl:Restriction>
                <owl:onProperty rdf:resource="http://trdf.sourceforge.net/trustvocab#truster"/>
                <owl:cardinality rdf:datatype="http://www.w3.org/2001/XMLSchema#nonNegativeInteger">1</owl:cardinality>
            </owl:Restriction>
        </rdfs:subClassOf>
        <rdfs:comment xml:lang="en">This class represents a trust value that is associated to an RDF statement. Use the rdf:value property to specify the actual value of the trust value. This value must be a number in the interval [-1,1]. Trust values that do not have this property are considered as unknown trust values.</rdfs:comment>
    </owl:Class>
    


    <!-- http://www.semanticweb.org/k_mil/ontologies/2021/8/EvalLOD#BlackList -->

    <owl:Class rdf:about="http://www.semanticweb.org/k_mil/ontologies/2021/8/EvalLOD#BlackList">
        <rdfs:subClassOf rdf:resource="http://xmlns.com/foaf/0.1/Group"/>
    </owl:Class>
    


    <!-- http://www.semanticweb.org/k_mil/ontologies/2021/8/EvalLOD#Trusted -->

    <owl:Class rdf:about="http://www.semanticweb.org/k_mil/ontologies/2021/8/EvalLOD#Trusted">
        <rdfs:subClassOf rdf:resource="http://www.w3.org/2004/02/skos/core#Concept"/>
    </owl:Class>
    


    <!-- http://www.semanticweb.org/k_mil/ontologies/2021/8/EvalLOD#WhiteList -->

    <owl:Class rdf:about="http://www.semanticweb.org/k_mil/ontologies/2021/8/EvalLOD#WhiteList">
        <rdfs:subClassOf rdf:resource="http://xmlns.com/foaf/0.1/Group"/>
    </owl:Class>
    


    <!-- http://www.semanticweb.org/k_mil/ontologies/2021/8/EvalLOD#blacklistedDataset -->

    <owl:Class rdf:about="http://www.semanticweb.org/k_mil/ontologies/2021/8/EvalLOD#blacklistedDataset">
        <owl:equivalentClass>
            <owl:Restriction>
                <owl:onProperty rdf:resource="http://www.semanticweb.org/k_mil/ontologies/2021/8/EvalLOD#belongsTo"/>
                <owl:minQualifiedCardinality rdf:datatype="http://www.w3.org/2001/XMLSchema#nonNegativeInteger">1</owl:minQualifiedCardinality>
                <owl:onClass rdf:resource="http://www.semanticweb.org/k_mil/ontologies/2021/8/EvalLOD#BlackList"/>
            </owl:Restriction>
        </owl:equivalentClass>
        <rdfs:subClassOf rdf:resource="http://rdfs.org/ns/void#Dataset"/>
    </owl:Class>
    


    <!-- http://www.semanticweb.org/k_mil/ontologies/2021/8/EvalLOD#datasetWithLicense -->

    <owl:Class rdf:about="http://www.semanticweb.org/k_mil/ontologies/2021/8/EvalLOD#datasetWithLicense">
        <rdfs:subClassOf rdf:resource="http://rdfs.org/ns/void#Dataset"/>
    </owl:Class>
    


    <!-- http://www.semanticweb.org/k_mil/ontologies/2021/8/EvalLOD#datasetWithProvenance -->

    <owl:Class rdf:about="http://www.semanticweb.org/k_mil/ontologies/2021/8/EvalLOD#datasetWithProvenance">
        <rdfs:subClassOf rdf:resource="http://rdfs.org/ns/void#Dataset"/>
    </owl:Class>
    


    <!-- http://www.semanticweb.org/k_mil/ontologies/2021/8/EvalLOD#verifiableDataset -->

    <owl:Class rdf:about="http://www.semanticweb.org/k_mil/ontologies/2021/8/EvalLOD#verifiableDataset">
        <rdfs:subClassOf rdf:resource="http://rdfs.org/ns/void#Dataset"/>
    </owl:Class>
    


    <!-- http://www.w3.org/2000/01/rdf-schema#Class -->

    <owl:Class rdf:about="http://www.w3.org/2000/01/rdf-schema#Class"/>
    


    <!-- http://www.w3.org/2000/10/swap/pim/contact#Person -->

    <owl:Class rdf:about="http://www.w3.org/2000/10/swap/pim/contact#Person">
        <owl:equivalentClass rdf:resource="http://xmlns.com/foaf/0.1/Person"/>
    </owl:Class>
    


    <!-- http://www.w3.org/2002/07/owl#Thing -->

    <owl:Class rdf:about="http://www.w3.org/2002/07/owl#Thing">
        <rdfs:label>Thing</rdfs:label>
    </owl:Class>
    


    <!-- http://www.w3.org/2003/01/geo/wgs84_pos#SpatialThing -->

    <owl:Class rdf:about="http://www.w3.org/2003/01/geo/wgs84_pos#SpatialThing">
        <rdfs:label>Spatial Thing</rdfs:label>
    </owl:Class>
    


    <!-- http://www.w3.org/2004/02/skos/core#Concept -->

    <rdf:Description rdf:about="http://www.w3.org/2004/02/skos/core#Concept">
        <rdfs:subClassOf rdf:resource="http://rdfs.org/ns/void#Dataset"/>
        <rdfs:label>Concept</rdfs:label>
    </rdf:Description>
    


    <!-- http://www.w3.org/ns/oa#Annotation -->

    <owl:Class rdf:about="http://www.w3.org/ns/oa#Annotation">
        <rdfs:comment>The class for Web Annotations.</rdfs:comment>
        <rdfs:isDefinedBy rdf:resource="http://www.w3.org/ns/oa#"/>
        <rdfs:label>Annotation</rdfs:label>
    </owl:Class>
    


    <!-- http://www.w3.org/ns/oa#Choice -->

    <owl:Class rdf:about="http://www.w3.org/ns/oa#Choice">
        <rdfs:subClassOf rdf:resource="http://www.w3.org/ns/activitystreams#OrderedCollection"/>
        <rdfs:comment>A subClass of  as:OrderedCollection  that conveys to a consuming application that it should select one of the resources in the  as:items  list to use, rather than all of them.  This is typically used to provide a choice of resources to render to the user, based on further supplied properties.  If the consuming application cannot determine the user&apos;s preference, then it should use the first in the list.</rdfs:comment>
        <rdfs:isDefinedBy rdf:resource="http://www.w3.org/ns/oa#"/>
        <rdfs:label>Choice</rdfs:label>
    </owl:Class>
    


    <!-- http://www.w3.org/ns/oa#CssSelector -->

    <owl:Class rdf:about="http://www.w3.org/ns/oa#CssSelector">
        <rdfs:subClassOf rdf:resource="http://www.w3.org/ns/oa#Selector"/>
        <rdfs:comment>A CssSelector describes a Segment of interest in a representation that conforms to the Document Object Model through the use of the CSS selector specification.</rdfs:comment>
        <rdfs:isDefinedBy rdf:resource="http://www.w3.org/ns/oa#"/>
        <rdfs:label>CssSelector</rdfs:label>
    </owl:Class>
    


    <!-- http://www.w3.org/ns/oa#CssStyle -->

    <owl:Class rdf:about="http://www.w3.org/ns/oa#CssStyle">
        <rdfs:subClassOf rdf:resource="http://www.w3.org/ns/oa#Style"/>
        <rdfs:comment>A resource which describes styles for resources participating in the Annotation using CSS.</rdfs:comment>
        <rdfs:isDefinedBy rdf:resource="http://www.w3.org/ns/oa#"/>
        <rdfs:label>CssStyle</rdfs:label>
    </owl:Class>
    


    <!-- http://www.w3.org/ns/oa#DataPositionSelector -->

    <owl:Class rdf:about="http://www.w3.org/ns/oa#DataPositionSelector">
        <rdfs:subClassOf rdf:resource="http://www.w3.org/ns/oa#Selector"/>
        <rdfs:comment>DataPositionSelector describes a range of data by recording the start and end positions of the selection in the stream. Position 0 would be immediately before the first byte, position 1 would be immediately before the second byte, and so on. The start byte is thus included in the list, but the end byte is not.</rdfs:comment>
        <rdfs:isDefinedBy rdf:resource="http://www.w3.org/ns/oa#"/>
        <rdfs:label>DataPositionSelector</rdfs:label>
    </owl:Class>
    


    <!-- http://www.w3.org/ns/oa#Direction -->

    <owl:Class rdf:about="http://www.w3.org/ns/oa#Direction">
        <rdfs:comment>A class to encapsulate the different text directions that a textual resource might take.  It is not used directly in the Annotation Model, only its three instances.</rdfs:comment>
        <rdfs:isDefinedBy rdf:resource="http://www.w3.org/ns/oa#"/>
        <rdfs:label>Direction</rdfs:label>
    </owl:Class>
    


    <!-- http://www.w3.org/ns/oa#FragmentSelector -->

    <owl:Class rdf:about="http://www.w3.org/ns/oa#FragmentSelector">
        <rdfs:subClassOf rdf:resource="http://www.w3.org/ns/oa#Selector"/>
        <rdfs:comment>The FragmentSelector class is used to record the segment of a representation using the IRI fragment specification defined by the representation&apos;s media type.</rdfs:comment>
        <rdfs:isDefinedBy rdf:resource="http://www.w3.org/ns/oa#"/>
        <rdfs:label>FragmentSelector</rdfs:label>
    </owl:Class>
    


    <!-- http://www.w3.org/ns/oa#HttpRequestState -->

    <owl:Class rdf:about="http://www.w3.org/ns/oa#HttpRequestState">
        <rdfs:subClassOf rdf:resource="http://www.w3.org/ns/oa#State"/>
        <rdfs:comment>The HttpRequestState class is used to record the HTTP request headers that a client SHOULD use to request the correct representation from the resource. </rdfs:comment>
        <rdfs:isDefinedBy rdf:resource="http://www.w3.org/ns/oa#"/>
        <rdfs:label>HttpRequestState</rdfs:label>
    </owl:Class>
    


    <!-- http://www.w3.org/ns/oa#Motivation -->

    <owl:Class rdf:about="http://www.w3.org/ns/oa#Motivation">
        <rdfs:subClassOf rdf:resource="http://www.w3.org/2004/02/skos/core#Concept"/>
        <rdfs:comment>The Motivation class is used to record the user&apos;s intent or motivation for the creation of the Annotation, or the inclusion of the body or target, that it is associated with.</rdfs:comment>
        <rdfs:isDefinedBy rdf:resource="http://www.w3.org/ns/oa#"/>
        <rdfs:label>Motivation</rdfs:label>
    </owl:Class>
    


    <!-- http://www.w3.org/ns/oa#RangeSelector -->

    <owl:Class rdf:about="http://www.w3.org/ns/oa#RangeSelector">
        <rdfs:subClassOf rdf:resource="http://www.w3.org/ns/oa#Selector"/>
        <rdfs:comment>A Range Selector can be used to identify the beginning and the end of the selection by using other Selectors. The selection consists of everything from the beginning of the starting selector through to the beginning of the ending selector, but not including it.</rdfs:comment>
        <rdfs:isDefinedBy rdf:resource="http://www.w3.org/ns/oa#"/>
        <rdfs:label>RangeSelector</rdfs:label>
    </owl:Class>
    


    <!-- http://www.w3.org/ns/oa#ResourceSelection -->

    <owl:Class rdf:about="http://www.w3.org/ns/oa#ResourceSelection">
        <rdfs:comment>Instances of the ResourceSelection class identify part (described by an oa:Selector) of another resource (referenced with oa:hasSource), possibly from a particular representation of a resource (described by an oa:State). Please note that ResourceSelection is not used directly in the Web Annotation model, but is provided as a separate class for further application profiles to use, separate from oa:SpecificResource which has many Annotation specific features.</rdfs:comment>
        <rdfs:isDefinedBy rdf:resource="http://www.w3.org/ns/oa#"/>
        <rdfs:label>ResourceSelection</rdfs:label>
    </owl:Class>
    


    <!-- http://www.w3.org/ns/oa#Selector -->

    <owl:Class rdf:about="http://www.w3.org/ns/oa#Selector">
        <rdfs:comment>A resource which describes the segment of interest in a representation of a Source resource, indicated with oa:hasSelector from the Specific Resource. This class is not used directly in the Annotation model, only its subclasses.</rdfs:comment>
        <rdfs:isDefinedBy rdf:resource="http://www.w3.org/ns/oa#"/>
        <rdfs:label>Selector</rdfs:label>
    </owl:Class>
    


    <!-- http://www.w3.org/ns/oa#SpecificResource -->

    <owl:Class rdf:about="http://www.w3.org/ns/oa#SpecificResource">
        <rdfs:subClassOf rdf:resource="http://www.w3.org/ns/oa#ResourceSelection"/>
        <rdfs:comment>Instances of the SpecificResource class identify part of another resource (referenced with oa:hasSource), a particular representation of a resource, a resource with styling hints for renders, or any combination of these, as used within an Annotation.</rdfs:comment>
        <rdfs:isDefinedBy rdf:resource="http://www.w3.org/ns/oa#"/>
        <rdfs:label>SpecificResource</rdfs:label>
    </owl:Class>
    


    <!-- http://www.w3.org/ns/oa#State -->

    <owl:Class rdf:about="http://www.w3.org/ns/oa#State">
        <rdfs:comment>A State describes the intended state of a resource as applied to the particular Annotation, and thus provides the information needed to retrieve the correct representation of that resource.</rdfs:comment>
        <rdfs:isDefinedBy rdf:resource="http://www.w3.org/ns/oa#"/>
        <rdfs:label>State</rdfs:label>
    </owl:Class>
    


    <!-- http://www.w3.org/ns/oa#Style -->

    <owl:Class rdf:about="http://www.w3.org/ns/oa#Style">
        <rdfs:comment>A Style describes the intended styling of a resource as applied to the particular Annotation, and thus provides the information to ensure that rendering is consistent across implementations.</rdfs:comment>
        <rdfs:isDefinedBy rdf:resource="http://www.w3.org/ns/oa#"/>
        <rdfs:label>Style</rdfs:label>
    </owl:Class>
    


    <!-- http://www.w3.org/ns/oa#SvgSelector -->

    <owl:Class rdf:about="http://www.w3.org/ns/oa#SvgSelector">
        <rdfs:subClassOf rdf:resource="http://www.w3.org/ns/oa#Selector"/>
        <rdfs:comment>An SvgSelector defines an area through the use of the Scalable Vector Graphics [SVG] standard. This allows the user to select a non-rectangular area of the content, such as a circle or polygon by describing the region using SVG. The SVG may be either embedded within the Annotation or referenced as an External Resource.</rdfs:comment>
        <rdfs:isDefinedBy rdf:resource="http://www.w3.org/ns/oa#"/>
        <rdfs:label>SvgSelector</rdfs:label>
    </owl:Class>
    


    <!-- http://www.w3.org/ns/oa#TextPositionSelector -->

    <owl:Class rdf:about="http://www.w3.org/ns/oa#TextPositionSelector">
        <rdfs:subClassOf rdf:resource="http://www.w3.org/ns/oa#Selector"/>
        <rdfs:comment>The TextPositionSelector describes a range of text by recording the start and end positions of the selection in the stream. Position 0 would be immediately before the first character, position 1 would be immediately before the second character, and so on.</rdfs:comment>
        <rdfs:isDefinedBy rdf:resource="http://www.w3.org/ns/oa#"/>
        <rdfs:label>TextPositionSelector</rdfs:label>
    </owl:Class>
    


    <!-- http://www.w3.org/ns/oa#TextQuoteSelector -->

    <owl:Class rdf:about="http://www.w3.org/ns/oa#TextQuoteSelector">
        <rdfs:subClassOf rdf:resource="http://www.w3.org/ns/oa#Selector"/>
        <rdfs:comment>The TextQuoteSelector describes a range of text by copying it, and including some of the text immediately before (a prefix) and after (a suffix) it to distinguish between multiple copies of the same sequence of characters.</rdfs:comment>
        <rdfs:isDefinedBy rdf:resource="http://www.w3.org/ns/oa#"/>
        <rdfs:label>TextQuoteSelector</rdfs:label>
    </owl:Class>
    


    <!-- http://www.w3.org/ns/oa#TextualBody -->

    <owl:Class rdf:about="http://www.w3.org/ns/oa#TextualBody">
        <rdfs:comment></rdfs:comment>
        <rdfs:isDefinedBy rdf:resource="http://www.w3.org/ns/oa#"/>
        <rdfs:label>TextualBody</rdfs:label>
    </owl:Class>
    


    <!-- http://www.w3.org/ns/oa#TimeState -->

    <owl:Class rdf:about="http://www.w3.org/ns/oa#TimeState">
        <rdfs:subClassOf rdf:resource="http://www.w3.org/ns/oa#State"/>
        <rdfs:comment>A TimeState records the time at which the resource&apos;s state is appropriate for the Annotation, typically the time that the Annotation was created and/or a link to a persistent copy of the current version.</rdfs:comment>
        <rdfs:isDefinedBy rdf:resource="http://www.w3.org/ns/oa#"/>
        <rdfs:label>TimeState</rdfs:label>
    </owl:Class>
    


    <!-- http://www.w3.org/ns/oa#XPathSelector -->

    <owl:Class rdf:about="http://www.w3.org/ns/oa#XPathSelector">
        <rdfs:subClassOf rdf:resource="http://www.w3.org/ns/oa#Selector"/>
        <rdfs:comment> An XPathSelector is used to select elements and content within a resource that supports the Document Object Model via a specified XPath value.</rdfs:comment>
        <rdfs:isDefinedBy rdf:resource="http://www.w3.org/ns/oa#"/>
        <rdfs:label>XPathSelector</rdfs:label>
    </owl:Class>
    


    <!-- http://www.w3.org/ns/prov#Activity -->

    <owl:Class rdf:about="http://www.w3.org/ns/prov#Activity">
        <owl:disjointWith rdf:resource="http://www.w3.org/ns/prov#Entity"/>
        <rdfs:isDefinedBy rdf:resource="http://www.w3.org/ns/prov-o#"/>
        <rdfs:label>Activity</rdfs:label>
        <prov:category>starting-point</prov:category>
        <prov:component>entities-activities</prov:component>
        <prov:constraints rdf:datatype="http://www.w3.org/2001/XMLSchema#anyURI">http://www.w3.org/TR/2013/REC-prov-constraints-20130430/#prov-dm-constraints-fig</prov:constraints>
        <prov:definition>An activity is something that occurs over a period of time and acts upon or with entities; it may include consuming, processing, transforming, modifying, relocating, using, or generating entities.</prov:definition>
        <prov:dm rdf:datatype="http://www.w3.org/2001/XMLSchema#anyURI">http://www.w3.org/TR/2013/REC-prov-dm-20130430/#term-Activity</prov:dm>
        <prov:n rdf:datatype="http://www.w3.org/2001/XMLSchema#anyURI">http://www.w3.org/TR/2013/REC-prov-n-20130430/#expression-Activity</prov:n>
    </owl:Class>
    


    <!-- http://www.w3.org/ns/prov#ActivityInfluence -->

    <owl:Class rdf:about="http://www.w3.org/ns/prov#ActivityInfluence">
        <rdfs:subClassOf rdf:resource="http://www.w3.org/ns/prov#Influence"/>
        <rdfs:subClassOf>
            <owl:Restriction>
                <owl:onProperty rdf:resource="http://www.w3.org/ns/prov#hadActivity"/>
                <owl:maxCardinality rdf:datatype="http://www.w3.org/2001/XMLSchema#nonNegativeInteger">0</owl:maxCardinality>
            </owl:Restriction>
        </rdfs:subClassOf>
        <owl:disjointWith rdf:resource="http://www.w3.org/ns/prov#EntityInfluence"/>
        <rdfs:comment xml:lang="en">ActivityInfluence provides additional descriptions of an Activity&apos;s binary influence upon any other kind of resource. Instances of ActivityInfluence use the prov:activity property to cite the influencing Activity.</rdfs:comment>
        <rdfs:comment xml:lang="en">It is not recommended that the type ActivityInfluence be asserted without also asserting one of its more specific subclasses.</rdfs:comment>
        <rdfs:isDefinedBy rdf:resource="http://www.w3.org/ns/prov-o#"/>
        <rdfs:label>ActivityInfluence</rdfs:label>
        <rdfs:seeAlso rdf:resource="http://www.w3.org/ns/prov#activity"/>
        <prov:category>qualified</prov:category>
        <prov:editorsDefinition xml:lang="en">ActivitiyInfluence is the capacity of an activity to have an effect on the character, development, or behavior of another by means of generation, invalidation, communication, or other.</prov:editorsDefinition>
    </owl:Class>
    


    <!-- http://www.w3.org/ns/prov#Agent -->

    <owl:Class rdf:about="http://www.w3.org/ns/prov#Agent">
        <owl:disjointWith rdf:resource="http://www.w3.org/ns/prov#InstantaneousEvent"/>
        <rdfs:isDefinedBy rdf:resource="http://www.w3.org/ns/prov-o#"/>
        <rdfs:label>Agent</rdfs:label>
        <prov:category>starting-point</prov:category>
        <prov:component>agents-responsibility</prov:component>
        <prov:definition xml:lang="en">An agent is something that bears some form of responsibility for an activity taking place, for the existence of an entity, or for another agent&apos;s activity. </prov:definition>
        <prov:dm rdf:datatype="http://www.w3.org/2001/XMLSchema#anyURI">http://www.w3.org/TR/2013/REC-prov-dm-20130430/#term-agent</prov:dm>
        <prov:n rdf:datatype="http://www.w3.org/2001/XMLSchema#anyURI">http://www.w3.org/TR/2013/REC-prov-n-20130430/#expression-Agent</prov:n>
    </owl:Class>
    


    <!-- http://www.w3.org/ns/prov#AgentInfluence -->

    <owl:Class rdf:about="http://www.w3.org/ns/prov#AgentInfluence">
        <rdfs:subClassOf rdf:resource="http://www.w3.org/ns/prov#Influence"/>
        <rdfs:comment xml:lang="en">AgentInfluence provides additional descriptions of an Agent&apos;s binary influence upon any other kind of resource. Instances of AgentInfluence use the prov:agent property to cite the influencing Agent.</rdfs:comment>
        <rdfs:comment xml:lang="en">It is not recommended that the type AgentInfluence be asserted without also asserting one of its more specific subclasses.</rdfs:comment>
        <rdfs:isDefinedBy rdf:resource="http://www.w3.org/ns/prov-o#"/>
        <rdfs:label>AgentInfluence</rdfs:label>
        <rdfs:seeAlso rdf:resource="http://www.w3.org/ns/prov#agent"/>
        <prov:category>qualified</prov:category>
        <prov:editorsDefinition xml:lang="en">AgentInfluence is the capacity of an agent to have an effect on the character, development, or behavior of another by means of attribution, association, delegation, or other.</prov:editorsDefinition>
    </owl:Class>
    


    <!-- http://www.w3.org/ns/prov#Association -->

    <owl:Class rdf:about="http://www.w3.org/ns/prov#Association">
        <rdfs:subClassOf rdf:resource="http://www.w3.org/ns/prov#AgentInfluence"/>
        <rdfs:comment xml:lang="en">An instance of prov:Association provides additional descriptions about the binary prov:wasAssociatedWith relation from an prov:Activity to some prov:Agent that had some responsiblity for it. For example, :baking prov:wasAssociatedWith :baker; prov:qualifiedAssociation [ a prov:Association; prov:agent :baker; :foo :bar ].</rdfs:comment>
        <rdfs:isDefinedBy rdf:resource="http://www.w3.org/ns/prov-o#"/>
        <rdfs:label>Association</rdfs:label>
        <prov:category>qualified</prov:category>
        <prov:component>agents-responsibility</prov:component>
        <prov:definition xml:lang="en">An activity association is an assignment of responsibility to an agent for an activity, indicating that the agent had a role in the activity. It further allows for a plan to be specified, which is the plan intended by the agent to achieve some goals in the context of this activity.</prov:definition>
        <prov:dm rdf:datatype="http://www.w3.org/2001/XMLSchema#anyURI">http://www.w3.org/TR/2013/REC-prov-dm-20130430/#term-Association</prov:dm>
        <prov:n rdf:datatype="http://www.w3.org/2001/XMLSchema#anyURI">http://www.w3.org/TR/2013/REC-prov-n-20130430/#expression-Association</prov:n>
        <prov:unqualifiedForm rdf:resource="http://www.w3.org/ns/prov#wasAssociatedWith"/>
    </owl:Class>
    


    <!-- http://www.w3.org/ns/prov#Attribution -->

    <owl:Class rdf:about="http://www.w3.org/ns/prov#Attribution">
        <rdfs:subClassOf rdf:resource="http://www.w3.org/ns/prov#AgentInfluence"/>
        <rdfs:comment xml:lang="en">An instance of prov:Attribution provides additional descriptions about the binary prov:wasAttributedTo relation from an prov:Entity to some prov:Agent that had some responsible for it. For example, :cake prov:wasAttributedTo :baker; prov:qualifiedAttribution [ a prov:Attribution; prov:entity :baker; :foo :bar ].</rdfs:comment>
        <rdfs:isDefinedBy rdf:resource="http://www.w3.org/ns/prov-o#"/>
        <rdfs:label>Attribution</rdfs:label>
        <prov:category>qualified</prov:category>
        <prov:component>agents-responsibility</prov:component>
        <prov:constraints rdf:datatype="http://www.w3.org/2001/XMLSchema#anyURI">http://www.w3.org/TR/2013/REC-prov-constraints-20130430/#prov-dm-constraints-fig</prov:constraints>
        <prov:definition xml:lang="en">Attribution is the ascribing of an entity to an agent.

When an entity e is attributed to agent ag, entity e was generated by some unspecified activity that in turn was associated to agent ag. Thus, this relation is useful when the activity is not known, or irrelevant.</prov:definition>
        <prov:dm rdf:datatype="http://www.w3.org/2001/XMLSchema#anyURI">http://www.w3.org/TR/2013/REC-prov-dm-20130430/#term-attribution</prov:dm>
        <prov:n rdf:datatype="http://www.w3.org/2001/XMLSchema#anyURI">http://www.w3.org/TR/2013/REC-prov-n-20130430/#expression-attribution</prov:n>
        <prov:unqualifiedForm rdf:resource="http://www.w3.org/ns/prov#wasAttributedTo"/>
    </owl:Class>
    


    <!-- http://www.w3.org/ns/prov#Bundle -->

    <owl:Class rdf:about="http://www.w3.org/ns/prov#Bundle">
        <rdfs:subClassOf rdf:resource="http://www.w3.org/ns/prov#Entity"/>
        <rdfs:comment xml:lang="en">Note that there are kinds of bundles (e.g. handwritten letters, audio recordings, etc.) that are not expressed in PROV-O, but can be still be described by PROV-O.</rdfs:comment>
        <rdfs:isDefinedBy rdf:resource="http://www.w3.org/ns/prov-o#"/>
        <rdfs:label>Bundle</rdfs:label>
        <prov:category>expanded</prov:category>
        <prov:definition xml:lang="en">A bundle is a named set of provenance descriptions, and is itself an Entity, so allowing provenance of provenance to be expressed.</prov:definition>
        <prov:dm rdf:datatype="http://www.w3.org/2001/XMLSchema#anyURI">http://www.w3.org/TR/2013/REC-prov-dm-20130430/#term-bundle-entity</prov:dm>
        <prov:n rdf:datatype="http://www.w3.org/2001/XMLSchema#anyURI">http://www.w3.org/TR/2013/REC-prov-n-20130430/#expression-bundle-declaration</prov:n>
    </owl:Class>
    


    <!-- http://www.w3.org/ns/prov#Collection -->

    <owl:Class rdf:about="http://www.w3.org/ns/prov#Collection">
        <rdfs:subClassOf rdf:resource="http://www.w3.org/ns/prov#Entity"/>
        <rdfs:isDefinedBy rdf:resource="http://www.w3.org/ns/prov-o#"/>
        <rdfs:label>Collection</rdfs:label>
        <prov:category>expanded</prov:category>
        <prov:component>collections</prov:component>
        <prov:definition xml:lang="en">A collection is an entity that provides a structure to some constituents, which are themselves entities. These constituents are said to be member of the collections.</prov:definition>
        <prov:dm rdf:datatype="http://www.w3.org/2001/XMLSchema#anyURI">http://www.w3.org/TR/2013/REC-prov-dm-20130430/#term-collection</prov:dm>
    </owl:Class>
    


    <!-- http://www.w3.org/ns/prov#Communication -->

    <owl:Class rdf:about="http://www.w3.org/ns/prov#Communication">
        <rdfs:subClassOf rdf:resource="http://www.w3.org/ns/prov#ActivityInfluence"/>
        <rdfs:comment xml:lang="en">An instance of prov:Communication provides additional descriptions about the binary prov:wasInformedBy relation from an informed prov:Activity to the prov:Activity that informed it. For example, :you_jumping_off_bridge prov:wasInformedBy :everyone_else_jumping_off_bridge; prov:qualifiedCommunication [ a prov:Communication; prov:activity :everyone_else_jumping_off_bridge; :foo :bar ].</rdfs:comment>
        <rdfs:isDefinedBy rdf:resource="http://www.w3.org/ns/prov-o#"/>
        <rdfs:label>Communication</rdfs:label>
        <prov:category>qualified</prov:category>
        <prov:component>entities-activities</prov:component>
        <prov:constraints rdf:datatype="http://www.w3.org/2001/XMLSchema#anyURI">http://www.w3.org/TR/2013/REC-prov-constraints-20130430/#prov-dm-constraints-fig</prov:constraints>
        <prov:definition>Communication is the exchange of an entity by two activities, one activity using the entity generated by the other.</prov:definition>
        <prov:dm rdf:datatype="http://www.w3.org/2001/XMLSchema#anyURI">http://www.w3.org/TR/2013/REC-prov-dm-20130430/#term-Communication</prov:dm>
        <prov:n rdf:datatype="http://www.w3.org/2001/XMLSchema#anyURI">http://www.w3.org/TR/2013/REC-prov-n-20130430/#expression-wasInformedBy</prov:n>
        <prov:unqualifiedForm rdf:resource="http://www.w3.org/ns/prov#wasInformedBy"/>
    </owl:Class>
    


    <!-- http://www.w3.org/ns/prov#Delegation -->

    <owl:Class rdf:about="http://www.w3.org/ns/prov#Delegation">
        <rdfs:subClassOf rdf:resource="http://www.w3.org/ns/prov#AgentInfluence"/>
        <rdfs:comment xml:lang="en">An instance of prov:Delegation provides additional descriptions about the binary prov:actedOnBehalfOf relation from a performing prov:Agent to some prov:Agent for whom it was performed. For example, :mixing prov:wasAssociatedWith :toddler . :toddler prov:actedOnBehalfOf :mother; prov:qualifiedDelegation [ a prov:Delegation; prov:entity :mother; :foo :bar ].</rdfs:comment>
        <rdfs:isDefinedBy rdf:resource="http://www.w3.org/ns/prov-o#"/>
        <rdfs:label>Delegation</rdfs:label>
        <prov:category>qualified</prov:category>
        <prov:component>agents-responsibility</prov:component>
        <prov:definition xml:lang="en">Delegation is the assignment of authority and responsibility to an agent (by itself or by another agent) to carry out a specific activity as a delegate or representative, while the agent it acts on behalf of retains some responsibility for the outcome of the delegated work.

For example, a student acted on behalf of his supervisor, who acted on behalf of the department chair, who acted on behalf of the university; all those agents are responsible in some way for the activity that took place but we do not say explicitly who bears responsibility and to what degree.</prov:definition>
        <prov:dm rdf:datatype="http://www.w3.org/2001/XMLSchema#anyURI">http://www.w3.org/TR/2013/REC-prov-dm-20130430/#term-delegation</prov:dm>
        <prov:n rdf:datatype="http://www.w3.org/2001/XMLSchema#anyURI">http://www.w3.org/TR/2013/REC-prov-n-20130430/#expression-delegation</prov:n>
        <prov:unqualifiedForm rdf:resource="http://www.w3.org/ns/prov#actedOnBehalfOf"/>
    </owl:Class>
    


    <!-- http://www.w3.org/ns/prov#Derivation -->

    <owl:Class rdf:about="http://www.w3.org/ns/prov#Derivation">
        <rdfs:subClassOf rdf:resource="http://www.w3.org/ns/prov#EntityInfluence"/>
        <rdfs:comment xml:lang="en">An instance of prov:Derivation provides additional descriptions about the binary prov:wasDerivedFrom relation from some derived prov:Entity to another prov:Entity from which it was derived. For example, :chewed_bubble_gum prov:wasDerivedFrom :unwrapped_bubble_gum; prov:qualifiedDerivation [ a prov:Derivation; prov:entity :unwrapped_bubble_gum; :foo :bar ].</rdfs:comment>
        <rdfs:comment xml:lang="en">The more specific forms of prov:Derivation (i.e., prov:Revision, prov:Quotation, prov:PrimarySource) should be asserted if they apply.</rdfs:comment>
        <rdfs:isDefinedBy rdf:resource="http://www.w3.org/ns/prov-o#"/>
        <rdfs:label>Derivation</rdfs:label>
        <prov:category>qualified</prov:category>
        <prov:component>derivations</prov:component>
        <prov:constraints rdf:datatype="http://www.w3.org/2001/XMLSchema#anyURI">http://www.w3.org/TR/2013/REC-prov-constraints-20130430/#prov-dm-constraints-fig</prov:constraints>
        <prov:definition xml:lang="en">A derivation is a transformation of an entity into another, an update of an entity resulting in a new one, or the construction of a new entity based on a pre-existing entity.</prov:definition>
        <prov:dm rdf:datatype="http://www.w3.org/2001/XMLSchema#anyURI">http://www.w3.org/TR/2013/REC-prov-dm-20130430/#term-Derivation</prov:dm>
        <prov:n rdf:datatype="http://www.w3.org/2001/XMLSchema#anyURI">http://www.w3.org/TR/2013/REC-prov-n-20130430/#Derivation-Relation</prov:n>
        <prov:unqualifiedForm rdf:resource="http://www.w3.org/ns/prov#wasDerivedFrom"/>
    </owl:Class>
    


    <!-- http://www.w3.org/ns/prov#EmptyCollection -->

    <owl:Class rdf:about="http://www.w3.org/ns/prov#EmptyCollection">
        <rdfs:subClassOf rdf:resource="http://www.w3.org/ns/prov#Collection"/>
    </owl:Class>
    


    <!-- http://www.w3.org/ns/prov#End -->

    <owl:Class rdf:about="http://www.w3.org/ns/prov#End">
        <rdfs:subClassOf rdf:resource="http://www.w3.org/ns/prov#EntityInfluence"/>
        <rdfs:subClassOf rdf:resource="http://www.w3.org/ns/prov#InstantaneousEvent"/>
        <rdfs:comment xml:lang="en">An instance of prov:End provides additional descriptions about the binary prov:wasEndedBy relation from some ended prov:Activity to an prov:Entity that ended it. For example, :ball_game prov:wasEndedBy :buzzer; prov:qualifiedEnd [ a prov:End; prov:entity :buzzer; :foo :bar; prov:atTime &apos;2012-03-09T08:05:08-05:00&apos;^^xsd:dateTime ].</rdfs:comment>
        <rdfs:isDefinedBy rdf:resource="http://www.w3.org/ns/prov-o#"/>
        <rdfs:label>End</rdfs:label>
        <prov:category>qualified</prov:category>
        <prov:component>entities-activities</prov:component>
        <prov:constraints rdf:datatype="http://www.w3.org/2001/XMLSchema#anyURI">http://www.w3.org/TR/2013/REC-prov-constraints-20130430/#prov-dm-constraints-fig</prov:constraints>
        <prov:definition xml:lang="en">End is when an activity is deemed to have been ended by an entity, known as trigger. The activity no longer exists after its end. Any usage, generation, or invalidation involving an activity precedes the activity&apos;s end. An end may refer to a trigger entity that terminated the activity, or to an activity, known as ender that generated the trigger.</prov:definition>
        <prov:dm rdf:datatype="http://www.w3.org/2001/XMLSchema#anyURI">http://www.w3.org/TR/2013/REC-prov-dm-20130430/#term-End</prov:dm>
        <prov:n rdf:datatype="http://www.w3.org/2001/XMLSchema#anyURI">http://www.w3.org/TR/2013/REC-prov-n-20130430/#expression-End</prov:n>
        <prov:unqualifiedForm rdf:resource="http://www.w3.org/ns/prov#wasEndedBy"/>
    </owl:Class>
    


    <!-- http://www.w3.org/ns/prov#Entity -->

    <owl:Class rdf:about="http://www.w3.org/ns/prov#Entity">
        <owl:disjointWith rdf:resource="http://www.w3.org/ns/prov#InstantaneousEvent"/>
        <rdfs:isDefinedBy rdf:resource="http://www.w3.org/ns/prov-o#"/>
        <rdfs:label>Entity</rdfs:label>
        <prov:category>starting-point</prov:category>
        <prov:component>entities-activities</prov:component>
        <prov:constraints rdf:datatype="http://www.w3.org/2001/XMLSchema#anyURI">http://www.w3.org/TR/2013/REC-prov-constraints-20130430/#prov-dm-constraints-fig</prov:constraints>
        <prov:definition xml:lang="en">An entity is a physical, digital, conceptual, or other kind of thing with some fixed aspects; entities may be real or imaginary. </prov:definition>
        <prov:dm rdf:datatype="http://www.w3.org/2001/XMLSchema#anyURI">http://www.w3.org/TR/2013/REC-prov-dm-20130430/#term-entity</prov:dm>
        <prov:n rdf:datatype="http://www.w3.org/2001/XMLSchema#anyURI">http://www.w3.org/TR/2013/REC-prov-n-20130430/#expression-Entity</prov:n>
    </owl:Class>
    


    <!-- http://www.w3.org/ns/prov#EntityInfluence -->

    <owl:Class rdf:about="http://www.w3.org/ns/prov#EntityInfluence">
        <rdfs:subClassOf rdf:resource="http://www.w3.org/ns/prov#Influence"/>
        <rdfs:comment xml:lang="en">EntityInfluence provides additional descriptions of an Entity&apos;s binary influence upon any other kind of resource. Instances of EntityInfluence use the prov:entity property to cite the influencing Entity.</rdfs:comment>
        <rdfs:comment xml:lang="en">It is not recommended that the type EntityInfluence be asserted without also asserting one of its more specific subclasses.</rdfs:comment>
        <rdfs:isDefinedBy rdf:resource="http://www.w3.org/ns/prov-o#"/>
        <rdfs:label>EntityInfluence</rdfs:label>
        <rdfs:seeAlso rdf:resource="http://www.w3.org/ns/prov#entity"/>
        <prov:category>qualified</prov:category>
        <prov:editorsDefinition xml:lang="en">EntityInfluence is the capacity of an entity to have an effect on the character, development, or behavior of another by means of usage, start, end, derivation, or other. </prov:editorsDefinition>
    </owl:Class>
    


    <!-- http://www.w3.org/ns/prov#Generation -->

    <owl:Class rdf:about="http://www.w3.org/ns/prov#Generation">
        <rdfs:subClassOf rdf:resource="http://www.w3.org/ns/prov#ActivityInfluence"/>
        <rdfs:subClassOf rdf:resource="http://www.w3.org/ns/prov#InstantaneousEvent"/>
        <rdfs:comment xml:lang="en">An instance of prov:Generation provides additional descriptions about the binary prov:wasGeneratedBy relation from a generated prov:Entity to the prov:Activity that generated it. For example, :cake prov:wasGeneratedBy :baking; prov:qualifiedGeneration [ a prov:Generation; prov:activity :baking; :foo :bar ].</rdfs:comment>
        <rdfs:isDefinedBy rdf:resource="http://www.w3.org/ns/prov-o#"/>
        <rdfs:label>Generation</rdfs:label>
        <prov:category>qualified</prov:category>
        <prov:component>entities-activities</prov:component>
        <prov:constraints rdf:datatype="http://www.w3.org/2001/XMLSchema#anyURI">http://www.w3.org/TR/2013/REC-prov-constraints-20130430/#prov-dm-constraints-fig</prov:constraints>
        <prov:definition xml:lang="en">Generation is the completion of production of a new entity by an activity. This entity did not exist before generation and becomes available for usage after this generation.</prov:definition>
        <prov:dm rdf:datatype="http://www.w3.org/2001/XMLSchema#anyURI">http://www.w3.org/TR/2013/REC-prov-dm-20130430/#term-Generation</prov:dm>
        <prov:n rdf:datatype="http://www.w3.org/2001/XMLSchema#anyURI">http://www.w3.org/TR/2013/REC-prov-n-20130430/#expression-Generation</prov:n>
        <prov:unqualifiedForm rdf:resource="http://www.w3.org/ns/prov#wasGeneratedBy"/>
    </owl:Class>
    


    <!-- http://www.w3.org/ns/prov#Influence -->

    <owl:Class rdf:about="http://www.w3.org/ns/prov#Influence">
        <rdfs:comment xml:lang="en">An instance of prov:Influence provides additional descriptions about the binary prov:wasInfluencedBy relation from some influenced Activity, Entity, or Agent to the influencing Activity, Entity, or Agent. For example, :stomach_ache prov:wasInfluencedBy :spoon; prov:qualifiedInfluence [ a prov:Influence; prov:entity :spoon; :foo :bar ] . Because prov:Influence is a broad relation, the more specific relations (Communication, Delegation, End, etc.) should be used when applicable.</rdfs:comment>
        <rdfs:comment xml:lang="en">Because prov:Influence is a broad relation, its most specific subclasses (e.g. prov:Communication, prov:Delegation, prov:End, prov:Revision, etc.) should be used when applicable.</rdfs:comment>
        <rdfs:isDefinedBy rdf:resource="http://www.w3.org/ns/prov-o#"/>
        <rdfs:label>Influence</rdfs:label>
        <prov:category>qualified</prov:category>
        <prov:component>derivations</prov:component>
        <prov:definition xml:lang="en">Influence is the capacity of an entity, activity, or agent to have an effect on the character, development, or behavior of another by means of usage, start, end, generation, invalidation, communication, derivation, attribution, association, or delegation.</prov:definition>
        <prov:dm rdf:datatype="http://www.w3.org/2001/XMLSchema#anyURI">http://www.w3.org/TR/2013/REC-prov-dm-20130430/#term-influence</prov:dm>
        <prov:n rdf:datatype="http://www.w3.org/2001/XMLSchema#anyURI">http://www.w3.org/TR/2013/REC-prov-n-20130430/#expression-influence</prov:n>
        <prov:unqualifiedForm rdf:resource="http://www.w3.org/ns/prov#wasInfluencedBy"/>
    </owl:Class>
    


    <!-- http://www.w3.org/ns/prov#InstantaneousEvent -->

    <owl:Class rdf:about="http://www.w3.org/ns/prov#InstantaneousEvent">
        <rdfs:comment xml:lang="en">An instantaneous event, or event for short, happens in the world and marks a change in the world, in its activities and in its entities. The term &apos;event&apos; is commonly used in process algebra with a similar meaning. Events represent communications or interactions; they are assumed to be atomic and instantaneous.</rdfs:comment>
        <rdfs:isDefinedBy rdf:resource="http://www.w3.org/ns/prov-o#"/>
        <rdfs:label>InstantaneousEvent</rdfs:label>
        <prov:category>qualified</prov:category>
        <prov:component>entities-activities</prov:component>
        <prov:constraints rdf:datatype="http://www.w3.org/2001/XMLSchema#anyURI">http://www.w3.org/TR/2013/REC-prov-constraints-20130430/#dfn-event</prov:constraints>
        <prov:definition xml:lang="en">The PROV data model is implicitly based on a notion of instantaneous events (or just events), that mark transitions in the world. Events include generation, usage, or invalidation of entities, as well as starting or ending of activities. This notion of event is not first-class in the data model, but it is useful for explaining its other concepts and its semantics.</prov:definition>
    </owl:Class>
    


    <!-- http://www.w3.org/ns/prov#Invalidation -->

    <owl:Class rdf:about="http://www.w3.org/ns/prov#Invalidation">
        <rdfs:subClassOf rdf:resource="http://www.w3.org/ns/prov#ActivityInfluence"/>
        <rdfs:subClassOf rdf:resource="http://www.w3.org/ns/prov#InstantaneousEvent"/>
        <rdfs:comment xml:lang="en">An instance of prov:Invalidation provides additional descriptions about the binary prov:wasInvalidatedBy relation from an invalidated prov:Entity to the prov:Activity that invalidated it. For example, :uncracked_egg prov:wasInvalidatedBy :baking; prov:qualifiedInvalidation [ a prov:Invalidation; prov:activity :baking; :foo :bar ].</rdfs:comment>
        <rdfs:isDefinedBy rdf:resource="http://www.w3.org/ns/prov-o#"/>
        <rdfs:label>Invalidation</rdfs:label>
        <prov:category>qualified</prov:category>
        <prov:component>entities-activities</prov:component>
        <prov:constraints rdf:datatype="http://www.w3.org/2001/XMLSchema#anyURI">http://www.w3.org/TR/2013/REC-prov-constraints-20130430/#prov-dm-constraints-fig</prov:constraints>
        <prov:definition>Invalidation is the start of the destruction, cessation, or expiry of an existing entity by an activity. The entity is no longer available for use (or further invalidation) after invalidation. Any generation or usage of an entity precedes its invalidation.</prov:definition>
        <prov:dm rdf:datatype="http://www.w3.org/2001/XMLSchema#anyURI">http://www.w3.org/TR/2013/REC-prov-dm-20130430/#term-Invalidation</prov:dm>
        <prov:n rdf:datatype="http://www.w3.org/2001/XMLSchema#anyURI">http://www.w3.org/TR/2013/REC-prov-n-20130430/#expression-Invalidation</prov:n>
        <prov:unqualifiedForm rdf:resource="http://www.w3.org/ns/prov#wasInvalidatedBy"/>
    </owl:Class>
    


    <!-- http://www.w3.org/ns/prov#Location -->

    <owl:Class rdf:about="http://www.w3.org/ns/prov#Location">
        <rdfs:isDefinedBy rdf:resource="http://www.w3.org/ns/prov-o#"/>
        <rdfs:label>Location</rdfs:label>
        <rdfs:seeAlso rdf:resource="http://www.w3.org/ns/prov#atLocation"/>
        <prov:category>expanded</prov:category>
        <prov:definition xml:lang="en">A location can be an identifiable geographic place (ISO 19112), but it can also be a non-geographic place such as a directory, row, or column. As such, there are numerous ways in which location can be expressed, such as by a coordinate, address, landmark, and so forth.</prov:definition>
        <prov:dm rdf:datatype="http://www.w3.org/2001/XMLSchema#anyURI">http://www.w3.org/TR/2013/REC-prov-dm-20130430/#term-attribute-location</prov:dm>
        <prov:n rdf:datatype="http://www.w3.org/2001/XMLSchema#anyURI">http://www.w3.org/TR/2013/REC-prov-n-20130430/#expression-attribute</prov:n>
    </owl:Class>
    


    <!-- http://www.w3.org/ns/prov#Organization -->

    <owl:Class rdf:about="http://www.w3.org/ns/prov#Organization">
        <owl:equivalentClass rdf:resource="http://xmlns.com/foaf/0.1/Organization"/>
        <owl:equivalentClass rdf:resource="https://schema.org/Organization"/>
        <rdfs:subClassOf rdf:resource="http://www.w3.org/ns/prov#Agent"/>
        <rdfs:isDefinedBy rdf:resource="http://www.w3.org/ns/prov-o#"/>
        <rdfs:label>Organization</rdfs:label>
        <prov:category>expanded</prov:category>
        <prov:component>agents-responsibility</prov:component>
        <prov:definition>An organization is a social or legal institution such as a company, society, etc.</prov:definition>
        <prov:dm rdf:datatype="http://www.w3.org/2001/XMLSchema#anyURI">http://www.w3.org/TR/2013/REC-prov-dm-20130430/#term-agent</prov:dm>
        <prov:n rdf:datatype="http://www.w3.org/2001/XMLSchema#anyURI">http://www.w3.org/TR/2013/REC-prov-n-20130430/#expression-types</prov:n>
    </owl:Class>
    


    <!-- http://www.w3.org/ns/prov#Person -->

    <owl:Class rdf:about="http://www.w3.org/ns/prov#Person">
        <rdfs:subClassOf rdf:resource="http://www.w3.org/ns/prov#Agent"/>
        <rdfs:isDefinedBy rdf:resource="http://www.w3.org/ns/prov-o#"/>
        <rdfs:label>Person</rdfs:label>
        <prov:category>expanded</prov:category>
        <prov:component>agents-responsibility</prov:component>
        <prov:definition xml:lang="en">Person agents are people.</prov:definition>
        <prov:dm rdf:datatype="http://www.w3.org/2001/XMLSchema#anyURI">http://www.w3.org/TR/2013/REC-prov-dm-20130430/#term-agent</prov:dm>
        <prov:n rdf:datatype="http://www.w3.org/2001/XMLSchema#anyURI">http://www.w3.org/TR/2013/REC-prov-n-20130430/#expression-types</prov:n>
    </owl:Class>
    


    <!-- http://www.w3.org/ns/prov#Plan -->

    <owl:Class rdf:about="http://www.w3.org/ns/prov#Plan">
        <rdfs:subClassOf rdf:resource="http://www.w3.org/ns/prov#Entity"/>
        <rdfs:comment xml:lang="en">There exist no prescriptive requirement on the nature of plans, their representation, the actions or steps they consist of, or their intended goals. Since plans may evolve over time, it may become necessary to track their provenance, so plans themselves are entities. Representing the plan explicitly in the provenance can be useful for various tasks: for example, to validate the execution as represented in the provenance record, to manage expectation failures, or to provide explanations.</rdfs:comment>
        <rdfs:isDefinedBy rdf:resource="http://www.w3.org/ns/prov-o#"/>
        <rdfs:label>Plan</rdfs:label>
        <prov:category>expanded</prov:category>
        <prov:category>qualified</prov:category>
        <prov:component>agents-responsibility</prov:component>
        <prov:definition>A plan is an entity that represents a set of actions or steps intended by one or more agents to achieve some goals.</prov:definition>
        <prov:dm rdf:datatype="http://www.w3.org/2001/XMLSchema#anyURI">http://www.w3.org/TR/2013/REC-prov-dm-20130430/#term-Association</prov:dm>
        <prov:n rdf:datatype="http://www.w3.org/2001/XMLSchema#anyURI">http://www.w3.org/TR/2013/REC-prov-n-20130430/#expression-Association</prov:n>
    </owl:Class>
    


    <!-- http://www.w3.org/ns/prov#PrimarySource -->

    <owl:Class rdf:about="http://www.w3.org/ns/prov#PrimarySource">
        <rdfs:subClassOf rdf:resource="http://www.w3.org/ns/prov#Derivation"/>
        <rdfs:comment xml:lang="en">An instance of prov:PrimarySource provides additional descriptions about the binary prov:hadPrimarySource relation from some secondary prov:Entity to an earlier, primary prov:Entity. For example, :blog prov:hadPrimarySource :newsArticle; prov:qualifiedPrimarySource [ a prov:PrimarySource; prov:entity :newsArticle; :foo :bar ] .</rdfs:comment>
        <rdfs:isDefinedBy rdf:resource="http://www.w3.org/ns/prov-o#"/>
        <rdfs:label>PrimarySource</rdfs:label>
        <prov:category>qualified</prov:category>
        <prov:component>derivations</prov:component>
        <prov:definition xml:lang="en">A primary source for a topic refers to something produced by some agent with direct experience and knowledge about the topic, at the time of the topic&apos;s study, without benefit from hindsight.

Because of the directness of primary sources, they &apos;speak for themselves&apos; in ways that cannot be captured through the filter of secondary sources. As such, it is important for secondary sources to reference those primary sources from which they were derived, so that their reliability can be investigated.

A primary source relation is a particular case of derivation of secondary materials from their primary sources. It is recognized that the determination of primary sources can be up to interpretation, and should be done according to conventions accepted within the application&apos;s domain.</prov:definition>
        <prov:dm rdf:datatype="http://www.w3.org/2001/XMLSchema#anyURI">http://www.w3.org/TR/2013/REC-prov-dm-20130430/#term-primary-source</prov:dm>
        <prov:n rdf:datatype="http://www.w3.org/2001/XMLSchema#anyURI">http://www.w3.org/TR/2013/REC-prov-n-20130430/#expression-original-source</prov:n>
        <prov:unqualifiedForm rdf:resource="http://www.w3.org/ns/prov#hadPrimarySource"/>
    </owl:Class>
    


    <!-- http://www.w3.org/ns/prov#Quotation -->

    <owl:Class rdf:about="http://www.w3.org/ns/prov#Quotation">
        <rdfs:subClassOf rdf:resource="http://www.w3.org/ns/prov#Derivation"/>
        <rdfs:comment xml:lang="en">An instance of prov:Quotation provides additional descriptions about the binary prov:wasQuotedFrom relation from some taken prov:Entity from an earlier, larger prov:Entity. For example, :here_is_looking_at_you_kid prov:wasQuotedFrom :casablanca_script; prov:qualifiedQuotation [ a prov:Quotation; prov:entity :casablanca_script; :foo :bar ].</rdfs:comment>
        <rdfs:isDefinedBy rdf:resource="http://www.w3.org/ns/prov-o#"/>
        <rdfs:label>Quotation</rdfs:label>
        <prov:category>qualified</prov:category>
        <prov:component>derivations</prov:component>
        <prov:definition xml:lang="en">A quotation is the repeat of (some or all of) an entity, such as text or image, by someone who may or may not be its original author. Quotation is a particular case of derivation.</prov:definition>
        <prov:dm rdf:datatype="http://www.w3.org/2001/XMLSchema#anyURI">http://www.w3.org/TR/2013/REC-prov-dm-20130430/#term-quotation</prov:dm>
        <prov:n rdf:datatype="http://www.w3.org/2001/XMLSchema#anyURI">http://www.w3.org/TR/2013/REC-prov-n-20130430/#expression-quotation</prov:n>
        <prov:unqualifiedForm rdf:resource="http://www.w3.org/ns/prov#wasQuotedFrom"/>
    </owl:Class>
    


    <!-- http://www.w3.org/ns/prov#Revision -->

    <owl:Class rdf:about="http://www.w3.org/ns/prov#Revision">
        <rdfs:subClassOf rdf:resource="http://www.w3.org/ns/prov#Derivation"/>
        <rdfs:comment xml:lang="en">An instance of prov:Revision provides additional descriptions about the binary prov:wasRevisionOf relation from some newer prov:Entity to an earlier prov:Entity. For example, :draft_2 prov:wasRevisionOf :draft_1; prov:qualifiedRevision [ a prov:Revision; prov:entity :draft_1; :foo :bar ].</rdfs:comment>
        <rdfs:isDefinedBy rdf:resource="http://www.w3.org/ns/prov-o#"/>
        <rdfs:label>Revision</rdfs:label>
        <prov:category>qualified</prov:category>
        <prov:component>derivations</prov:component>
        <prov:definition xml:lang="en">A revision is a derivation for which the resulting entity is a revised version of some original. The implication here is that the resulting entity contains substantial content from the original. Revision is a particular case of derivation.</prov:definition>
        <prov:dm rdf:datatype="http://www.w3.org/2001/XMLSchema#anyURI">http://www.w3.org/TR/2013/REC-prov-dm-20130430/#term-revision</prov:dm>
        <prov:n rdf:datatype="http://www.w3.org/2001/XMLSchema#anyURI">http://www.w3.org/TR/2013/REC-prov-n-20130430/#expression-Revision</prov:n>
        <prov:unqualifiedForm rdf:resource="http://www.w3.org/ns/prov#wasRevisionOf"/>
    </owl:Class>
    


    <!-- http://www.w3.org/ns/prov#Role -->

    <owl:Class rdf:about="http://www.w3.org/ns/prov#Role">
        <rdfs:isDefinedBy rdf:resource="http://www.w3.org/ns/prov-o#"/>
        <rdfs:label>Role</rdfs:label>
        <rdfs:seeAlso rdf:resource="http://www.w3.org/ns/prov#hadRole"/>
        <prov:category>qualified</prov:category>
        <prov:component>agents-responsibility</prov:component>
        <prov:definition xml:lang="en">A role is the function of an entity or agent with respect to an activity, in the context of a usage, generation, invalidation, association, start, and end.</prov:definition>
        <prov:dm rdf:datatype="http://www.w3.org/2001/XMLSchema#anyURI">http://www.w3.org/TR/2013/REC-prov-dm-20130430/#term-attribute-role</prov:dm>
        <prov:n rdf:datatype="http://www.w3.org/2001/XMLSchema#anyURI">http://www.w3.org/TR/2013/REC-prov-n-20130430/#expression-attribute</prov:n>
    </owl:Class>
    


    <!-- http://www.w3.org/ns/prov#SoftwareAgent -->

    <owl:Class rdf:about="http://www.w3.org/ns/prov#SoftwareAgent">
        <rdfs:subClassOf rdf:resource="http://www.w3.org/ns/prov#Agent"/>
        <rdfs:isDefinedBy rdf:resource="http://www.w3.org/ns/prov-o#"/>
        <rdfs:label>SoftwareAgent</rdfs:label>
        <prov:category>expanded</prov:category>
        <prov:component>agents-responsibility</prov:component>
        <prov:definition xml:lang="en">A software agent is running software.</prov:definition>
        <prov:dm rdf:datatype="http://www.w3.org/2001/XMLSchema#anyURI">http://www.w3.org/TR/2013/REC-prov-dm-20130430/#term-agent</prov:dm>
        <prov:n rdf:datatype="http://www.w3.org/2001/XMLSchema#anyURI">http://www.w3.org/TR/2013/REC-prov-n-20130430/#expression-types</prov:n>
    </owl:Class>
    


    <!-- http://www.w3.org/ns/prov#Start -->

    <owl:Class rdf:about="http://www.w3.org/ns/prov#Start">
        <rdfs:subClassOf rdf:resource="http://www.w3.org/ns/prov#EntityInfluence"/>
        <rdfs:subClassOf rdf:resource="http://www.w3.org/ns/prov#InstantaneousEvent"/>
        <rdfs:comment xml:lang="en">An instance of prov:Start provides additional descriptions about the binary prov:wasStartedBy relation from some started prov:Activity to an prov:Entity that started it. For example, :foot_race prov:wasStartedBy :bang; prov:qualifiedStart [ a prov:Start; prov:entity :bang; :foo :bar; prov:atTime &apos;2012-03-09T08:05:08-05:00&apos;^^xsd:dateTime ] .</rdfs:comment>
        <rdfs:isDefinedBy rdf:resource="http://www.w3.org/ns/prov-o#"/>
        <rdfs:label>Start</rdfs:label>
        <prov:category>qualified</prov:category>
        <prov:component>entities-activities</prov:component>
        <prov:constraints rdf:datatype="http://www.w3.org/2001/XMLSchema#anyURI">http://www.w3.org/TR/2013/REC-prov-constraints-20130430/#prov-dm-constraints-fig</prov:constraints>
        <prov:definition xml:lang="en">Start is when an activity is deemed to have been started by an entity, known as trigger. The activity did not exist before its start. Any usage, generation, or invalidation involving an activity follows the activity&apos;s start. A start may refer to a trigger entity that set off the activity, or to an activity, known as starter, that generated the trigger.</prov:definition>
        <prov:dm rdf:datatype="http://www.w3.org/2001/XMLSchema#anyURI">http://www.w3.org/TR/2013/REC-prov-dm-20130430/#term-Start</prov:dm>
        <prov:n rdf:datatype="http://www.w3.org/2001/XMLSchema#anyURI">http://www.w3.org/TR/2013/REC-prov-n-20130430/#expression-Start</prov:n>
        <prov:unqualifiedForm rdf:resource="http://www.w3.org/ns/prov#wasStartedBy"/>
    </owl:Class>
    


    <!-- http://www.w3.org/ns/prov#Usage -->

    <owl:Class rdf:about="http://www.w3.org/ns/prov#Usage">
        <rdfs:subClassOf rdf:resource="http://www.w3.org/ns/prov#EntityInfluence"/>
        <rdfs:subClassOf rdf:resource="http://www.w3.org/ns/prov#InstantaneousEvent"/>
        <rdfs:comment xml:lang="en">An instance of prov:Usage provides additional descriptions about the binary prov:used relation from some prov:Activity to an prov:Entity that it used. For example, :keynote prov:used :podium; prov:qualifiedUsage [ a prov:Usage; prov:entity :podium; :foo :bar ].</rdfs:comment>
        <rdfs:isDefinedBy rdf:resource="http://www.w3.org/ns/prov-o#"/>
        <rdfs:label>Usage</rdfs:label>
        <prov:category>qualified</prov:category>
        <prov:component>entities-activities</prov:component>
        <prov:constraints rdf:datatype="http://www.w3.org/2001/XMLSchema#anyURI">http://www.w3.org/TR/2013/REC-prov-constraints-20130430/#prov-dm-constraints-fig</prov:constraints>
        <prov:definition xml:lang="en">Usage is the beginning of utilizing an entity by an activity. Before usage, the activity had not begun to utilize this entity and could not have been affected by the entity.</prov:definition>
        <prov:dm rdf:datatype="http://www.w3.org/2001/XMLSchema#anyURI">http://www.w3.org/TR/2013/REC-prov-dm-20130430/#term-Usage</prov:dm>
        <prov:n rdf:datatype="http://www.w3.org/2001/XMLSchema#anyURI">http://www.w3.org/TR/2013/REC-prov-n-20130430/#expression-Usage</prov:n>
        <prov:unqualifiedForm rdf:resource="http://www.w3.org/ns/prov#used"/>
    </owl:Class>
    


    <!-- http://xmlns.com/foaf/0.1/Agent -->

    <owl:Class rdf:about="http://xmlns.com/foaf/0.1/Agent">
        <rdfs:comment>An agent (eg. person, group, software or physical artifact).</rdfs:comment>
        <rdfs:label>Agent</rdfs:label>
        <ns:term_status>stable</ns:term_status>
    </owl:Class>
    


    <!-- http://xmlns.com/foaf/0.1/Document -->

    <owl:Class rdf:about="http://xmlns.com/foaf/0.1/Document">
        <owl:disjointWith rdf:resource="http://xmlns.com/foaf/0.1/Organization"/>
        <owl:disjointWith rdf:resource="http://xmlns.com/foaf/0.1/Project"/>
        <rdfs:comment>A document.</rdfs:comment>
        <rdfs:isDefinedBy rdf:resource="http://xmlns.com/foaf/0.1/"/>
        <rdfs:label>Document</rdfs:label>
        <ns:term_status>stable</ns:term_status>
    </owl:Class>
    


    <!-- http://xmlns.com/foaf/0.1/Group -->

    <owl:Class rdf:about="http://xmlns.com/foaf/0.1/Group">
        <rdfs:subClassOf rdf:resource="http://xmlns.com/foaf/0.1/Agent"/>
        <rdfs:comment>A class of Agents.</rdfs:comment>
        <rdfs:label>Group</rdfs:label>
        <ns:term_status>stable</ns:term_status>
    </owl:Class>
    


    <!-- http://xmlns.com/foaf/0.1/Image -->

    <owl:Class rdf:about="http://xmlns.com/foaf/0.1/Image">
        <rdfs:subClassOf rdf:resource="http://xmlns.com/foaf/0.1/Document"/>
        <rdfs:comment>An image.</rdfs:comment>
        <rdfs:isDefinedBy rdf:resource="http://xmlns.com/foaf/0.1/"/>
        <rdfs:label>Image</rdfs:label>
        <ns:term_status>stable</ns:term_status>
    </owl:Class>
    


    <!-- http://xmlns.com/foaf/0.1/LabelProperty -->

    <owl:Class rdf:about="http://xmlns.com/foaf/0.1/LabelProperty">
        <rdfs:comment>A foaf:LabelProperty is any RDF property with texual values that serve as labels.</rdfs:comment>
        <rdfs:isDefinedBy rdf:resource="http://xmlns.com/foaf/0.1/"/>
        <rdfs:label>Label Property</rdfs:label>
        <ns:term_status>unstable</ns:term_status>
    </owl:Class>
    


    <!-- http://xmlns.com/foaf/0.1/OnlineAccount -->

    <owl:Class rdf:about="http://xmlns.com/foaf/0.1/OnlineAccount">
        <rdfs:subClassOf rdf:resource="http://www.w3.org/2002/07/owl#Thing"/>
        <rdfs:comment>An online account.</rdfs:comment>
        <rdfs:isDefinedBy rdf:resource="http://xmlns.com/foaf/0.1/"/>
        <rdfs:label>Online Account</rdfs:label>
        <ns:term_status>testing</ns:term_status>
    </owl:Class>
    


    <!-- http://xmlns.com/foaf/0.1/OnlineChatAccount -->

    <owl:Class rdf:about="http://xmlns.com/foaf/0.1/OnlineChatAccount">
        <rdfs:subClassOf rdf:resource="http://xmlns.com/foaf/0.1/OnlineAccount"/>
        <rdfs:comment>An online chat account.</rdfs:comment>
        <rdfs:isDefinedBy rdf:resource="http://xmlns.com/foaf/0.1/"/>
        <rdfs:label>Online Chat Account</rdfs:label>
        <ns:term_status>unstable</ns:term_status>
    </owl:Class>
    


    <!-- http://xmlns.com/foaf/0.1/OnlineEcommerceAccount -->

    <owl:Class rdf:about="http://xmlns.com/foaf/0.1/OnlineEcommerceAccount">
        <rdfs:subClassOf rdf:resource="http://xmlns.com/foaf/0.1/OnlineAccount"/>
        <rdfs:comment>An online e-commerce account.</rdfs:comment>
        <rdfs:isDefinedBy rdf:resource="http://xmlns.com/foaf/0.1/"/>
        <rdfs:label>Online E-commerce Account</rdfs:label>
        <ns:term_status>unstable</ns:term_status>
    </owl:Class>
    


    <!-- http://xmlns.com/foaf/0.1/OnlineGamingAccount -->

    <owl:Class rdf:about="http://xmlns.com/foaf/0.1/OnlineGamingAccount">
        <rdfs:subClassOf rdf:resource="http://xmlns.com/foaf/0.1/OnlineAccount"/>
        <rdfs:comment>An online gaming account.</rdfs:comment>
        <rdfs:isDefinedBy rdf:resource="http://xmlns.com/foaf/0.1/"/>
        <rdfs:label>Online Gaming Account</rdfs:label>
        <ns:term_status>unstable</ns:term_status>
    </owl:Class>
    


    <!-- http://xmlns.com/foaf/0.1/Organization -->

    <owl:Class rdf:about="http://xmlns.com/foaf/0.1/Organization">
        <rdfs:subClassOf rdf:resource="http://xmlns.com/foaf/0.1/Agent"/>
        <owl:disjointWith rdf:resource="http://xmlns.com/foaf/0.1/Person"/>
        <rdfs:comment>An organization.</rdfs:comment>
        <rdfs:isDefinedBy rdf:resource="http://xmlns.com/foaf/0.1/"/>
        <rdfs:label>Organization</rdfs:label>
        <ns:term_status>stable</ns:term_status>
    </owl:Class>
    


    <!-- http://xmlns.com/foaf/0.1/Person -->

    <owl:Class rdf:about="http://xmlns.com/foaf/0.1/Person">
        <rdfs:subClassOf rdf:resource="http://www.w3.org/2003/01/geo/wgs84_pos#SpatialThing"/>
        <rdfs:subClassOf rdf:resource="http://xmlns.com/foaf/0.1/Agent"/>
        <owl:disjointWith rdf:resource="http://xmlns.com/foaf/0.1/Project"/>
        <rdfs:comment>A person.</rdfs:comment>
        <rdfs:isDefinedBy rdf:resource="http://xmlns.com/foaf/0.1/"/>
        <rdfs:label>Person</rdfs:label>
        <ns:term_status>stable</ns:term_status>
    </owl:Class>
    


    <!-- http://xmlns.com/foaf/0.1/PersonalProfileDocument -->

    <owl:Class rdf:about="http://xmlns.com/foaf/0.1/PersonalProfileDocument">
        <rdfs:subClassOf rdf:resource="http://xmlns.com/foaf/0.1/Document"/>
        <rdfs:comment>A personal profile RDF document.</rdfs:comment>
        <rdfs:label>PersonalProfileDocument</rdfs:label>
        <ns:term_status>testing</ns:term_status>
    </owl:Class>
    


    <!-- http://xmlns.com/foaf/0.1/Project -->

    <owl:Class rdf:about="http://xmlns.com/foaf/0.1/Project">
        <rdfs:comment>A project (a collective endeavour of some kind).</rdfs:comment>
        <rdfs:isDefinedBy rdf:resource="http://xmlns.com/foaf/0.1/"/>
        <rdfs:label>Project</rdfs:label>
        <ns:term_status>testing</ns:term_status>
    </owl:Class>
    


    <!-- 
    ///////////////////////////////////////////////////////////////////////////////////////
    //
    // Individuals
    //
    ///////////////////////////////////////////////////////////////////////////////////////
     -->

    


    <!-- http://purl.org/dc/dcmitype/Collection -->

    <rdf:Description rdf:about="http://purl.org/dc/dcmitype/Collection">
        <rdf:type rdf:resource="http://purl.org/dc/terms/DCMIType"/>
        <dc:type rdf:resource="http://dublincore.org/usage/documents/principles/#vocabulary-term"/>
        <terms:hasVersion rdf:resource="http://dublincore.org/usage/terms/history/#Collection-001"/>
        <terms:issued>2000-07-11</terms:issued>
        <rdfs:comment xml:lang="en-us">A collection is an aggregation of items. The term 
            collection means that the resource is described as a 
            group; its parts may be separately described and navigated.</rdfs:comment>
        <rdfs:isDefinedBy rdf:resource="http://purl.org/dc/dcmitype/"/>
        <rdfs:label xml:lang="en-us">Collection</rdfs:label>
    </rdf:Description>
    


    <!-- http://purl.org/dc/dcmitype/Dataset -->

    <rdf:Description rdf:about="http://purl.org/dc/dcmitype/Dataset">
        <rdf:type rdf:resource="http://purl.org/dc/terms/DCMIType"/>
        <dc:type rdf:resource="http://dublincore.org/usage/documents/principles/#vocabulary-term"/>
        <terms:hasVersion rdf:resource="http://dublincore.org/usage/terms/history/#Dataset-001"/>
        <terms:issued>2000-07-11</terms:issued>
        <rdfs:comment xml:lang="en-us">A dataset is information encoded in a defined structure 
            (for example, lists, tables, and databases), intended to 
            be useful for direct machine processing.</rdfs:comment>
        <rdfs:isDefinedBy rdf:resource="http://purl.org/dc/dcmitype/"/>
        <rdfs:label xml:lang="en-us">Dataset</rdfs:label>
    </rdf:Description>
    


    <!-- http://purl.org/dc/dcmitype/Event -->

    <rdf:Description rdf:about="http://purl.org/dc/dcmitype/Event">
        <rdf:type rdf:resource="http://purl.org/dc/terms/DCMIType"/>
        <dc:type rdf:resource="http://dublincore.org/usage/documents/principles/#vocabulary-term"/>
        <terms:hasVersion rdf:resource="http://dublincore.org/usage/terms/history/#Event-001"/>
        <terms:issued>2000-07-11</terms:issued>
        <rdfs:comment xml:lang="en-us">An event is a non-persistent, time-based occurrence. 
            Metadata for an event provides descriptive
            information that is the basis for discovery of the
            purpose, location, duration, responsible agents, and
            links to related events and resources.  The resource
            of type event may not be retrievable if the described
            instantiation has expired or is yet to occur.
            Examples - exhibition, web-cast, conference,
            workshop, open-day, performance, battle, trial,
            wedding, tea-party, conflagration.</rdfs:comment>
        <rdfs:isDefinedBy rdf:resource="http://purl.org/dc/dcmitype/"/>
        <rdfs:label xml:lang="en-us">Event</rdfs:label>
    </rdf:Description>
    


    <!-- http://purl.org/dc/dcmitype/Image -->

    <rdf:Description rdf:about="http://purl.org/dc/dcmitype/Image">
        <rdf:type rdf:resource="http://purl.org/dc/terms/DCMIType"/>
        <dc:type rdf:resource="http://dublincore.org/usage/documents/principles/#vocabulary-term"/>
        <terms:hasVersion rdf:resource="http://dublincore.org/usage/terms/history/#Image-001"/>
        <terms:issued>2000-07-11</terms:issued>
        <rdfs:comment xml:lang="en-us">An image is a primarily symbolic visual representation 
            other than text. For example - images and photographs of 
            physical objects, paintings, prints, drawings, other 
            images and graphics, animations and moving pictures, 
            film, diagrams, maps, musical notation. Note that image 
            may include both electronic and physical representations.</rdfs:comment>
        <rdfs:isDefinedBy rdf:resource="http://purl.org/dc/dcmitype/"/>
        <rdfs:label xml:lang="en-us">Image</rdfs:label>
    </rdf:Description>
    


    <!-- http://purl.org/dc/dcmitype/InteractiveResource -->

    <rdf:Description rdf:about="http://purl.org/dc/dcmitype/InteractiveResource">
        <rdf:type rdf:resource="http://purl.org/dc/terms/DCMIType"/>
        <dc:type rdf:resource="http://dublincore.org/usage/documents/principles/#vocabulary-term"/>
        <terms:hasVersion rdf:resource="http://dublincore.org/usage/terms/history/#InteractiveResource-001"/>
        <terms:issued>2000-07-11</terms:issued>
        <rdfs:comment xml:lang="en-us">An interactive resource is a resource which requires 
            interaction from the user to be understood, executed, 
            or experienced. For example - forms on web pages, applets, 
            multimedia learning objects, chat services, virtual 
            reality.</rdfs:comment>
        <rdfs:isDefinedBy rdf:resource="http://purl.org/dc/dcmitype/"/>
        <rdfs:label xml:lang="en-us">Interactive Resource</rdfs:label>
    </rdf:Description>
    


    <!-- http://purl.org/dc/dcmitype/PhysicalObject -->

    <rdf:Description rdf:about="http://purl.org/dc/dcmitype/PhysicalObject">
        <rdf:type rdf:resource="http://purl.org/dc/terms/DCMIType"/>
        <dc:type rdf:resource="http://dublincore.org/usage/documents/principles/#vocabulary-term"/>
        <terms:hasVersion rdf:resource="http://dublincore.org/usage/terms/history/#PhysicalObject-001"/>
        <terms:issued>2002-07-13</terms:issued>
        <rdfs:comment xml:lang="en-us">An inanimate, three-dimensional object or substance.  
            For example -- a computer, the great pyramid, a 
            sculpture.  Note that digital representations 
            of, or surrogates for, these things should use Image, 
            Text or one of the other types.</rdfs:comment>
        <rdfs:isDefinedBy rdf:resource="http://purl.org/dc/dcmitype/"/>
        <rdfs:label xml:lang="en-us">Physical Object</rdfs:label>
    </rdf:Description>
    


    <!-- http://purl.org/dc/dcmitype/Service -->

    <rdf:Description rdf:about="http://purl.org/dc/dcmitype/Service">
        <rdf:type rdf:resource="http://purl.org/dc/terms/DCMIType"/>
        <dc:type rdf:resource="http://dublincore.org/usage/documents/principles/#vocabulary-term"/>
        <terms:hasVersion rdf:resource="http://dublincore.org/usage/terms/history/#Service-001"/>
        <terms:issued>2000-07-11</terms:issued>
        <rdfs:comment xml:lang="en-us">A service is a system that provides one or more 
            functions of value to the end-user. Examples include: 
            a photocopying service, a banking service, an 
            authentication service, interlibrary loans, a Z39.50 
            or Web server.</rdfs:comment>
        <rdfs:isDefinedBy rdf:resource="http://purl.org/dc/dcmitype/"/>
        <rdfs:label xml:lang="en-us">Service</rdfs:label>
    </rdf:Description>
    


    <!-- http://purl.org/dc/dcmitype/Software -->

    <rdf:Description rdf:about="http://purl.org/dc/dcmitype/Software">
        <rdf:type rdf:resource="http://purl.org/dc/terms/DCMIType"/>
        <dc:type rdf:resource="http://dublincore.org/usage/documents/principles/#vocabulary-term"/>
        <terms:hasVersion rdf:resource="http://dublincore.org/usage/terms/history/#Software-001"/>
        <terms:issued>2000-07-11</terms:issued>
        <rdfs:comment xml:lang="en-us">Software is a computer program in source or 
            compiled form which may be available for installation 
            non-transiently on another machine. For software which 
            exists only to create an interactive environment, use 
            interactive instead.</rdfs:comment>
        <rdfs:isDefinedBy rdf:resource="http://purl.org/dc/dcmitype/"/>
        <rdfs:label xml:lang="en-us">Software</rdfs:label>
    </rdf:Description>
    


    <!-- http://purl.org/dc/dcmitype/Sound -->

    <rdf:Description rdf:about="http://purl.org/dc/dcmitype/Sound">
        <rdf:type rdf:resource="http://purl.org/dc/terms/DCMIType"/>
        <dc:type rdf:resource="http://dublincore.org/usage/documents/principles/#vocabulary-term"/>
        <terms:hasVersion rdf:resource="http://dublincore.org/usage/terms/history/#Sound-001"/>
        <terms:issued>2000-07-11</terms:issued>
        <rdfs:comment xml:lang="en-us">A sound is a resource whose content is primarily 
            intended to be rendered as audio. For example - a 
            music playback file format, an audio compact disc, 
            and recorded speech or sounds.</rdfs:comment>
        <rdfs:isDefinedBy rdf:resource="http://purl.org/dc/dcmitype/"/>
        <rdfs:label xml:lang="en-us">Sound</rdfs:label>
    </rdf:Description>
    


    <!-- http://purl.org/dc/dcmitype/Text -->

    <rdf:Description rdf:about="http://purl.org/dc/dcmitype/Text">
        <rdf:type rdf:resource="http://purl.org/dc/terms/DCMIType"/>
        <dc:type rdf:resource="http://dublincore.org/usage/documents/principles/#vocabulary-term"/>
        <terms:hasVersion rdf:resource="http://dublincore.org/usage/terms/history/#Text-001"/>
        <terms:issued>2000-07-11</terms:issued>
        <rdfs:comment xml:lang="en-us">A text is a resource whose content is primarily 
            words for reading. For example - books, letters, 
            dissertations, poems, newspapers, articles, 
            archives of mailing lists. Note that facsimiles 
            or images of texts are still of the genre text.</rdfs:comment>
        <rdfs:isDefinedBy rdf:resource="http://purl.org/dc/dcmitype/"/>
        <rdfs:label xml:lang="en-us">Text</rdfs:label>
    </rdf:Description>
    


    <!-- http://purl.org/dc/terms/Box -->

    <rdf:Description rdf:about="http://purl.org/dc/terms/Box">
        <rdf:type rdf:resource="http://purl.org/dc/terms/SpatialScheme"/>
        <dc:type rdf:resource="http://dublincore.org/usage/documents/principles/#encoding-scheme"/>
        <terms:hasVersion rdf:resource="http://dublincore.org/usage/terms/history/#Box-002"/>
        <terms:issued>2000-07-11</terms:issued>
        <terms:modified>2002-06-15</terms:modified>
        <rdfs:comment xml:lang="en-us">The DCMI Box identifies a region of space using its geographic limits.</rdfs:comment>
        <rdfs:isDefinedBy rdf:resource="http://purl.org/dc/terms/"/>
        <rdfs:label xml:lang="en-us">DCMI Box</rdfs:label>
        <rdfs:seeAlso rdf:resource="http://dublincore.org/documents/dcmi-box/"/>
    </rdf:Description>
    


    <!-- http://purl.org/dc/terms/DDC -->

    <rdf:Description rdf:about="http://purl.org/dc/terms/DDC">
        <rdf:type rdf:resource="http://purl.org/dc/terms/SubjectScheme"/>
        <dc:type rdf:resource="http://dublincore.org/usage/documents/principles/#encoding-scheme"/>
        <terms:hasVersion rdf:resource="http://dublincore.org/usage/terms/history/#DDC-002"/>
        <terms:issued>2000-07-11</terms:issued>
        <terms:modified>2002-06-15</terms:modified>
        <rdfs:comment xml:lang="en-us">Dewey Decimal Classification</rdfs:comment>
        <rdfs:isDefinedBy rdf:resource="http://purl.org/dc/terms/"/>
        <rdfs:label xml:lang="en-us">DDC</rdfs:label>
        <rdfs:seeAlso rdf:resource="http://www.oclc.org/dewey/index.htm"/>
    </rdf:Description>
    


    <!-- http://purl.org/dc/terms/IMT -->

    <rdf:Description rdf:about="http://purl.org/dc/terms/IMT">
        <rdf:type rdf:resource="http://purl.org/dc/terms/FormatScheme"/>
        <dc:type rdf:resource="http://dublincore.org/usage/documents/principles/#encoding-scheme"/>
        <terms:hasVersion rdf:resource="http://dublincore.org/usage/terms/history/#IMT-002"/>
        <terms:issued>2000-07-11</terms:issued>
        <terms:modified>2002-06-15</terms:modified>
        <rdfs:comment xml:lang="en-us">The Internet media type of the resource.</rdfs:comment>
        <rdfs:isDefinedBy rdf:resource="http://purl.org/dc/terms/"/>
        <rdfs:label xml:lang="en-us">IMT</rdfs:label>
        <rdfs:seeAlso rdf:resource="http://www.isi.edu/in-notes/iana/assignments/media-types/media-types"/>
    </rdf:Description>
    


    <!-- http://purl.org/dc/terms/ISO3166 -->

    <rdf:Description rdf:about="http://purl.org/dc/terms/ISO3166">
        <rdf:type rdf:resource="http://purl.org/dc/terms/SpatialScheme"/>
        <dc:type rdf:resource="http://dublincore.org/usage/documents/principles/#encoding-scheme"/>
        <terms:hasVersion rdf:resource="http://dublincore.org/usage/terms/history/#ISO3166-002"/>
        <terms:issued>2000-07-11</terms:issued>
        <terms:modified>2002-06-15</terms:modified>
        <rdfs:comment xml:lang="en-us">ISO 3166 Codes for the representation of names of countries</rdfs:comment>
        <rdfs:isDefinedBy rdf:resource="http://purl.org/dc/terms/"/>
        <rdfs:label xml:lang="en-us">ISO 3166</rdfs:label>
        <rdfs:seeAlso rdf:resource="http://www.din.de/gremien/nas/nabd/iso3166ma/codlstp1/index.html"/>
    </rdf:Description>
    


    <!-- http://purl.org/dc/terms/ISO639-2 -->

    <rdf:Description rdf:about="http://purl.org/dc/terms/ISO639-2">
        <rdf:type rdf:resource="http://purl.org/dc/terms/LanguageScheme"/>
        <dc:type rdf:resource="http://dublincore.org/usage/documents/principles/#encoding-scheme"/>
        <terms:hasVersion rdf:resource="http://dublincore.org/usage/terms/history/#ISO639-2-002"/>
        <terms:issued>2000-07-11</terms:issued>
        <terms:modified>2002-06-15</terms:modified>
        <rdfs:comment xml:lang="en-us">ISO 639-2: Codes for the representation of names of languages.</rdfs:comment>
        <rdfs:isDefinedBy rdf:resource="http://purl.org/dc/terms/"/>
        <rdfs:label xml:lang="en-us">ISO 639-2</rdfs:label>
        <rdfs:seeAlso rdf:resource="http://lcweb.loc.gov/standards/iso639-2/langhome.html"/>
    </rdf:Description>
    


    <!-- http://purl.org/dc/terms/LCC -->

    <rdf:Description rdf:about="http://purl.org/dc/terms/LCC">
        <rdf:type rdf:resource="http://purl.org/dc/terms/SubjectScheme"/>
        <dc:type rdf:resource="http://dublincore.org/usage/documents/principles/#encoding-scheme"/>
        <terms:hasVersion rdf:resource="http://dublincore.org/usage/terms/history/#LCC-002"/>
        <terms:issued>2000-07-11</terms:issued>
        <terms:modified>2002-06-15</terms:modified>
        <rdfs:comment xml:lang="en-us">Library of Congress Classification</rdfs:comment>
        <rdfs:isDefinedBy rdf:resource="http://purl.org/dc/terms/"/>
        <rdfs:label xml:lang="en-us">LCC</rdfs:label>
        <rdfs:seeAlso rdf:resource="http://lcweb.loc.gov/catdir/cpso/lcco/lcco.html"/>
    </rdf:Description>
    


    <!-- http://purl.org/dc/terms/LCSH -->

    <rdf:Description rdf:about="http://purl.org/dc/terms/LCSH">
        <rdf:type rdf:resource="http://purl.org/dc/terms/SubjectScheme"/>
        <dc:type rdf:resource="http://dublincore.org/usage/documents/principles/#encoding-scheme"/>
        <terms:hasVersion rdf:resource="http://dublincore.org/usage/terms/history/#LCSH-002"/>
        <terms:issued>2000-07-11</terms:issued>
        <terms:modified>2002-06-15</terms:modified>
        <rdfs:comment xml:lang="en-us">Library of Congress Subject Headings</rdfs:comment>
        <rdfs:isDefinedBy rdf:resource="http://purl.org/dc/terms/"/>
        <rdfs:label xml:lang="en-us">LCSH</rdfs:label>
    </rdf:Description>
    


    <!-- http://purl.org/dc/terms/MESH -->

    <rdf:Description rdf:about="http://purl.org/dc/terms/MESH">
        <rdf:type rdf:resource="http://purl.org/dc/terms/SubjectScheme"/>
        <dc:type rdf:resource="http://dublincore.org/usage/documents/principles/#encoding-scheme"/>
        <terms:hasVersion rdf:resource="http://dublincore.org/usage/terms/history/#MESH-002"/>
        <terms:issued>2000-07-11</terms:issued>
        <terms:modified>2002-06-15</terms:modified>
        <rdfs:comment xml:lang="en-us">Medical Subject Headings</rdfs:comment>
        <rdfs:isDefinedBy rdf:resource="http://purl.org/dc/terms/"/>
        <rdfs:label xml:lang="en-us">MeSH</rdfs:label>
        <rdfs:seeAlso rdf:resource="http://www.nlm.nih.gov/mesh/meshhome.html"/>
    </rdf:Description>
    


    <!-- http://purl.org/dc/terms/Period -->

    <rdf:Description rdf:about="http://purl.org/dc/terms/Period">
        <rdf:type rdf:resource="http://purl.org/dc/terms/DateScheme"/>
        <rdf:type rdf:resource="http://purl.org/dc/terms/TemporalScheme"/>
        <dc:type rdf:resource="http://dublincore.org/usage/documents/principles/#encoding-scheme"/>
        <terms:hasVersion rdf:resource="http://dublincore.org/usage/terms/history/#Period-002"/>
        <terms:issued>2000-07-11</terms:issued>
        <terms:modified>2002-06-15</terms:modified>
        <rdfs:comment xml:lang="en-us">A specification of the limits of a time interval.</rdfs:comment>
        <rdfs:isDefinedBy rdf:resource="http://purl.org/dc/terms/"/>
        <rdfs:label xml:lang="en-us">DCMI Period</rdfs:label>
        <rdfs:seeAlso rdf:resource="http://dublincore.org/documents/dcmi-period/"/>
    </rdf:Description>
    


    <!-- http://purl.org/dc/terms/Point -->

    <rdf:Description rdf:about="http://purl.org/dc/terms/Point">
        <rdf:type rdf:resource="http://purl.org/dc/terms/SpatialScheme"/>
        <dc:type rdf:resource="http://dublincore.org/usage/documents/principles/#encoding-scheme"/>
        <terms:hasVersion rdf:resource="http://dublincore.org/usage/terms/history/#Point-002"/>
        <terms:issued>2000-07-11</terms:issued>
        <terms:modified>2002-06-15</terms:modified>
        <rdfs:comment xml:lang="en-us">The DCMI Point identifies a point in space using its geographic coordinates.</rdfs:comment>
        <rdfs:isDefinedBy rdf:resource="http://purl.org/dc/terms/"/>
        <rdfs:label xml:lang="en-us">DCMI Point</rdfs:label>
        <rdfs:seeAlso rdf:resource="http://dublincore.org/documents/dcmi-point/"/>
    </rdf:Description>
    


    <!-- http://purl.org/dc/terms/RFC1766 -->

    <rdf:Description rdf:about="http://purl.org/dc/terms/RFC1766">
        <rdf:type rdf:resource="http://purl.org/dc/terms/LanguageScheme"/>
        <dc:type rdf:resource="http://dublincore.org/usage/documents/principles/#encoding-scheme"/>
        <terms:hasVersion rdf:resource="http://dublincore.org/usage/terms/history/#RFC1766-002"/>
        <terms:issued>2000-07-11</terms:issued>
        <terms:modified>2002-06-15</terms:modified>
        <rdfs:comment xml:lang="en-us">Internet RFC 1766 &apos;Tags for the identification of Language&apos; 
                                            specifies a two letter code taken from ISO 639, followed 
                                            optionally by a two letter country code taken from ISO 3166.</rdfs:comment>
        <rdfs:isDefinedBy rdf:resource="http://purl.org/dc/terms/"/>
        <rdfs:label xml:lang="en-us">RFC 1766</rdfs:label>
        <rdfs:seeAlso rdf:resource="http://www.ietf.org/rfc/rfc1766.txt"/>
    </rdf:Description>
    


    <!-- http://purl.org/dc/terms/RFC3066 -->

    <rdf:Description rdf:about="http://purl.org/dc/terms/RFC3066">
        <rdf:type rdf:resource="http://purl.org/dc/terms/LanguageScheme"/>
        <dc:type rdf:resource="http://dublincore.org/usage/documents/principles/#encoding-scheme"/>
        <terms:hasVersion rdf:resource="http://dublincore.org/usage/terms/history/#RFC3066-001"/>
        <terms:issued>2002-07-13</terms:issued>
        <rdfs:comment xml:lang="en-us">Internet RFC 3066 &apos;Tags for the Identification of 
            Languages&apos; specifies a primary subtag which
            is a two-letter code taken from ISO 639 part
            1 or a three-letter code taken from ISO 639
            part 2, followed optionally by a two-letter
            country code taken from ISO 3166.  When a
            language in ISO 639 has both a two-letter and
            three-letter code, use the two-letter code;
            when it has only a three-letter code, use the
            three-letter code.  This RFC replaces RFC
            1766.</rdfs:comment>
        <rdfs:isDefinedBy rdf:resource="http://purl.org/dc/terms/"/>
        <rdfs:label xml:lang="en-us">RFC 3066</rdfs:label>
    </rdf:Description>
    


    <!-- http://purl.org/dc/terms/TGN -->

    <rdf:Description rdf:about="http://purl.org/dc/terms/TGN">
        <rdf:type rdf:resource="http://purl.org/dc/terms/SpatialScheme"/>
        <dc:type rdf:resource="http://dublincore.org/usage/documents/principles/#encoding-scheme"/>
        <terms:hasVersion rdf:resource="http://dublincore.org/usage/terms/history/#TGN-002"/>
        <terms:issued>2000-07-11</terms:issued>
        <terms:modified>2002-06-15</terms:modified>
        <rdfs:comment xml:lang="en-us">The Getty Thesaurus of Geographic Names</rdfs:comment>
        <rdfs:isDefinedBy rdf:resource="http://purl.org/dc/terms/"/>
        <rdfs:label xml:lang="en-us">TGN</rdfs:label>
        <rdfs:seeAlso rdf:resource="http://www.getty.edu/research/tools/vocabulary/tgn/index.html"/>
    </rdf:Description>
    


    <!-- http://purl.org/dc/terms/UDC -->

    <rdf:Description rdf:about="http://purl.org/dc/terms/UDC">
        <rdf:type rdf:resource="http://purl.org/dc/terms/SubjectScheme"/>
        <dc:type rdf:resource="http://dublincore.org/usage/documents/principles/#encoding-scheme"/>
        <terms:hasVersion rdf:resource="http://dublincore.org/usage/terms/history/#UDC-002"/>
        <terms:issued>2000-07-11</terms:issued>
        <terms:modified>2002-06-15</terms:modified>
        <rdfs:comment xml:lang="en-us">Universal Decimal Classification</rdfs:comment>
        <rdfs:isDefinedBy rdf:resource="http://purl.org/dc/terms/"/>
        <rdfs:label xml:lang="en-us">UDC</rdfs:label>
        <rdfs:seeAlso rdf:resource="http://www.udcc.org/"/>
    </rdf:Description>
    


    <!-- http://purl.org/dc/terms/URI -->

    <rdf:Description rdf:about="http://purl.org/dc/terms/URI">
        <rdf:type rdf:resource="http://purl.org/dc/terms/IdentifierScheme"/>
        <rdf:type rdf:resource="http://purl.org/dc/terms/RelationScheme"/>
        <rdf:type rdf:resource="http://purl.org/dc/terms/SourceScheme"/>
        <dc:type rdf:resource="http://dublincore.org/usage/documents/principles/#encoding-scheme"/>
        <terms:hasVersion rdf:resource="http://dublincore.org/usage/terms/history/#URI-002"/>
        <terms:issued>2000-07-11</terms:issued>
        <terms:modified>2002-06-15</terms:modified>
        <rdfs:comment xml:lang="en-us">A URI Uniform Resource Identifier</rdfs:comment>
        <rdfs:isDefinedBy rdf:resource="http://purl.org/dc/terms/"/>
        <rdfs:label xml:lang="en-us">URI</rdfs:label>
        <rdfs:seeAlso rdf:resource="http://www.ietf.org/rfc/rfc2396.txt"/>
    </rdf:Description>
    


    <!-- http://purl.org/dc/terms/W3CDTF -->

    <rdf:Description rdf:about="http://purl.org/dc/terms/W3CDTF">
        <rdf:type rdf:resource="http://purl.org/dc/terms/DateScheme"/>
        <rdf:type rdf:resource="http://purl.org/dc/terms/TemporalScheme"/>
        <dc:type rdf:resource="http://dublincore.org/usage/documents/principles/#encoding-scheme"/>
        <terms:hasVersion rdf:resource="http://dublincore.org/usage/terms/history/#W3CDTF-002"/>
        <terms:issued>2000-07-11</terms:issued>
        <terms:modified>2002-06-15</terms:modified>
        <rdfs:comment xml:lang="en-us">W3C Encoding rules for dates and times - a profile based on ISO 8601</rdfs:comment>
        <rdfs:isDefinedBy rdf:resource="http://purl.org/dc/terms/"/>
        <rdfs:label xml:lang="en-us">W3C-DTF</rdfs:label>
        <rdfs:seeAlso rdf:resource="http://www.w3.org/TR/NOTE-datetime"/>
    </rdf:Description>
    


    <!-- http://rdfs.org/ns/void#uriRegexPattern -->

    <rdf:Description rdf:about="http://rdfs.org/ns/void#uriRegexPattern">
        <rdf:type rdf:resource="http://www.w3.org/1999/02/22-rdf-syntax-ns#DatatypeProperty"/>
    </rdf:Description>
    


    <!-- http://vocab.deri.ie/void -->

    <rdf:Description rdf:about="http://vocab.deri.ie/void">
        <rdf:type rdf:resource="http://www.w3.org/ns/adms#SemanticAsset"/>
    </rdf:Description>
    


    <!-- http://vocab.deri.ie/void.html -->

    <owl:NamedIndividual rdf:about="http://vocab.deri.ie/void.html"/>
    


    <!-- http://vocab.deri.ie/void#rdf -->

    <rdf:Description rdf:about="http://vocab.deri.ie/void#rdf">
        <rdf:type rdf:resource="http://www.w3.org/ns/adms#SemanticDistribution"/>
        <terms:FileFormat rdf:resource="http://vocab.deri.ie/"/>
        <adms:accessURL>http://vocab.deri.ie/void.rdf</adms:accessURL>
        <adms:status rdf:resource="http://purl.org/adms/status/Completed"/>
    </rdf:Description>
    


    <!-- http://vocab.deri.ie/void#ttl -->

    <rdf:Description rdf:about="http://vocab.deri.ie/void#ttl">
        <rdf:type rdf:resource="http://www.w3.org/ns/adms#SemanticDistribution"/>
        <terms:FileFormat rdf:resource="http://vocab.deri.ie/"/>
        <adms:accessURL>http://vocab.deri.ie/void.ttl</adms:accessURL>
        <adms:status rdf:resource="http://purl.org/adms/status/Completed"/>
    </rdf:Description>
    


    <!-- http://www.openannotation.org/spec/core/20130208/oa.owl -->

    <owl:NamedIndividual rdf:about="http://www.openannotation.org/spec/core/20130208/oa.owl"/>
    


    <!-- http://www.semanticweb.org/k_mil/ontologies/2021/8/EvalLOD -->

    <owl:NamedIndividual rdf:about="http://www.semanticweb.org/k_mil/ontologies/2021/8/EvalLOD">
        <prov:wasRevisionOf rdf:resource="http://www.openannotation.org/spec/core/20130208/oa.owl"/>
        <foaf:homepage rdf:resource="http://vocab.deri.ie/void.html"/>
    </owl:NamedIndividual>
    


    <!-- http://www.semanticweb.org/k_mil/ontologies/2021/8/EvalLOD#EvalloPlatform -->

    <owl:NamedIndividual rdf:about="http://www.semanticweb.org/k_mil/ontologies/2021/8/EvalLOD#EvalloPlatform">
        <rdf:type rdf:resource="https://schema.org/Organization"/>
    </owl:NamedIndividual>
    


    <!-- http://www.w3.org/ns/oa#PreferContainedDescriptions -->

    <rdf:Description rdf:about="http://www.w3.org/ns/oa#PreferContainedDescriptions">
        <rdf:type rdf:resource="http://www.w3.org/2000/01/rdf-schema#Resource"/>
        <rdfs:comment>An IRI to signal the client prefers to receive full descriptions of the Annotations from a container, not just their IRIs.</rdfs:comment>
        <rdfs:isDefinedBy rdf:resource="http://www.w3.org/ns/oa#"/>
        <rdfs:label>PreferContainedDescriptions</rdfs:label>
    </rdf:Description>
    


    <!-- http://www.w3.org/ns/oa#PreferContainedIRIs -->

    <rdf:Description rdf:about="http://www.w3.org/ns/oa#PreferContainedIRIs">
        <rdf:type rdf:resource="http://www.w3.org/2000/01/rdf-schema#Resource"/>
        <rdfs:comment>An IRI to signal that the client prefers to receive only the IRIs of the Annotations from a container, not their full descriptions.</rdfs:comment>
        <rdfs:isDefinedBy rdf:resource="http://www.w3.org/ns/oa#"/>
        <rdfs:label>PreferContainedIRIs</rdfs:label>
    </rdf:Description>
    


    <!-- http://www.w3.org/ns/oa#assessing -->

    <rdf:Description rdf:about="http://www.w3.org/ns/oa#assessing">
        <rdf:type rdf:resource="http://www.w3.org/ns/oa#Motivation"/>
        <rdfs:comment>The motivation for when the user intends to provide an assessment about the Target resource.</rdfs:comment>
        <rdfs:isDefinedBy rdf:resource="http://www.w3.org/ns/oa#"/>
        <rdfs:label>assessing</rdfs:label>
    </rdf:Description>
    


    <!-- http://www.w3.org/ns/oa#bookmarking -->

    <rdf:Description rdf:about="http://www.w3.org/ns/oa#bookmarking">
        <rdf:type rdf:resource="http://www.w3.org/ns/oa#Motivation"/>
        <rdfs:comment>The motivation for when the user intends to create a bookmark to the Target or part thereof.</rdfs:comment>
        <rdfs:isDefinedBy rdf:resource="http://www.w3.org/ns/oa#"/>
        <rdfs:label>bookmarking</rdfs:label>
    </rdf:Description>
    


    <!-- http://www.w3.org/ns/oa#classifying -->

    <rdf:Description rdf:about="http://www.w3.org/ns/oa#classifying">
        <rdf:type rdf:resource="http://www.w3.org/ns/oa#Motivation"/>
        <rdfs:comment>The motivation for when the user intends to that classify the Target as something.</rdfs:comment>
        <rdfs:isDefinedBy rdf:resource="http://www.w3.org/ns/oa#"/>
        <rdfs:label>classifying</rdfs:label>
    </rdf:Description>
    


    <!-- http://www.w3.org/ns/oa#commenting -->

    <rdf:Description rdf:about="http://www.w3.org/ns/oa#commenting">
        <rdf:type rdf:resource="http://www.w3.org/ns/oa#Motivation"/>
        <rdfs:comment>The motivation for when the user intends to comment about the Target.</rdfs:comment>
        <rdfs:isDefinedBy rdf:resource="http://www.w3.org/ns/oa#"/>
        <rdfs:label>commenting</rdfs:label>
    </rdf:Description>
    


    <!-- http://www.w3.org/ns/oa#describing -->

    <rdf:Description rdf:about="http://www.w3.org/ns/oa#describing">
        <rdf:type rdf:resource="http://www.w3.org/ns/oa#Motivation"/>
        <rdfs:comment>The motivation for when the user intends to describe the Target, as opposed to a comment about them.</rdfs:comment>
        <rdfs:isDefinedBy rdf:resource="http://www.w3.org/ns/oa#"/>
        <rdfs:label>describing</rdfs:label>
    </rdf:Description>
    


    <!-- http://www.w3.org/ns/oa#editing -->

    <rdf:Description rdf:about="http://www.w3.org/ns/oa#editing">
        <rdf:type rdf:resource="http://www.w3.org/ns/oa#Motivation"/>
        <rdfs:comment>The motivation for when the user intends to request a change or edit to the Target resource.</rdfs:comment>
        <rdfs:isDefinedBy rdf:resource="http://www.w3.org/ns/oa#"/>
        <rdfs:label>editing</rdfs:label>
    </rdf:Description>
    


    <!-- http://www.w3.org/ns/oa#highlighting -->

    <rdf:Description rdf:about="http://www.w3.org/ns/oa#highlighting">
        <rdf:type rdf:resource="http://www.w3.org/ns/oa#Motivation"/>
        <rdfs:comment>The motivation for when the user intends to highlight the Target resource or segment of it.</rdfs:comment>
        <rdfs:isDefinedBy rdf:resource="http://www.w3.org/ns/oa#"/>
        <rdfs:label>highlighting</rdfs:label>
    </rdf:Description>
    


    <!-- http://www.w3.org/ns/oa#identifying -->

    <rdf:Description rdf:about="http://www.w3.org/ns/oa#identifying">
        <rdf:type rdf:resource="http://www.w3.org/ns/oa#Motivation"/>
        <rdfs:comment>The motivation for when the user intends to assign an identity to the Target or identify what is being depicted or described in the Target.</rdfs:comment>
        <rdfs:isDefinedBy rdf:resource="http://www.w3.org/ns/oa#"/>
        <rdfs:label>identifying</rdfs:label>
    </rdf:Description>
    


    <!-- http://www.w3.org/ns/oa#linking -->

    <rdf:Description rdf:about="http://www.w3.org/ns/oa#linking">
        <rdf:type rdf:resource="http://www.w3.org/ns/oa#Motivation"/>
        <rdfs:comment>The motivation for when the user intends to link to a resource related to the Target.</rdfs:comment>
        <rdfs:isDefinedBy rdf:resource="http://www.w3.org/ns/oa#"/>
        <rdfs:label>linking</rdfs:label>
    </rdf:Description>
    


    <!-- http://www.w3.org/ns/oa#ltrDirection -->

    <rdf:Description rdf:about="http://www.w3.org/ns/oa#ltrDirection">
        <rdf:type rdf:resource="http://www.w3.org/ns/oa#Direction"/>
        <rdfs:comment>The direction of text that is read from left to right.</rdfs:comment>
        <rdfs:isDefinedBy rdf:resource="http://www.w3.org/ns/oa#"/>
        <rdfs:label>ltrDirection</rdfs:label>
    </rdf:Description>
    


    <!-- http://www.w3.org/ns/oa#moderating -->

    <rdf:Description rdf:about="http://www.w3.org/ns/oa#moderating">
        <rdf:type rdf:resource="http://www.w3.org/ns/oa#Motivation"/>
        <rdfs:comment>The motivation for when the user intends to assign some value or quality to the Target.</rdfs:comment>
        <rdfs:isDefinedBy rdf:resource="http://www.w3.org/ns/oa#"/>
        <rdfs:label>moderating</rdfs:label>
    </rdf:Description>
    


    <!-- http://www.w3.org/ns/oa#questioning -->

    <rdf:Description rdf:about="http://www.w3.org/ns/oa#questioning">
        <rdf:type rdf:resource="http://www.w3.org/ns/oa#Motivation"/>
        <rdfs:comment>The motivation for when the user intends to ask a question about the Target.</rdfs:comment>
        <rdfs:isDefinedBy rdf:resource="http://www.w3.org/ns/oa#"/>
        <rdfs:label>questioning</rdfs:label>
    </rdf:Description>
    


    <!-- http://www.w3.org/ns/oa#replying -->

    <rdf:Description rdf:about="http://www.w3.org/ns/oa#replying">
        <rdf:type rdf:resource="http://www.w3.org/ns/oa#Motivation"/>
        <rdfs:comment>The motivation for when the user intends to reply to a previous statement, either an Annotation or another resource.</rdfs:comment>
        <rdfs:isDefinedBy rdf:resource="http://www.w3.org/ns/oa#"/>
        <rdfs:label>replying</rdfs:label>
    </rdf:Description>
    


    <!-- http://www.w3.org/ns/oa#rtlDirection -->

    <rdf:Description rdf:about="http://www.w3.org/ns/oa#rtlDirection">
        <rdf:type rdf:resource="http://www.w3.org/ns/oa#Direction"/>
        <rdfs:comment>The direction of text that is read from right to left.</rdfs:comment>
        <rdfs:isDefinedBy rdf:resource="http://www.w3.org/ns/oa#"/>
        <rdfs:label>rtlDirection</rdfs:label>
    </rdf:Description>
    


    <!-- http://www.w3.org/ns/oa#tagging -->

    <rdf:Description rdf:about="http://www.w3.org/ns/oa#tagging">
        <rdf:type rdf:resource="http://www.w3.org/ns/oa#Motivation"/>
        <rdfs:comment>The motivation for when the user intends to associate a tag with the Target.</rdfs:comment>
        <rdfs:isDefinedBy rdf:resource="http://www.w3.org/ns/oa#"/>
        <rdfs:label>tagging</rdfs:label>
    </rdf:Description>
    


    <!-- http://www.w3.org/ns/prov#EmptyCollection -->

    <owl:NamedIndividual rdf:about="http://www.w3.org/ns/prov#EmptyCollection"/>
    


    <!-- http://www.w3.org/ns/prov-o# -->

    <rdf:Description rdf:about="http://www.w3.org/ns/prov-o#">
        <prov:specializationOf rdf:resource="http://www.w3.org/ns/prov-o"/>
        <prov:wasRevisionOf rdf:resource="http://www.w3.org/ns/prov-o-20120312"/>
    </rdf:Description>
    


    <!-- https://bioportal.bioontology.org/ontologies/MEDDRA -->

    <owl:NamedIndividual rdf:about="https://bioportal.bioontology.org/ontologies/MEDDRA">
        <rdf:type rdf:resource="http://rdfs.org/ns/void#Dataset"/>
        <dc:date>January 6, 2023</dc:date>
        <dc:description>MedDRA is an international medical terminology with an emphasis on use for data entry, retrieval, analysis, and display. It applies to all phases of drug development, excluding animal toxicology, and to the health effects and malfunction of devices. An appendix includes concept descriptions which describe how a medical concept is interpreted, used, and classified within the MedDRA terminology. It is not intended as a medical definition. The concept descriptions are intended to aid the consistent and accurate use of MedDRA in coding, retrieval, and analysis.</dc:description>
        <dc:title>Medical Dictionary for Regulatory Activities Terminology (MedDRA)</dc:title>
        <adms:accessURL>https://bioportal.bioontology.org/ontologies/MEDDRA</adms:accessURL>
    </owl:NamedIndividual>
    <rdf:Description>
        <rdf:type rdf:resource="https://schema.org/Person"/>
        <schema:affiliation>
            <rdf:Description>
                <rdf:type rdf:resource="https://schema.org/Organization"/>
            </rdf:Description>
        </schema:affiliation>
        <schema:email rdf:resource="mailto:richard.cyganiak@deri.org"/>
        <schema:name>Richard Cyganiak</schema:name>
        <schema:url rdf:resource="http://richard.cyganiak.de/"/>
    </rdf:Description>
    <rdf:Description>
        <rdf:type rdf:resource="https://schema.org/Person"/>
        <schema:affiliation>
            <rdf:Description>
                <rdf:type rdf:resource="https://schema.org/Organization"/>
                <schema:name>Department of Zoology, University of Oxford</schema:name>
                <schema:url rdf:resource="http://www.zoo.ox.ac.uk/"/>
            </rdf:Description>
        </schema:affiliation>
        <schema:email rdf:resource="mailto:jun.zhao@zoo.ox.ac.uk"/>
        <schema:name>Jun Zhao</schema:name>
        <schema:url rdf:resource="http://users.ox.ac.uk/~zool0770/"/>
    </rdf:Description>
    <rdf:Description>
        <rdf:type rdf:resource="https://schema.org/Person"/>
        <schema:affiliation>
            <rdf:Description>
                <rdf:type rdf:resource="https://schema.org/Organization"/>
                <schema:name>Talis</schema:name>
                <schema:url rdf:resource="http://www.talis.com/"/>
            </rdf:Description>
        </schema:affiliation>
        <schema:email rdf:resource="mailto:Keith.Alexander@talis.com"/>
        <schema:name>Keith Alexander</schema:name>
        <schema:url rdf:resource="http://kwijibo.talis.com/"/>
    </rdf:Description>
    <rdf:Description>
        <rdf:type rdf:resource="https://schema.org/Person"/>
        <schema:affiliation>
            <rdf:Description>
                <rdf:type rdf:resource="https://schema.org/Organization"/>
                <schema:name>LiDRC</schema:name>
                <schema:url rdf:resource="http://linkeddata.deri.ie/"/>
            </rdf:Description>
        </schema:affiliation>
        <schema:email rdf:resource="mailto:michael.hausenblas@deri.org"/>
        <schema:name>Michael Hausenblas</schema:name>
        <schema:url rdf:resource="http://sw-app.org/about.html"/>
    </rdf:Description>
    <rdf:Description>
        <rdf:type rdf:resource="http://xmlns.com/foaf/0.1/Person"/>
    </rdf:Description>
    <rdf:Description>
        <rdf:type rdf:resource="http://xmlns.com/foaf/0.1/Person"/>
    </rdf:Description>
    <rdf:Description>
        <rdf:type rdf:resource="http://xmlns.com/foaf/0.1/Person"/>
    </rdf:Description>
    <rdf:Description>
        <rdf:type rdf:resource="https://schema.org/Person"/>
        <schema:affiliation>
            <rdf:Description>
                <rdf:type rdf:resource="https://schema.org/Organization"/>
            </rdf:Description>
        </schema:affiliation>
        <schema:email rdf:resource="mailto:richard.cyganiak@deri.org"/>
        <schema:name>Richard Cyganiak</schema:name>
        <schema:url rdf:resource="http://richard.cyganiak.de/"/>
    </rdf:Description>
    <rdf:Description>
        <rdf:type rdf:resource="https://schema.org/Person"/>
        <schema:affiliation>
            <rdf:Description>
                <rdf:type rdf:resource="https://schema.org/Organization"/>
                <schema:name>Department of Zoology, University of Oxford</schema:name>
                <schema:url rdf:resource="http://www.zoo.ox.ac.uk/"/>
            </rdf:Description>
        </schema:affiliation>
        <schema:email rdf:resource="mailto:jun.zhao@zoo.ox.ac.uk"/>
        <schema:name>Jun Zhao</schema:name>
        <schema:url rdf:resource="http://users.ox.ac.uk/~zool0770/"/>
    </rdf:Description>
    <rdf:Description>
        <rdf:type rdf:resource="https://schema.org/Person"/>
        <schema:affiliation>
            <rdf:Description>
                <rdf:type rdf:resource="https://schema.org/Organization"/>
                <schema:name>Talis</schema:name>
                <schema:url rdf:resource="http://www.talis.com/"/>
            </rdf:Description>
        </schema:affiliation>
        <schema:email rdf:resource="mailto:Keith.Alexander@talis.com"/>
        <schema:name>Keith Alexander</schema:name>
        <schema:url rdf:resource="http://kwijibo.talis.com/"/>
    </rdf:Description>
    <rdf:Description>
        <rdf:type rdf:resource="https://schema.org/Person"/>
        <schema:affiliation>
            <rdf:Description>
                <rdf:type rdf:resource="https://schema.org/Organization"/>
                <schema:name>LiDRC</schema:name>
                <schema:url rdf:resource="http://linkeddata.deri.ie/"/>
            </rdf:Description>
        </schema:affiliation>
        <schema:email rdf:resource="mailto:michael.hausenblas@deri.org"/>
        <schema:name>Michael Hausenblas</schema:name>
        <schema:url rdf:resource="http://sw-app.org/about.html"/>
    </rdf:Description>
    <rdf:Description>
        <rdf:type rdf:resource="http://xmlns.com/foaf/0.1/Person"/>
    </rdf:Description>
    <rdf:Description>
        <rdf:type rdf:resource="http://xmlns.com/foaf/0.1/Person"/>
    </rdf:Description>
    <rdf:Description>
        <rdf:type rdf:resource="http://xmlns.com/foaf/0.1/Person"/>
    </rdf:Description>
    <rdf:Description>
        <foaf:homepage rdf:resource="http://www.deri.ie/"/>
    </rdf:Description>
    <rdf:Description>
        <rdfs:seeAlso rdf:resource="http://www.insight-centre.org"/>
        <rdfs:seeAlso rdf:resource="http://www.deri.ie/"/>
        <schema:identifier rdf:resource="http://vocab.deri.ie/void#Digital%20Enterprise%20Research%20Institute%2C%20NUI%20Galway"/>
        <schema:name>Digital Enterprise Research Institute, NUI Galway</schema:name>
    </rdf:Description>
    <rdf:Description>
        <rdfs:seeAlso rdf:resource="http://www.insight-centre.org"/>
        <rdfs:seeAlso rdf:resource="http://www.deri.ie/"/>
        <schema:identifier rdf:resource="http://vocab.deri.ie/void#Digital%20Enterprise%20Research%20Institute%2C%20NUI%20Galway"/>
        <schema:name>Digital Enterprise Research Institute, NUI Galway</schema:name>
    </rdf:Description>
    <rdf:Description>
        <foaf:name>Benjamin Young</foaf:name>
    </rdf:Description>
    <rdf:Description>
        <foaf:name>Robert Sanderson</foaf:name>
    </rdf:Description>
    <rdf:Description>
        <foaf:name>Paolo Ciccarese</foaf:name>
    </rdf:Description>
    <rdf:Description>
        <foaf:name>Digital Enterprise Research Institute, NUI Galway</foaf:name>
    </rdf:Description>
    <rdf:Description>
        <owl:maxCardinality rdf:datatype="http://www.w3.org/2001/XMLSchema#int">1</owl:maxCardinality>
    </rdf:Description>
    


    <!-- 
    ///////////////////////////////////////////////////////////////////////////////////////
    //
    // Annotations
    //
    ///////////////////////////////////////////////////////////////////////////////////////
     -->

    <rdf:Description rdf:about="http://rdfs.org/ns/void#uriRegexPattern">
        <rdfs:comment>Defines a regular expression pattern matching URIs in the dataset.</rdfs:comment>
        <rdfs:label>has URI regular expression pattern</rdfs:label>
    </rdf:Description>
    <rdf:Description rdf:about="http://www.w3.org/ns/oa#annotationService">
        <rdfs:comment>The object of the relationship is the end point of a service that conforms to the annotation-protocol, and it may be associated with any resource.  The expectation of asserting the relationship is that the object is the preferred service for maintaining annotations about the subject resource, according to the publisher of the relationship.

  This relationship is intended to be used both within Linked Data descriptions and as the  rel  type of a Link, via HTTP Link Headers rfc5988 for binary resources and in HTML &lt;link&gt; elements.  For more information about these, please see the Annotation Protocol specification annotation-protocol.
  </rdfs:comment>
        <rdfs:isDefinedBy rdf:resource="http://www.w3.org/ns/oa#"/>
        <rdfs:label>annotationService</rdfs:label>
    </rdf:Description>
    <rdf:Description rdf:about="http://www.w3.org/ns/oa#canonical">
        <rdfs:comment>A object of the relationship is the canonical IRI that can always be used to deduplicate the Annotation, regardless of the current IRI used to access the representation.</rdfs:comment>
        <rdfs:isDefinedBy rdf:resource="http://www.w3.org/ns/oa#"/>
        <rdfs:label>canonical</rdfs:label>
    </rdf:Description>
    <rdf:Description rdf:about="http://www.w3.org/ns/oa#refinedBy">
        <rdfs:comment>The relationship between a Selector and another Selector or a State and a Selector or State that should be applied to the results of the first to refine the processing of the source resource. </rdfs:comment>
        <rdfs:isDefinedBy rdf:resource="http://www.w3.org/ns/oa#"/>
        <rdfs:label>refinedBy</rdfs:label>
    </rdf:Description>
    <rdf:Description rdf:about="http://www.w3.org/ns/oa#via">
        <rdfs:comment>A object of the relationship is a resource from which the source resource was retrieved by the providing system.</rdfs:comment>
        <rdfs:isDefinedBy rdf:resource="http://www.w3.org/ns/oa#"/>
        <rdfs:label>via</rdfs:label>
    </rdf:Description>
    <rdf:Description rdf:about="http://www.w3.org/ns/prov#EmptyCollection">
        <rdfs:isDefinedBy rdf:resource="http://www.w3.org/ns/prov-o#"/>
        <rdfs:label xml:lang="en">EmptyCollection</rdfs:label>
        <prov:category>expanded</prov:category>
        <prov:component>collections</prov:component>
        <prov:definition xml:lang="en">An empty collection is a collection without members.</prov:definition>
    </rdf:Description>
    <rdf:Description rdf:about="http://www.w3.org/ns/prov#specializationOf">
        <rdfs:isDefinedBy rdf:resource="http://www.w3.org/ns/prov-o#"/>
        <rdfs:label>specializationOf</rdfs:label>
        <rdfs:seeAlso rdf:resource="http://www.w3.org/ns/prov#alternateOf"/>
        <prov:category>expanded</prov:category>
        <prov:component>alternate</prov:component>
        <prov:constraints rdf:datatype="http://www.w3.org/2001/XMLSchema#anyURI">http://www.w3.org/TR/2013/REC-prov-constraints-20130430/#prov-dm-constraints-fig</prov:constraints>
        <prov:definition xml:lang="en">An entity that is a specialization of another shares all aspects of the latter, and additionally presents more specific aspects of the same thing as the latter. In particular, the lifetime of the entity being specialized contains that of any specialization. Examples of aspects include a time period, an abstraction, and a context associated with the entity.</prov:definition>
        <prov:dm rdf:datatype="http://www.w3.org/2001/XMLSchema#anyURI">http://www.w3.org/TR/2013/REC-prov-dm-20130430/#term-specialization</prov:dm>
        <prov:inverse>generalizationOf</prov:inverse>
        <prov:n rdf:datatype="http://www.w3.org/2001/XMLSchema#anyURI">http://www.w3.org/TR/2013/REC-prov-n-20130430/#expression-specialization</prov:n>
    </rdf:Description>
    <rdf:Description rdf:about="http://www.w3.org/ns/prov#wasRevisionOf">
        <rdfs:comment xml:lang="en">A revision is a derivation that revises an entity into a revised version.</rdfs:comment>
        <rdfs:isDefinedBy rdf:resource="http://www.w3.org/ns/prov-o#"/>
        <rdfs:label>wasRevisionOf</rdfs:label>
        <prov:category>expanded</prov:category>
        <prov:component>derivations</prov:component>
        <prov:inverse>hadRevision</prov:inverse>
        <prov:qualifiedForm rdf:resource="http://www.w3.org/ns/prov#Revision"/>
        <prov:qualifiedForm rdf:resource="http://www.w3.org/ns/prov#qualifiedRevision"/>
    </rdf:Description>
    <rdf:Description rdf:about="http://xmlns.com/foaf/0.1/name">
        <rdfs:comment>A name for some thing.</rdfs:comment>
        <rdfs:isDefinedBy rdf:resource="http://xmlns.com/foaf/0.1/"/>
        <rdfs:label>name</rdfs:label>
        <ns:term_status>testing</ns:term_status>
    </rdf:Description>
    <rdf:Description rdf:about="http://xmlns.com/foaf/0.1/nick">
        <rdfs:comment>A short informal nickname characterising an agent (includes login identifiers, IRC and other chat nicknames).</rdfs:comment>
        <rdfs:isDefinedBy rdf:resource="http://xmlns.com/foaf/0.1/"/>
        <rdfs:label>nickname</rdfs:label>
        <ns:term_status>testing</ns:term_status>
    </rdf:Description>
    


    <!-- 
    ///////////////////////////////////////////////////////////////////////////////////////
    //
    // Rules
    //
    ///////////////////////////////////////////////////////////////////////////////////////
     -->

    <rdf:Description rdf:about="http://www.semanticweb.org/k_mil/ontologies/2021/8/EvalLOD#d">
        <rdf:type rdf:resource="http://www.w3.org/2003/11/swrl#Variable"/>
    </rdf:Description>
    <rdf:Description rdf:about="http://www.semanticweb.org/k_mil/ontologies/2021/8/EvalLOD#b">
        <rdf:type rdf:resource="http://www.w3.org/2003/11/swrl#Variable"/>
    </rdf:Description>
    <rdf:Description rdf:about="http://www.semanticweb.org/k_mil/ontologies/2021/8/EvalLOD#p">
        <rdf:type rdf:resource="http://www.w3.org/2003/11/swrl#Variable"/>
    </rdf:Description>
    <rdf:Description rdf:about="http://www.semanticweb.org/k_mil/ontologies/2021/8/EvalLOD#s">
        <rdf:type rdf:resource="http://www.w3.org/2003/11/swrl#Variable"/>
    </rdf:Description>
    <rdf:Description>
        <swrla:isRuleEnabled rdf:datatype="http://www.w3.org/2001/XMLSchema#boolean">true</swrla:isRuleEnabled>
        <rdfs:comment>Dataset(?d) ^ BlackList(?b) ^ belongsTo(?d, ?b) -&gt; blacklistedDataset(?d)</rdfs:comment>
        <rdfs:label>Validaciones listas negras</rdfs:label>
        <rdf:type rdf:resource="http://www.w3.org/2003/11/swrl#Imp"/>
        <swrl:body>
            <rdf:Description>
                <rdf:type rdf:resource="http://www.w3.org/2003/11/swrl#AtomList"/>
                <rdf:first>
                    <rdf:Description>
                        <rdf:type rdf:resource="http://www.w3.org/2003/11/swrl#ClassAtom"/>
                        <swrl:classPredicate rdf:resource="http://rdfs.org/ns/void#Dataset"/>
                        <swrl:argument1 rdf:resource="http://www.semanticweb.org/k_mil/ontologies/2021/8/EvalLOD#d"/>
                    </rdf:Description>
                </rdf:first>
                <rdf:rest>
                    <rdf:Description>
                        <rdf:type rdf:resource="http://www.w3.org/2003/11/swrl#AtomList"/>
                        <rdf:first>
                            <rdf:Description>
                                <rdf:type rdf:resource="http://www.w3.org/2003/11/swrl#ClassAtom"/>
                                <swrl:classPredicate rdf:resource="http://www.semanticweb.org/k_mil/ontologies/2021/8/EvalLOD#BlackList"/>
                                <swrl:argument1 rdf:resource="http://www.semanticweb.org/k_mil/ontologies/2021/8/EvalLOD#b"/>
                            </rdf:Description>
                        </rdf:first>
                        <rdf:rest>
                            <rdf:Description>
                                <rdf:type rdf:resource="http://www.w3.org/2003/11/swrl#AtomList"/>
                                <rdf:first>
                                    <rdf:Description>
                                        <rdf:type rdf:resource="http://www.w3.org/2003/11/swrl#IndividualPropertyAtom"/>
                                        <swrl:propertyPredicate rdf:resource="http://www.semanticweb.org/k_mil/ontologies/2021/8/EvalLOD#belongsTo"/>
                                        <swrl:argument1 rdf:resource="http://www.semanticweb.org/k_mil/ontologies/2021/8/EvalLOD#d"/>
                                        <swrl:argument2 rdf:resource="http://www.semanticweb.org/k_mil/ontologies/2021/8/EvalLOD#b"/>
                                    </rdf:Description>
                                </rdf:first>
                                <rdf:rest rdf:resource="http://www.w3.org/1999/02/22-rdf-syntax-ns#nil"/>
                            </rdf:Description>
                        </rdf:rest>
                    </rdf:Description>
                </rdf:rest>
            </rdf:Description>
        </swrl:body>
        <swrl:head>
            <rdf:Description>
                <rdf:type rdf:resource="http://www.w3.org/2003/11/swrl#AtomList"/>
                <rdf:first>
                    <rdf:Description>
                        <rdf:type rdf:resource="http://www.w3.org/2003/11/swrl#ClassAtom"/>
                        <swrl:classPredicate rdf:resource="http://www.semanticweb.org/k_mil/ontologies/2021/8/EvalLOD#blacklistedDataset"/>
                        <swrl:argument1 rdf:resource="http://www.semanticweb.org/k_mil/ontologies/2021/8/EvalLOD#d"/>
                    </rdf:Description>
                </rdf:first>
                <rdf:rest rdf:resource="http://www.w3.org/1999/02/22-rdf-syntax-ns#nil"/>
            </rdf:Description>
        </swrl:head>
    </rdf:Description>
    <rdf:Description>
        <swrla:isRuleEnabled rdf:datatype="http://www.w3.org/2001/XMLSchema#boolean">true</swrla:isRuleEnabled>
        <rdfs:comment>Construccin de grafos de confianza entre publicadores, y datasets</rdfs:comment>
        <rdfs:label>Confianza por autor o publicador</rdfs:label>
        <rdf:type rdf:resource="http://www.w3.org/2003/11/swrl#Imp"/>
        <swrl:body>
            <rdf:Description>
                <rdf:type rdf:resource="http://www.w3.org/2003/11/swrl#AtomList"/>
                <rdf:first>
                    <rdf:Description>
                        <rdf:type rdf:resource="http://www.w3.org/2003/11/swrl#ClassAtom"/>
                        <swrl:classPredicate rdf:resource="http://xmlns.com/foaf/0.1/Person"/>
                        <swrl:argument1 rdf:resource="http://www.semanticweb.org/k_mil/ontologies/2021/8/EvalLOD#p"/>
                    </rdf:Description>
                </rdf:first>
                <rdf:rest>
                    <rdf:Description>
                        <rdf:type rdf:resource="http://www.w3.org/2003/11/swrl#AtomList"/>
                        <rdf:first>
                            <rdf:Description>
                                <rdf:type rdf:resource="http://www.w3.org/2003/11/swrl#ClassAtom"/>
                                <swrl:classPredicate rdf:resource="http://rdfs.org/ns/void#Dataset"/>
                                <swrl:argument1 rdf:resource="http://www.semanticweb.org/k_mil/ontologies/2021/8/EvalLOD#d"/>
                            </rdf:Description>
                        </rdf:first>
                        <rdf:rest>
                            <rdf:Description>
                                <rdf:type rdf:resource="http://www.w3.org/2003/11/swrl#AtomList"/>
                                <rdf:first>
                                    <rdf:Description>
                                        <rdf:type rdf:resource="http://www.w3.org/2003/11/swrl#IndividualPropertyAtom"/>
                                        <swrl:propertyPredicate rdf:resource="http://www.semanticweb.org/k_mil/ontologies/2021/8/EvalLOD#publishedBy"/>
                                        <swrl:argument1 rdf:resource="http://www.semanticweb.org/k_mil/ontologies/2021/8/EvalLOD#s"/>
                                        <swrl:argument2 rdf:resource="http://www.semanticweb.org/k_mil/ontologies/2021/8/EvalLOD#p"/>
                                    </rdf:Description>
                                </rdf:first>
                                <rdf:rest>
                                    <rdf:Description>
                                        <rdf:type rdf:resource="http://www.w3.org/2003/11/swrl#AtomList"/>
                                        <rdf:first>
                                            <rdf:Description>
                                                <rdf:type rdf:resource="http://www.w3.org/2003/11/swrl#ClassAtom"/>
                                                <swrl:classPredicate rdf:resource="http://www.semanticweb.org/k_mil/ontologies/2021/8/EvalLOD#Trusted"/>
                                                <swrl:argument1 rdf:resource="http://www.semanticweb.org/k_mil/ontologies/2021/8/EvalLOD#p"/>
                                            </rdf:Description>
                                        </rdf:first>
                                        <rdf:rest rdf:resource="http://www.w3.org/1999/02/22-rdf-syntax-ns#nil"/>
                                    </rdf:Description>
                                </rdf:rest>
                            </rdf:Description>
                        </rdf:rest>
                    </rdf:Description>
                </rdf:rest>
            </rdf:Description>
        </swrl:body>
        <swrl:head>
            <rdf:Description>
                <rdf:type rdf:resource="http://www.w3.org/2003/11/swrl#AtomList"/>
                <rdf:first>
                    <rdf:Description>
                        <rdf:type rdf:resource="http://www.w3.org/2003/11/swrl#ClassAtom"/>
                        <swrl:classPredicate rdf:resource="http://www.semanticweb.org/k_mil/ontologies/2021/8/EvalLOD#Trusted"/>
                        <swrl:argument1 rdf:resource="http://www.semanticweb.org/k_mil/ontologies/2021/8/EvalLOD#d"/>
                    </rdf:Description>
                </rdf:first>
                <rdf:rest rdf:resource="http://www.w3.org/1999/02/22-rdf-syntax-ns#nil"/>
            </rdf:Description>
        </swrl:head>
    </rdf:Description>
</rdf:RDF>



<!-- Generated by the OWL API (version 4.5.25.2023-02-15T19:15:49Z) https://github.com/owlcs/owlapi -->

